<?xml version="1.0"?>
<rdf:RDF xmlns="http://purl.obolibrary.org/BCODMO_SM/matrix/material.owl#"
     xml:base="http://purl.obolibrary.org/BCODMO_SM/matrix/material.owl"
     xmlns:dc="http://purl.org/dc/elements/1.1/"
     xmlns:obo="http://purl.obolibrary.org/obo/"
     xmlns:owl="http://www.w3.org/2002/07/owl#"
     xmlns:rdf="http://www.w3.org/1999/02/22-rdf-syntax-ns#"
     xmlns:xml="http://www.w3.org/XML/1998/namespace"
     xmlns:xsd="http://www.w3.org/2001/XMLSchema#"
     xmlns:rdfs="http://www.w3.org/2000/01/rdf-schema#"
     xmlns:skos="http://www.w3.org/2004/02/skos/core#"
     xmlns:oboInOwl="http://www.geneontology.org/formats/oboInOwl#">
    <owl:Ontology rdf:about="http://purl.obolibrary.org/BCODMO_SM/matrix/material.owl">
        <owl:versionIRI rdf:resource="http://purl.obolibrary.org/BCODMO_SM/matrix/material.owl"/>
    </owl:Ontology>
    


    <!-- 
    ///////////////////////////////////////////////////////////////////////////////////////
    //
    // Annotation properties
    //
    ///////////////////////////////////////////////////////////////////////////////////////
     -->

    


    <!-- http://purl.obolibrary.org/obo/IAO_0000111 -->

    <owl:AnnotationProperty rdf:about="http://purl.obolibrary.org/obo/IAO_0000111"/>
    


    <!-- http://purl.obolibrary.org/obo/IAO_0000115 -->

    <owl:AnnotationProperty rdf:about="http://purl.obolibrary.org/obo/IAO_0000115"/>
    


    <!-- http://purl.obolibrary.org/obo/IAO_0000116 -->

    <owl:AnnotationProperty rdf:about="http://purl.obolibrary.org/obo/IAO_0000116"/>
    


    <!-- http://purl.obolibrary.org/obo/IAO_0000117 -->

    <owl:AnnotationProperty rdf:about="http://purl.obolibrary.org/obo/IAO_0000117"/>
    


    <!-- http://purl.org/dc/elements/1.1/creator -->

    <owl:AnnotationProperty rdf:about="http://purl.org/dc/elements/1.1/creator"/>
    


    <!-- http://purl.org/dc/elements/1.1/date -->

    <owl:AnnotationProperty rdf:about="http://purl.org/dc/elements/1.1/date"/>
    


    <!-- http://www.geneontology.org/formats/oboInOwl#created_by -->

    <owl:AnnotationProperty rdf:about="http://www.geneontology.org/formats/oboInOwl#created_by"/>
    


    <!-- http://www.geneontology.org/formats/oboInOwl#creation_date -->

    <owl:AnnotationProperty rdf:about="http://www.geneontology.org/formats/oboInOwl#creation_date"/>
    


    <!-- http://www.geneontology.org/formats/oboInOwl#hasBroadSynonym -->

    <owl:AnnotationProperty rdf:about="http://www.geneontology.org/formats/oboInOwl#hasBroadSynonym"/>
    


    <!-- http://www.geneontology.org/formats/oboInOwl#hasDbXref -->

    <owl:AnnotationProperty rdf:about="http://www.geneontology.org/formats/oboInOwl#hasDbXref"/>
    


    <!-- http://www.geneontology.org/formats/oboInOwl#hasExactSynonym -->

    <owl:AnnotationProperty rdf:about="http://www.geneontology.org/formats/oboInOwl#hasExactSynonym"/>
    


    <!-- http://www.geneontology.org/formats/oboInOwl#hasNarrowSynonym -->

    <owl:AnnotationProperty rdf:about="http://www.geneontology.org/formats/oboInOwl#hasNarrowSynonym"/>
    


    <!-- http://www.geneontology.org/formats/oboInOwl#hasOBONamespace -->

    <owl:AnnotationProperty rdf:about="http://www.geneontology.org/formats/oboInOwl#hasOBONamespace"/>
    


    <!-- http://www.geneontology.org/formats/oboInOwl#hasRelatedSynonym -->

    <owl:AnnotationProperty rdf:about="http://www.geneontology.org/formats/oboInOwl#hasRelatedSynonym"/>
    


    <!-- http://www.geneontology.org/formats/oboInOwl#id -->

    <owl:AnnotationProperty rdf:about="http://www.geneontology.org/formats/oboInOwl#id"/>
    


    <!-- http://www.geneontology.org/formats/oboInOwl#inSubset -->

    <owl:AnnotationProperty rdf:about="http://www.geneontology.org/formats/oboInOwl#inSubset"/>
    


    <!-- http://www.w3.org/2004/02/skos/core#exactMatch -->

    <owl:AnnotationProperty rdf:about="http://www.w3.org/2004/02/skos/core#exactMatch"/>
    


    <!-- 
    ///////////////////////////////////////////////////////////////////////////////////////
    //
    // Classes
    //
    ///////////////////////////////////////////////////////////////////////////////////////
     -->

    


    <!-- http://purl.obolibrary.org/obo/BSM_0100001 -->

    <owl:Class rdf:about="http://purl.obolibrary.org/obo/BSM_0100001">
        <rdfs:subClassOf rdf:resource="http://purl.obolibrary.org/obo/ENVO_01000155"/>
        <obo:IAO_0000111 xml:lang="en">seagrass</obo:IAO_0000111>
        <oboInOwl:inSubset rdf:resource="http://bcodmo/sm#material"/>
        <oboInOwl:inSubset rdf:resource="http://bcodmo/sm#matrix"/>
        <rdfs:label xml:lang="en">seagrass</rdfs:label>
    </owl:Class>
    


    <!-- http://purl.obolibrary.org/obo/BSM_0100002 -->

    <owl:Class rdf:about="http://purl.obolibrary.org/obo/BSM_0100002">
        <obo:IAO_0000111 xml:lang="en">radioactive material</obo:IAO_0000111>
        <oboInOwl:inSubset rdf:resource="http://bcodmo/sm#material"/>
        <oboInOwl:inSubset rdf:resource="http://bcodmo/sm#matrix"/>
        <rdfs:label xml:lang="en">radioactive material</rdfs:label>
        <skos:exactMatch rdf:resource="http://purl.obolibrary.org/obo/ENVO_03510037"/>
    </owl:Class>
    


    <!-- http://purl.obolibrary.org/obo/BSM_0100003 -->

    <owl:Class rdf:about="http://purl.obolibrary.org/obo/BSM_0100003">
        <obo:IAO_0000111 xml:lang="en">resin</obo:IAO_0000111>
        <oboInOwl:inSubset rdf:resource="http://bcodmo/sm#material"/>
        <oboInOwl:inSubset rdf:resource="http://bcodmo/sm#matrix"/>
        <rdfs:label xml:lang="en">resin</rdfs:label>
        <skos:exactMatch rdf:resource="http://purl.obolibrary.org/obo/ENVO_03510018"/>
    </owl:Class>
    


    <!-- http://purl.obolibrary.org/obo/BSM_0100004 -->

    <owl:Class rdf:about="http://purl.obolibrary.org/obo/BSM_0100004">
        <obo:IAO_0000111 xml:lang="en">incubation</obo:IAO_0000111>
        <oboInOwl:inSubset rdf:resource="http://bcodmo/sm#material"/>
        <oboInOwl:inSubset rdf:resource="http://bcodmo/sm#matrix"/>
        <rdfs:label xml:lang="en">incubation</rdfs:label>
    </owl:Class>
    


    <!-- http://purl.obolibrary.org/obo/ENVO_00000134 -->

    <owl:Class rdf:about="http://purl.obolibrary.org/obo/ENVO_00000134">
        <obo:IAO_0000111 xml:lang="en">permafrost</obo:IAO_0000111>
        <obo:IAO_0000115>Soil or rock and included ice or organic material at or below the freezing point of water (0 degrees Celsius or 32 degrees Fahrenheit) for two or more years.</obo:IAO_0000115>
        <oboInOwl:hasDbXref rdf:resource="http://sweetontology.net/realmSoil/Permafrost"/>
        <oboInOwl:hasDbXref>EcoLexicon:permafrost</oboInOwl:hasDbXref>
        <oboInOwl:hasDbXref>LTER:408</oboInOwl:hasDbXref>
        <oboInOwl:hasDbXref rdf:datatype="http://www.w3.org/2001/XMLSchema#string">https://en.wikipedia.org/wiki/Permafrost</oboInOwl:hasDbXref>
        <oboInOwl:hasExactSynonym>Permafrost</oboInOwl:hasExactSynonym>
        <oboInOwl:inSubset rdf:resource="http://bcodmo/sm#material"/>
        <oboInOwl:inSubset rdf:resource="http://bcodmo/sm#matrix"/>
        <oboInOwl:inSubset>envoPolar</oboInOwl:inSubset>
        <rdfs:comment>Ice is not always present, as may be in the case of nonporous bedrock, but it frequently occurs and it may be in amounts exceeding the potential hydraulic saturation of the ground material.</rdfs:comment>
        <rdfs:label>permafrost</rdfs:label>
        <rdfs:label xml:lang="en">permafrost</rdfs:label>
    </owl:Class>
    <owl:Axiom>
        <owl:annotatedSource rdf:resource="http://purl.obolibrary.org/obo/ENVO_00000134"/>
        <owl:annotatedProperty rdf:resource="http://purl.obolibrary.org/obo/IAO_0000115"/>
        <owl:annotatedTarget>Soil or rock and included ice or organic material at or below the freezing point of water (0 degrees Celsius or 32 degrees Fahrenheit) for two or more years.</owl:annotatedTarget>
        <oboInOwl:hasDbXref rdf:resource="https://orcid.org/0000-0003-4808-4736"/>
        <oboInOwl:hasDbXref rdf:datatype="http://www.w3.org/2001/XMLSchema#string">https://en.wikipedia.org/wiki/Permafrost</oboInOwl:hasDbXref>
    </owl:Axiom>
    <owl:Axiom>
        <owl:annotatedSource rdf:resource="http://purl.obolibrary.org/obo/ENVO_00000134"/>
        <owl:annotatedProperty rdf:resource="http://www.geneontology.org/formats/oboInOwl#hasExactSynonym"/>
        <owl:annotatedTarget>Permafrost</owl:annotatedTarget>
        <oboInOwl:hasDbXref rdf:datatype="http://www.w3.org/2001/XMLSchema#string">NASA:earthrealm</oboInOwl:hasDbXref>
    </owl:Axiom>
    


    <!-- http://purl.obolibrary.org/obo/ENVO_00000546 -->

    <owl:Class rdf:about="http://purl.obolibrary.org/obo/ENVO_00000546">
        <rdfs:subClassOf rdf:resource="http://purl.obolibrary.org/obo/ENVO_00002007"/>
        <obo:IAO_0000111 xml:lang="en">lake sediment</obo:IAO_0000111>
        <obo:IAO_0000115>Lake sediment is sediment which covers the bottom of a lake. Lake sediments are comprised mainly of clastic material (sediment of clay, silt, and sand sizes), organic debris, chemical precipitates, or combinations of these.</obo:IAO_0000115>
        <oboInOwl:hasRelatedSynonym>SedimentLayer</oboInOwl:hasRelatedSynonym>
        <oboInOwl:inSubset rdf:resource="http://bcodmo/sm#material"/>
        <oboInOwl:inSubset rdf:resource="http://bcodmo/sm#matrix"/>
        <rdfs:label>lake sediment</rdfs:label>
        <rdfs:label xml:lang="en">lake sediment</rdfs:label>
    </owl:Class>
    <owl:Axiom>
        <owl:annotatedSource rdf:resource="http://purl.obolibrary.org/obo/ENVO_00000546"/>
        <owl:annotatedProperty rdf:resource="http://purl.obolibrary.org/obo/IAO_0000115"/>
        <owl:annotatedTarget>Lake sediment is sediment which covers the bottom of a lake. Lake sediments are comprised mainly of clastic material (sediment of clay, silt, and sand sizes), organic debris, chemical precipitates, or combinations of these.</owl:annotatedTarget>
        <oboInOwl:hasDbXref>URL:http://www.britannica.com/EBchecked/topic/328083/lake/59070/Sediments-and-sedimentation</oboInOwl:hasDbXref>
    </owl:Axiom>
    <owl:Axiom>
        <owl:annotatedSource rdf:resource="http://purl.obolibrary.org/obo/ENVO_00000546"/>
        <owl:annotatedProperty rdf:resource="http://www.geneontology.org/formats/oboInOwl#hasRelatedSynonym"/>
        <owl:annotatedTarget>SedimentLayer</owl:annotatedTarget>
        <oboInOwl:hasDbXref rdf:datatype="http://www.w3.org/2001/XMLSchema#string">NASA:earthrealm</oboInOwl:hasDbXref>
    </owl:Axiom>
    


    <!-- http://purl.obolibrary.org/obo/ENVO_00001995 -->

    <owl:Class rdf:about="http://purl.obolibrary.org/obo/ENVO_00001995">
        <obo:IAO_0000111 xml:lang="en">rock</obo:IAO_0000111>
        <obo:IAO_0000115>A rock is a naturally occurring solid aggregate of one or more minerals or mineraloids.</obo:IAO_0000115>
        <oboInOwl:hasDbXref>EcoLexicon:rock</oboInOwl:hasDbXref>
        <oboInOwl:hasDbXref>FTT:1010</oboInOwl:hasDbXref>
        <oboInOwl:hasDbXref>FTT:145</oboInOwl:hasDbXref>
        <oboInOwl:hasDbXref>Geonames:T.RK</oboInOwl:hasDbXref>
        <oboInOwl:hasDbXref>Geonames:T.RKS</oboInOwl:hasDbXref>
        <oboInOwl:hasDbXref>SWEETRealm:Rock</oboInOwl:hasDbXref>
        <oboInOwl:hasDbXref>TGN:21444</oboInOwl:hasDbXref>
        <oboInOwl:hasDbXref>https://en.wikipedia.org/wiki/Rock</oboInOwl:hasDbXref>
        <oboInOwl:inSubset rdf:resource="http://bcodmo/sm#material"/>
        <oboInOwl:inSubset rdf:resource="http://bcodmo/sm#matrix"/>
        <rdfs:comment>From https://en.wikipedia.org/wiki/ [A mineral] is different from a rock, which can be an aggregate of minerals or non-minerals and does not have a specific chemical composition. The exact definition of a mineral is under debate, especially with respect to the requirement a valid species be abiogenic, and to a lesser extent with regards to it having an ordered atomic structure.</rdfs:comment>
        <rdfs:label>rock</rdfs:label>
        <rdfs:label xml:lang="en">rock</rdfs:label>
    </owl:Class>
    <owl:Axiom>
        <owl:annotatedSource rdf:resource="http://purl.obolibrary.org/obo/ENVO_00001995"/>
        <owl:annotatedProperty rdf:resource="http://purl.obolibrary.org/obo/IAO_0000115"/>
        <owl:annotatedTarget>A rock is a naturally occurring solid aggregate of one or more minerals or mineraloids.</owl:annotatedTarget>
        <oboInOwl:hasDbXref rdf:datatype="http://www.w3.org/2001/XMLSchema#string">MA:ma</oboInOwl:hasDbXref>
        <oboInOwl:hasDbXref>https://en.wikipedia.org/wiki/Rock_(geology)</oboInOwl:hasDbXref>
    </owl:Axiom>
    


    <!-- http://purl.obolibrary.org/obo/ENVO_00001998 -->

    <owl:Class rdf:about="http://purl.obolibrary.org/obo/ENVO_00001998">
        <obo:IAO_0000111 xml:lang="en">soil</obo:IAO_0000111>
        <obo:IAO_0000115>Soil is an environmental material which is primarily composed of minerals, varying proportions of sand, silt, and clay, organic material such as humus, gases, liquids, and a broad range of resident micro- and macroorganisms.</obo:IAO_0000115>
        <obo:IAO_0000116>The various &apos;has part&apos; and &apos;has quality&apos; relations may not hold true for all soils; however, I have yet to find counter examples. Require input from a pedologist or similar. [pbuttigieg]</obo:IAO_0000116>
        <oboInOwl:hasBroadSynonym>regolith</oboInOwl:hasBroadSynonym>
        <oboInOwl:hasDbXref>LTER:535</oboInOwl:hasDbXref>
        <oboInOwl:hasDbXref>SPIRE:Soil</oboInOwl:hasDbXref>
        <oboInOwl:hasDbXref>SWEETRealm:Soil</oboInOwl:hasDbXref>
        <oboInOwl:hasDbXref rdf:datatype="http://www.w3.org/2001/XMLSchema#string">https://en.wikipedia.org/wiki/Soil</oboInOwl:hasDbXref>
        <oboInOwl:inSubset rdf:resource="http://bcodmo/sm#material"/>
        <oboInOwl:inSubset rdf:resource="http://bcodmo/sm#matrix"/>
        <oboInOwl:inSubset rdf:resource="http://purl.obolibrary.org/obo/envo#EnvO-Lite-GSC"/>
        <rdfs:comment>&apos;In engineering terms, soil is referred to as regolith, or loose rock material that lies above the &apos;solid geology&apos;. Soil is commonly referred to as &quot;earth&quot; or &quot;dirt&quot;; technically, the term &quot;dirt&quot; should be restricted to displaced soil.&apos; https://en.wikipedia.org/wiki/Soil

&quot; The upper limit of soil is the boundary between soil and air, shallow water, live plants, or plant materials that have not begun to decompose. Areas are not considered to have soil if the surface is permanently covered by water too deep (typically more than 2.5 meters) for the growth of rooted plants.

The lower boundary that separates soil from the nonsoil underneath is most difficult to define. Soil consists of horizons near the Earth&apos;s surface that, in contrast to the underlying parent material, have been altered by the interactions of climate, relief, and living organisms over time. Commonly, soil grades at its lower boundary to hard rock or to earthy materials virtually devoid of animals, roots, or other marks of biological activity. For purposes of classification, the lower boundary of soil is arbitrarily set at 200 cm.&quot;  Soil taxonomy, 2nd Ed., quoted in http://www.nrcs.usda.gov/wps/portal/nrcs/detail/soils/edu/?cid=nrcs142p2_054280</rdfs:comment>
        <rdfs:label>soil</rdfs:label>
        <rdfs:label xml:lang="en">soil</rdfs:label>
    </owl:Class>
    <owl:Axiom>
        <owl:annotatedSource rdf:resource="http://purl.obolibrary.org/obo/ENVO_00001998"/>
        <owl:annotatedProperty rdf:resource="http://purl.obolibrary.org/obo/IAO_0000115"/>
        <owl:annotatedTarget>Soil is an environmental material which is primarily composed of minerals, varying proportions of sand, silt, and clay, organic material such as humus, gases, liquids, and a broad range of resident micro- and macroorganisms.</owl:annotatedTarget>
        <oboInOwl:hasDbXref rdf:datatype="http://www.w3.org/2001/XMLSchema#string">https://en.wikipedia.org/wiki/Soil</oboInOwl:hasDbXref>
    </owl:Axiom>
    


    <!-- http://purl.obolibrary.org/obo/ENVO_00002001 -->

    <owl:Class rdf:about="http://purl.obolibrary.org/obo/ENVO_00002001">
        <rdfs:subClassOf rdf:resource="http://purl.obolibrary.org/obo/ENVO_00002006"/>
        <rdfs:subClassOf rdf:resource="http://purl.obolibrary.org/obo/ENVO_00002264"/>
        <obo:IAO_0000111 xml:lang="en">waste water</obo:IAO_0000111>
        <obo:IAO_0000115>Water that has been adversely affected in quality by anthropogenic influence.</obo:IAO_0000115>
        <oboInOwl:hasDbXref>EcoLexicon:waste_water</oboInOwl:hasDbXref>
        <oboInOwl:hasDbXref>SWEETRealm:Wastewater</oboInOwl:hasDbXref>
        <oboInOwl:hasDbXref>https://en.wikipedia.org/wiki/Waste_water</oboInOwl:hasDbXref>
        <oboInOwl:hasOBONamespace>ENVO</oboInOwl:hasOBONamespace>
        <oboInOwl:id>ENVO:00002001</oboInOwl:id>
        <oboInOwl:inSubset rdf:resource="http://bcodmo/sm#material"/>
        <oboInOwl:inSubset rdf:resource="http://bcodmo/sm#matrix"/>
        <oboInOwl:inSubset rdf:resource="http://purl.obolibrary.org/obo/envo#EnvO-Lite-GSC"/>
        <rdfs:label>waste water</rdfs:label>
        <rdfs:label xml:lang="en">waste water</rdfs:label>
    </owl:Class>
    <owl:Axiom>
        <owl:annotatedSource rdf:resource="http://purl.obolibrary.org/obo/ENVO_00002001"/>
        <owl:annotatedProperty rdf:resource="http://purl.obolibrary.org/obo/IAO_0000115"/>
        <owl:annotatedTarget>Water that has been adversely affected in quality by anthropogenic influence.</owl:annotatedTarget>
        <oboInOwl:hasDbXref rdf:datatype="http://www.w3.org/2001/XMLSchema#string">https://en.wikipedia.org/wiki/Wastewater</oboInOwl:hasDbXref>
    </owl:Axiom>
    


    <!-- http://purl.obolibrary.org/obo/ENVO_00002005 -->

    <owl:Class rdf:about="http://purl.obolibrary.org/obo/ENVO_00002005">
        <rdfs:subClassOf rdf:resource="http://purl.obolibrary.org/obo/ENVO_01000797"/>
        <obo:IAO_0000111 xml:lang="en">air</obo:IAO_0000111>
        <obo:IAO_0000115>The mixture of gases (roughly (by molar content/volume: 78% nitrogen, 20.95% oxygen, 0.93% argon, 0.038% carbon dioxide, trace amounts of other gases, and a variable amount (average around 1%) of water vapor) that surrounds the planet Earth.</obo:IAO_0000115>
        <oboInOwl:hasDbXref>EcoLexicon:air</oboInOwl:hasDbXref>
        <oboInOwl:hasDbXref>LTER:18</oboInOwl:hasDbXref>
        <oboInOwl:hasDbXref>SWEETRealm:Air</oboInOwl:hasDbXref>
        <oboInOwl:hasDbXref rdf:datatype="http://www.w3.org/2001/XMLSchema#string">https://en.wikipedia.org/wiki/Air</oboInOwl:hasDbXref>
        <oboInOwl:inSubset rdf:resource="http://bcodmo/sm#material"/>
        <oboInOwl:inSubset rdf:resource="http://bcodmo/sm#matrix"/>
        <oboInOwl:inSubset rdf:resource="http://purl.obolibrary.org/obo/envo#EnvO-Lite-GSC"/>
        <oboInOwl:inSubset>envoPolar</oboInOwl:inSubset>
        <rdfs:label>air</rdfs:label>
        <rdfs:label xml:lang="en">air</rdfs:label>
    </owl:Class>
    <owl:Axiom>
        <owl:annotatedSource rdf:resource="http://purl.obolibrary.org/obo/ENVO_00002005"/>
        <owl:annotatedProperty rdf:resource="http://purl.obolibrary.org/obo/IAO_0000115"/>
        <owl:annotatedTarget>The mixture of gases (roughly (by molar content/volume: 78% nitrogen, 20.95% oxygen, 0.93% argon, 0.038% carbon dioxide, trace amounts of other gases, and a variable amount (average around 1%) of water vapor) that surrounds the planet Earth.</owl:annotatedTarget>
        <oboInOwl:hasDbXref rdf:datatype="http://www.w3.org/2001/XMLSchema#string">https://en.wikipedia.org/wiki/Air</oboInOwl:hasDbXref>
    </owl:Axiom>
    


    <!-- http://purl.obolibrary.org/obo/ENVO_00002006 -->

    <owl:Class rdf:about="http://purl.obolibrary.org/obo/ENVO_00002006">
        <obo:IAO_0000111 xml:lang="en">water</obo:IAO_0000111>
        <obo:IAO_0000115>An environmental material primarily composed of dihydrogen oxide in its liquid form.</obo:IAO_0000115>
        <oboInOwl:hasBroadSynonym>water</oboInOwl:hasBroadSynonym>
        <oboInOwl:hasDbXref>EcoLexicon:water</oboInOwl:hasDbXref>
        <oboInOwl:hasDbXref>LTER:617</oboInOwl:hasDbXref>
        <oboInOwl:hasDbXref>https://en.wikipedia.org/wiki/Water</oboInOwl:hasDbXref>
        <oboInOwl:inSubset rdf:resource="http://bcodmo/sm#material"/>
        <oboInOwl:inSubset rdf:resource="http://bcodmo/sm#matrix"/>
        <rdfs:label>liquid water</rdfs:label>
        <rdfs:label xml:lang="en">water</rdfs:label>
    </owl:Class>
    <owl:Axiom>
        <owl:annotatedSource rdf:resource="http://purl.obolibrary.org/obo/ENVO_00002006"/>
        <owl:annotatedProperty rdf:resource="http://purl.obolibrary.org/obo/IAO_0000115"/>
        <owl:annotatedTarget>An environmental material primarily composed of dihydrogen oxide in its liquid form.</owl:annotatedTarget>
        <oboInOwl:hasDbXref rdf:datatype="http://www.w3.org/2001/XMLSchema#string">MA:ma</oboInOwl:hasDbXref>
    </owl:Axiom>
    


    <!-- http://purl.obolibrary.org/obo/ENVO_00002007 -->

    <owl:Class rdf:about="http://purl.obolibrary.org/obo/ENVO_00002007">
        <obo:IAO_0000111 xml:lang="en">sediment</obo:IAO_0000111>
        <obo:IAO_0000115>Sediment is an environmental substance comprised of any particulate matter that can be transported by fluid flow and which eventually is deposited as a layer of solid particles on the bedor bottom of a body of water or other liquid.</obo:IAO_0000115>
        <oboInOwl:hasDbXref>EcoLexicon:sediment</oboInOwl:hasDbXref>
        <oboInOwl:hasDbXref>EcoLexicon:sedimentation</oboInOwl:hasDbXref>
        <oboInOwl:hasDbXref>LTER:492</oboInOwl:hasDbXref>
        <oboInOwl:hasDbXref>LTER:493</oboInOwl:hasDbXref>
        <oboInOwl:hasDbXref>SWEETRealm:Sediment</oboInOwl:hasDbXref>
        <oboInOwl:hasDbXref rdf:datatype="http://www.w3.org/2001/XMLSchema#string">https://en.wikipedia.org/wiki/Sediment</oboInOwl:hasDbXref>
        <oboInOwl:inSubset rdf:resource="http://bcodmo/sm#material"/>
        <oboInOwl:inSubset rdf:resource="http://bcodmo/sm#matrix"/>
        <oboInOwl:inSubset rdf:resource="http://purl.obolibrary.org/obo/envo#EnvO-Lite-GSC"/>
        <oboInOwl:inSubset>envoPolar</oboInOwl:inSubset>
        <rdfs:comment>It is recommended to use a combination of sediment terms to describe a more specific sediment type.</rdfs:comment>
        <rdfs:label>sediment</rdfs:label>
        <rdfs:label xml:lang="en">sediment</rdfs:label>
    </owl:Class>
    <owl:Axiom>
        <owl:annotatedSource rdf:resource="http://purl.obolibrary.org/obo/ENVO_00002007"/>
        <owl:annotatedProperty rdf:resource="http://purl.obolibrary.org/obo/IAO_0000115"/>
        <owl:annotatedTarget>Sediment is an environmental substance comprised of any particulate matter that can be transported by fluid flow and which eventually is deposited as a layer of solid particles on the bedor bottom of a body of water or other liquid.</owl:annotatedTarget>
        <oboInOwl:hasDbXref rdf:datatype="http://www.w3.org/2001/XMLSchema#string">https://en.wikipedia.org/wiki/Sediment</oboInOwl:hasDbXref>
    </owl:Axiom>
    


    <!-- http://purl.obolibrary.org/obo/ENVO_00002008 -->

    <owl:Class rdf:about="http://purl.obolibrary.org/obo/ENVO_00002008">
        <rdfs:subClassOf rdf:resource="http://purl.obolibrary.org/obo/ENVO_01000060"/>
        <obo:IAO_0000111 xml:lang="en">dust</obo:IAO_0000111>
        <obo:IAO_0000115>Minute solid particles with diameters less than 500 micrometers. Occurs in and may be deposited from, the atmosphere.</obo:IAO_0000115>
        <oboInOwl:hasDbXref>EcoLexicon:dust</oboInOwl:hasDbXref>
        <oboInOwl:hasDbXref>SWEETRealm:Dust</oboInOwl:hasDbXref>
        <oboInOwl:hasDbXref rdf:datatype="http://www.w3.org/2001/XMLSchema#string">https://en.wikipedia.org/wiki/Dust</oboInOwl:hasDbXref>
        <oboInOwl:inSubset rdf:resource="http://bcodmo/sm#material"/>
        <oboInOwl:inSubset rdf:resource="http://bcodmo/sm#matrix"/>
        <oboInOwl:inSubset>envoPolar</oboInOwl:inSubset>
        <rdfs:label>dust</rdfs:label>
        <rdfs:label xml:lang="en">dust</rdfs:label>
    </owl:Class>
    <owl:Axiom>
        <owl:annotatedSource rdf:resource="http://purl.obolibrary.org/obo/ENVO_00002008"/>
        <owl:annotatedProperty rdf:resource="http://purl.obolibrary.org/obo/IAO_0000115"/>
        <owl:annotatedTarget>Minute solid particles with diameters less than 500 micrometers. Occurs in and may be deposited from, the atmosphere.</owl:annotatedTarget>
        <oboInOwl:hasDbXref rdf:datatype="http://www.w3.org/2001/XMLSchema#string">https://en.wikipedia.org/wiki/Dust</oboInOwl:hasDbXref>
    </owl:Axiom>
    


    <!-- http://purl.obolibrary.org/obo/ENVO_00002011 -->

    <owl:Class rdf:about="http://purl.obolibrary.org/obo/ENVO_00002011">
        <rdfs:subClassOf rdf:resource="http://purl.obolibrary.org/obo/ENVO_00002006"/>
        <obo:IAO_0000111 xml:lang="en">fresh water</obo:IAO_0000111>
        <obo:IAO_0000115>Water which has a low concentration of dissolved solutes, particularly that of sodium chloride.</obo:IAO_0000115>
        <oboInOwl:hasDbXref>EcoLexicon:fresh_water</oboInOwl:hasDbXref>
        <oboInOwl:hasDbXref>LTER:216</oboInOwl:hasDbXref>
        <oboInOwl:hasDbXref>SWEETRealm:FreshWater</oboInOwl:hasDbXref>
        <oboInOwl:hasDbXref>https://en.wikipedia.org/wiki/Fresh_water</oboInOwl:hasDbXref>
        <oboInOwl:hasExactSynonym>freshwater</oboInOwl:hasExactSynonym>
        <oboInOwl:hasRelatedSynonym>sweet water</oboInOwl:hasRelatedSynonym>
        <oboInOwl:inSubset rdf:resource="http://bcodmo/sm#material"/>
        <oboInOwl:inSubset rdf:resource="http://bcodmo/sm#matrix"/>
        <oboInOwl:inSubset>envoEmpo</oboInOwl:inSubset>
        <oboInOwl:inSubset>envoPolar</oboInOwl:inSubset>
        <rdfs:comment>The lower bound of solute concentration required for water to be considered freshwater is variable, but is always less than that of seawater, and often cited as less than 1 gram of solutes per 1 litre of water.</rdfs:comment>
        <rdfs:label>fresh water</rdfs:label>
        <rdfs:label xml:lang="en">fresh water</rdfs:label>
    </owl:Class>
    


    <!-- http://purl.obolibrary.org/obo/ENVO_00002012 -->

    <owl:Class rdf:about="http://purl.obolibrary.org/obo/ENVO_00002012">
        <rdfs:subClassOf rdf:resource="http://purl.obolibrary.org/obo/ENVO_00002006"/>
        <obo:IAO_0000111 xml:lang="en">hypersaline water</obo:IAO_0000111>
        <obo:IAO_0000115>Water which contains a highly increased concentration of dissolved salts, surpassing the average salinity of seawater.</obo:IAO_0000115>
        <obo:IAO_0000116>We make no commitment to a particular threshold; this should be described on the data/information layer according to the norms of a discipline, accepted standard, or similar reference.</obo:IAO_0000116>
        <oboInOwl:inSubset rdf:resource="http://bcodmo/sm#material"/>
        <oboInOwl:inSubset rdf:resource="http://bcodmo/sm#matrix"/>
        <oboInOwl:inSubset>envoPolar</oboInOwl:inSubset>
        <rdfs:comment>The average salinity of sea water is assumed to be around 35,000 ppm, equivalent to 35 grams of salt per one liter (or kilogram) of water.</rdfs:comment>
        <rdfs:label>hypersaline water</rdfs:label>
        <rdfs:label xml:lang="en">hypersaline water</rdfs:label>
    </owl:Class>
    


    <!-- http://purl.obolibrary.org/obo/ENVO_00002016 -->

    <owl:Class rdf:about="http://purl.obolibrary.org/obo/ENVO_00002016">
        <rdfs:subClassOf rdf:resource="http://purl.obolibrary.org/obo/ENVO_00001995"/>
        <obo:IAO_0000111 xml:lang="en">sedimentary rock</obo:IAO_0000111>
        <obo:IAO_0000115>A rock formed by deposition of either clastic sediments, organic matter, or chemical precipitates (evaporites), followed by compaction of the particulate matter and cementation during diagenesis.</obo:IAO_0000115>
        <oboInOwl:hasDbXref>EcoLexicon:sedimentary_rock</oboInOwl:hasDbXref>
        <oboInOwl:hasDbXref>SWEETRealm:SedimentaryRock</oboInOwl:hasDbXref>
        <oboInOwl:hasDbXref>https://en.wikipedia.org/wiki/Sedimentary_rock</oboInOwl:hasDbXref>
        <oboInOwl:hasOBONamespace>ENVO</oboInOwl:hasOBONamespace>
        <oboInOwl:id>ENVO:00002016</oboInOwl:id>
        <oboInOwl:inSubset rdf:resource="http://bcodmo/sm#material"/>
        <oboInOwl:inSubset rdf:resource="http://bcodmo/sm#matrix"/>
        <rdfs:label>sedimentary rock</rdfs:label>
        <rdfs:label xml:lang="en">sedimentary rock</rdfs:label>
    </owl:Class>
    <owl:Axiom>
        <owl:annotatedSource rdf:resource="http://purl.obolibrary.org/obo/ENVO_00002016"/>
        <owl:annotatedProperty rdf:resource="http://purl.obolibrary.org/obo/IAO_0000115"/>
        <owl:annotatedTarget>A rock formed by deposition of either clastic sediments, organic matter, or chemical precipitates (evaporites), followed by compaction of the particulate matter and cementation during diagenesis.</owl:annotatedTarget>
        <oboInOwl:hasDbXref rdf:datatype="http://www.w3.org/2001/XMLSchema#string">https://en.wikipedia.org/wiki/Rock_%28geology%29</oboInOwl:hasDbXref>
    </owl:Axiom>
    


    <!-- http://purl.obolibrary.org/obo/ENVO_00002018 -->

    <owl:Class rdf:about="http://purl.obolibrary.org/obo/ENVO_00002018">
        <rdfs:subClassOf rdf:resource="http://purl.obolibrary.org/obo/ENVO_00002001"/>
        <rdfs:subClassOf rdf:resource="http://purl.obolibrary.org/obo/ENVO_00002264"/>
        <obo:IAO_0000111 xml:lang="en">sewage</obo:IAO_0000111>
        <obo:IAO_0000115>Wastewater that is contaminated with feces or urine,</obo:IAO_0000115>
        <oboInOwl:hasDbXref>SWEETRealm:Sewage</oboInOwl:hasDbXref>
        <oboInOwl:hasDbXref>https://en.wikipedia.org/wiki/Sewage</oboInOwl:hasDbXref>
        <oboInOwl:hasOBONamespace>ENVO</oboInOwl:hasOBONamespace>
        <oboInOwl:id>ENVO:00002018</oboInOwl:id>
        <oboInOwl:inSubset rdf:resource="http://bcodmo/sm#material"/>
        <oboInOwl:inSubset rdf:resource="http://bcodmo/sm#matrix"/>
        <rdfs:label>sewage</rdfs:label>
        <rdfs:label xml:lang="en">sewage</rdfs:label>
    </owl:Class>
    <owl:Axiom>
        <owl:annotatedSource rdf:resource="http://purl.obolibrary.org/obo/ENVO_00002018"/>
        <owl:annotatedProperty rdf:resource="http://purl.obolibrary.org/obo/IAO_0000115"/>
        <owl:annotatedTarget>Wastewater that is contaminated with feces or urine,</owl:annotatedTarget>
        <oboInOwl:hasDbXref rdf:datatype="http://www.w3.org/2001/XMLSchema#string">https://en.wikipedia.org/wiki/Wastewater</oboInOwl:hasDbXref>
    </owl:Axiom>
    


    <!-- http://purl.obolibrary.org/obo/ENVO_00002019 -->

    <owl:Class rdf:about="http://purl.obolibrary.org/obo/ENVO_00002019">
        <rdfs:subClassOf rdf:resource="http://purl.obolibrary.org/obo/ENVO_00002006"/>
        <obo:IAO_0000111 xml:lang="en">brackish water</obo:IAO_0000111>
        <obo:IAO_0000115>Water which has a higher salinity than fresh water but a lower salinity than marine water.</obo:IAO_0000115>
        <oboInOwl:hasDbXref>EcoLexicon:brackish_water</oboInOwl:hasDbXref>
        <oboInOwl:hasDbXref>LTER:702</oboInOwl:hasDbXref>
        <oboInOwl:hasDbXref>SPIRE:Brackish_water</oboInOwl:hasDbXref>
        <oboInOwl:hasDbXref>SWEETRealm:BrackishWater</oboInOwl:hasDbXref>
        <oboInOwl:hasDbXref>https://en.wikipedia.org/wiki/Brackish_water</oboInOwl:hasDbXref>
        <oboInOwl:inSubset rdf:resource="http://bcodmo/sm#material"/>
        <oboInOwl:inSubset rdf:resource="http://bcodmo/sm#matrix"/>
        <oboInOwl:inSubset>envoPolar</oboInOwl:inSubset>
        <rdfs:label>brackish water</rdfs:label>
        <rdfs:label xml:lang="en">brackish water</rdfs:label>
    </owl:Class>
    


    <!-- http://purl.obolibrary.org/obo/ENVO_00002040 -->

    <owl:Class rdf:about="http://purl.obolibrary.org/obo/ENVO_00002040">
        <obo:IAO_0000111 xml:lang="en">wood</obo:IAO_0000111>
        <oboInOwl:hasDbXref>EcoLexicon:wood</oboInOwl:hasDbXref>
        <oboInOwl:hasDbXref>LTER:637</oboInOwl:hasDbXref>
        <oboInOwl:hasDbXref>SWEETRealm:Wood</oboInOwl:hasDbXref>
        <oboInOwl:hasDbXref>https://en.wikipedia.org/wiki/Wood</oboInOwl:hasDbXref>
        <oboInOwl:hasOBONamespace>ENVO</oboInOwl:hasOBONamespace>
        <oboInOwl:id>ENVO:00002040</oboInOwl:id>
        <oboInOwl:inSubset rdf:resource="http://bcodmo/sm#material"/>
        <oboInOwl:inSubset rdf:resource="http://bcodmo/sm#matrix"/>
        <rdfs:label>wood</rdfs:label>
        <rdfs:label xml:lang="en">wood</rdfs:label>
    </owl:Class>
    


    <!-- http://purl.obolibrary.org/obo/ENVO_00002141 -->

    <owl:Class rdf:about="http://purl.obolibrary.org/obo/ENVO_00002141">
        <rdfs:subClassOf rdf:resource="http://purl.obolibrary.org/obo/ENVO_00002006"/>
        <obo:IAO_0000111 xml:lang="en">leachate</obo:IAO_0000111>
        <obo:IAO_0000115>The liquid produced when water percolates through any permeable material. It can contain either dissolved or suspended material, or usually both.</obo:IAO_0000115>
        <oboInOwl:hasDbXref>https://en.wikipedia.org/wiki/Leachate</oboInOwl:hasDbXref>
        <oboInOwl:hasOBONamespace>ENVO</oboInOwl:hasOBONamespace>
        <oboInOwl:id>ENVO:00002141</oboInOwl:id>
        <oboInOwl:inSubset rdf:resource="http://bcodmo/sm#material"/>
        <oboInOwl:inSubset rdf:resource="http://bcodmo/sm#matrix"/>
        <rdfs:label>leachate</rdfs:label>
        <rdfs:label xml:lang="en">leachate</rdfs:label>
    </owl:Class>
    <owl:Axiom>
        <owl:annotatedSource rdf:resource="http://purl.obolibrary.org/obo/ENVO_00002141"/>
        <owl:annotatedProperty rdf:resource="http://purl.obolibrary.org/obo/IAO_0000115"/>
        <owl:annotatedTarget>The liquid produced when water percolates through any permeable material. It can contain either dissolved or suspended material, or usually both.</owl:annotatedTarget>
        <oboInOwl:hasDbXref>https://en.wikipedia.org/wiki/Leachate</oboInOwl:hasDbXref>
    </owl:Axiom>
    


    <!-- http://purl.obolibrary.org/obo/ENVO_00002149 -->

    <owl:Class rdf:about="http://purl.obolibrary.org/obo/ENVO_00002149">
        <rdfs:subClassOf rdf:resource="http://purl.obolibrary.org/obo/ENVO_00002006"/>
        <obo:IAO_0000111 xml:lang="en">sea water</obo:IAO_0000111>
        <obo:IAO_0000115>Water which has physicochemical properties that have been determined by the processes occuring in a sea or ocean.</obo:IAO_0000115>
        <obo:IAO_0000116>When we have more classes representing the various processes which make seawater seawater, we can further axiomatise this class.</obo:IAO_0000116>
        <oboInOwl:hasDbXref>EcoLexicon:sea_water</oboInOwl:hasDbXref>
        <oboInOwl:hasDbXref>LTER:701</oboInOwl:hasDbXref>
        <oboInOwl:hasDbXref>SWEETRealm:SeaWater</oboInOwl:hasDbXref>
        <oboInOwl:hasDbXref>https://en.wikipedia.org/wiki/Sea_water</oboInOwl:hasDbXref>
        <oboInOwl:hasExactSynonym>ocean water</oboInOwl:hasExactSynonym>
        <oboInOwl:hasExactSynonym>seawater</oboInOwl:hasExactSynonym>
        <oboInOwl:inSubset rdf:resource="http://bcodmo/sm#material"/>
        <oboInOwl:inSubset rdf:resource="http://bcodmo/sm#matrix"/>
        <rdfs:comment>This definition refers to water that is actually in a sea or ocean. This water may have a wide range of salinity levels.</rdfs:comment>
        <rdfs:label>sea water</rdfs:label>
        <rdfs:label xml:lang="en">sea water</rdfs:label>
    </owl:Class>
    


    <!-- http://purl.obolibrary.org/obo/ENVO_00002150 -->

    <owl:Class rdf:about="http://purl.obolibrary.org/obo/ENVO_00002150">
        <rdfs:subClassOf rdf:resource="http://purl.obolibrary.org/obo/ENVO_00002149"/>
        <obo:IAO_0000111 xml:lang="en">coastal sea water</obo:IAO_0000111>
        <obo:IAO_0000115>Coastal sea water is sea water that is adjacent to a coast.</obo:IAO_0000115>
        <oboInOwl:hasBroadSynonym>coastal water</oboInOwl:hasBroadSynonym>
        <oboInOwl:hasExactSynonym>coastal ocean water</oboInOwl:hasExactSynonym>
        <oboInOwl:hasExactSynonym>coastal oceanic water</oboInOwl:hasExactSynonym>
        <oboInOwl:hasExactSynonym>coastal seawater</oboInOwl:hasExactSynonym>
        <oboInOwl:inSubset rdf:resource="http://bcodmo/sm#material"/>
        <oboInOwl:inSubset rdf:resource="http://bcodmo/sm#matrix"/>
        <oboInOwl:inSubset>envoPolar</oboInOwl:inSubset>
        <rdfs:comment>The limits of what qualifies as &quot;adjacent to&quot; vary greatly. This should be defined on a data level and is left intentionally fuzzy here. The label is &quot;coastal sea water&quot; rather than &quot;coastal water&quot; as some large lakes are often said to have coasts.</rdfs:comment>
        <rdfs:label>coastal sea water</rdfs:label>
        <rdfs:label xml:lang="en">coastal sea water</rdfs:label>
    </owl:Class>
    


    <!-- http://purl.obolibrary.org/obo/ENVO_00002164 -->

    <owl:Class rdf:about="http://purl.obolibrary.org/obo/ENVO_00002164">
        <obo:IAO_0000111 xml:lang="en">fossil</obo:IAO_0000111>
        <obo:IAO_0000115>A solid environmental material which is formed by the replacement of organic substances (including those in soils and sediments) with mineral material.</obo:IAO_0000115>
        <oboInOwl:hasDbXref>SWEETRealm:Fossil</oboInOwl:hasDbXref>
        <oboInOwl:hasDbXref>https://en.wikipedia.org/wiki/Fossil</oboInOwl:hasDbXref>
        <oboInOwl:inSubset rdf:resource="http://bcodmo/sm#material"/>
        <oboInOwl:inSubset rdf:resource="http://bcodmo/sm#matrix"/>
        <oboInOwl:inSubset rdf:resource="http://purl.obolibrary.org/obo/envo#EnvO-Lite-GSC"/>
        <rdfs:label xml:lang="en">fossil</rdfs:label>
        <rdfs:label>fossil material</rdfs:label>
    </owl:Class>
    <owl:Axiom>
        <owl:annotatedSource rdf:resource="http://purl.obolibrary.org/obo/ENVO_00002164"/>
        <owl:annotatedProperty rdf:resource="http://purl.obolibrary.org/obo/IAO_0000115"/>
        <owl:annotatedTarget>A solid environmental material which is formed by the replacement of organic substances (including those in soils and sediments) with mineral material.</owl:annotatedTarget>
        <oboInOwl:hasDbXref>https://en.wikipedia.org/wiki/Fossil</oboInOwl:hasDbXref>
    </owl:Axiom>
    


    <!-- http://purl.obolibrary.org/obo/ENVO_00002186 -->

    <owl:Class rdf:about="http://purl.obolibrary.org/obo/ENVO_00002186">
        <rdfs:subClassOf rdf:resource="http://purl.obolibrary.org/obo/ENVO_00002006"/>
        <obo:IAO_0000111 xml:lang="en">contaminated water</obo:IAO_0000111>
        <oboInOwl:hasDbXref>EcoLexicon:water_pollution</oboInOwl:hasDbXref>
        <oboInOwl:hasDbXref>https://en.wikipedia.org/wiki/Contaminated_water</oboInOwl:hasDbXref>
        <oboInOwl:hasExactSynonym>polluted water</oboInOwl:hasExactSynonym>
        <oboInOwl:hasOBONamespace>ENVO</oboInOwl:hasOBONamespace>
        <oboInOwl:id>ENVO:00002186</oboInOwl:id>
        <oboInOwl:inSubset rdf:resource="http://bcodmo/sm#material"/>
        <oboInOwl:inSubset rdf:resource="http://bcodmo/sm#matrix"/>
        <rdfs:label>contaminated water</rdfs:label>
        <rdfs:label xml:lang="en">contaminated water</rdfs:label>
    </owl:Class>
    


    <!-- http://purl.obolibrary.org/obo/ENVO_00002200 -->

    <owl:Class rdf:about="http://purl.obolibrary.org/obo/ENVO_00002200">
        <rdfs:subClassOf rdf:resource="http://purl.obolibrary.org/obo/ENVO_01000277"/>
        <obo:IAO_0000111 xml:lang="en">sea ice</obo:IAO_0000111>
        <obo:IAO_0000115>Water ice which has formed by the freezing of sea water.</obo:IAO_0000115>
        <obo:IAO_0000116>Parse comment from GCW and new subclases where appropriate.</obo:IAO_0000116>
        <oboInOwl:hasDbXref>http://sweetontology.net/realmCryo/SeaIce</oboInOwl:hasDbXref>
        <oboInOwl:hasDbXref>https://en.wikipedia.org/wiki/Sea_ice</oboInOwl:hasDbXref>
        <oboInOwl:inSubset rdf:resource="http://bcodmo/sm#material"/>
        <oboInOwl:inSubset rdf:resource="http://bcodmo/sm#matrix"/>
        <oboInOwl:inSubset>envoPolar</oboInOwl:inSubset>
        <rdfs:comment>In the United States, NOAA sea ice operations does not include superstructure icing as being sea ice. In sea ice operations however, sea ice is any form of ice found at sea which has originated from the freezing of sea water. It presents the main kind of floating ice encountered at sea. Except where it forms ridges, sea ice is up to a few metres thick, in which respect it differs from shelf ice.  Sea ice may be discontinuous pieces (ice floes) moved on the ocean surface by wind and currents (pack ice), or a motionless sheet attached to the coast (land-fast ice). In brief, it forms first as lolly ice (frazil crystals), thickens into sludge, and coagulates into sheet ice, pancake ice, or into floes of various shapes and sizes. Thereafter, sea ice may develop into pack ice and/or become a form of pressure ice.  Sea ice less than one year old is called first-year ice. Perennial ice is sea ice that survives at least one summer. It may be subdivided into second-year ice and multi-year ice, where multiyear ice has survived at least two summers.</rdfs:comment>
        <rdfs:label>sea ice</rdfs:label>
        <rdfs:label xml:lang="en">sea ice</rdfs:label>
    </owl:Class>
    <owl:Axiom>
        <owl:annotatedSource rdf:resource="http://purl.obolibrary.org/obo/ENVO_00002200"/>
        <owl:annotatedProperty rdf:resource="http://www.w3.org/2000/01/rdf-schema#comment"/>
        <owl:annotatedTarget>In the United States, NOAA sea ice operations does not include superstructure icing as being sea ice. In sea ice operations however, sea ice is any form of ice found at sea which has originated from the freezing of sea water. It presents the main kind of floating ice encountered at sea. Except where it forms ridges, sea ice is up to a few metres thick, in which respect it differs from shelf ice.  Sea ice may be discontinuous pieces (ice floes) moved on the ocean surface by wind and currents (pack ice), or a motionless sheet attached to the coast (land-fast ice). In brief, it forms first as lolly ice (frazil crystals), thickens into sludge, and coagulates into sheet ice, pancake ice, or into floes of various shapes and sizes. Thereafter, sea ice may develop into pack ice and/or become a form of pressure ice.  Sea ice less than one year old is called first-year ice. Perennial ice is sea ice that survives at least one summer. It may be subdivided into second-year ice and multi-year ice, where multiyear ice has survived at least two summers.</owl:annotatedTarget>
        <rdfs:comment>https://orcid.org/0000-0003-4808-4736</rdfs:comment>
    </owl:Axiom>
    


    <!-- http://purl.obolibrary.org/obo/ENVO_00002223 -->

    <owl:Class rdf:about="http://purl.obolibrary.org/obo/ENVO_00002223">
        <rdfs:subClassOf rdf:resource="http://purl.obolibrary.org/obo/ENVO_00002006"/>
        <obo:IAO_0000111 xml:lang="en">oligotrophic water</obo:IAO_0000111>
        <obo:IAO_0000115>Water with a very low nutrient level.</obo:IAO_0000115>
        <oboInOwl:hasOBONamespace>ENVO</oboInOwl:hasOBONamespace>
        <oboInOwl:id>ENVO:00002223</oboInOwl:id>
        <oboInOwl:inSubset rdf:resource="http://bcodmo/sm#material"/>
        <oboInOwl:inSubset rdf:resource="http://bcodmo/sm#matrix"/>
        <rdfs:label>oligotrophic water</rdfs:label>
        <rdfs:label xml:lang="en">oligotrophic water</rdfs:label>
    </owl:Class>
    <owl:Axiom>
        <owl:annotatedSource rdf:resource="http://purl.obolibrary.org/obo/ENVO_00002223"/>
        <owl:annotatedProperty rdf:resource="http://purl.obolibrary.org/obo/IAO_0000115"/>
        <owl:annotatedTarget>Water with a very low nutrient level.</owl:annotatedTarget>
        <oboInOwl:hasDbXref rdf:datatype="http://www.w3.org/2001/XMLSchema#string">MA:ma</oboInOwl:hasDbXref>
    </owl:Axiom>
    


    <!-- http://purl.obolibrary.org/obo/ENVO_00002224 -->

    <owl:Class rdf:about="http://purl.obolibrary.org/obo/ENVO_00002224">
        <rdfs:subClassOf rdf:resource="http://purl.obolibrary.org/obo/ENVO_00002006"/>
        <obo:IAO_0000111 xml:lang="en">eutrophic water</obo:IAO_0000111>
        <obo:IAO_0000115>Water with a high nutrient level.</obo:IAO_0000115>
        <oboInOwl:inSubset rdf:resource="http://bcodmo/sm#material"/>
        <oboInOwl:inSubset rdf:resource="http://bcodmo/sm#matrix"/>
        <rdfs:label>eutrophic water</rdfs:label>
        <rdfs:label xml:lang="en">eutrophic water</rdfs:label>
    </owl:Class>
    <owl:Axiom>
        <owl:annotatedSource rdf:resource="http://purl.obolibrary.org/obo/ENVO_00002224"/>
        <owl:annotatedProperty rdf:resource="http://purl.obolibrary.org/obo/IAO_0000115"/>
        <owl:annotatedTarget>Water with a high nutrient level.</owl:annotatedTarget>
        <oboInOwl:hasDbXref rdf:datatype="http://www.w3.org/2001/XMLSchema#string">MA:ma</oboInOwl:hasDbXref>
    </owl:Axiom>
    


    <!-- http://purl.obolibrary.org/obo/ENVO_00002225 -->

    <owl:Class rdf:about="http://purl.obolibrary.org/obo/ENVO_00002225">
        <rdfs:subClassOf rdf:resource="http://purl.obolibrary.org/obo/ENVO_00002006"/>
        <obo:IAO_0000111 xml:lang="en">mesotrophic water</obo:IAO_0000111>
        <obo:IAO_0000115>Water with a nutrient level intermediate between eutrophic and oligotrophic.</obo:IAO_0000115>
        <oboInOwl:hasOBONamespace>ENVO</oboInOwl:hasOBONamespace>
        <oboInOwl:id>ENVO:00002225</oboInOwl:id>
        <oboInOwl:inSubset rdf:resource="http://bcodmo/sm#material"/>
        <oboInOwl:inSubset rdf:resource="http://bcodmo/sm#matrix"/>
        <rdfs:label>mesotrophic water</rdfs:label>
        <rdfs:label xml:lang="en">mesotrophic water</rdfs:label>
    </owl:Class>
    <owl:Axiom>
        <owl:annotatedSource rdf:resource="http://purl.obolibrary.org/obo/ENVO_00002225"/>
        <owl:annotatedProperty rdf:resource="http://purl.obolibrary.org/obo/IAO_0000115"/>
        <owl:annotatedTarget>Water with a nutrient level intermediate between eutrophic and oligotrophic.</owl:annotatedTarget>
        <oboInOwl:hasDbXref rdf:datatype="http://www.w3.org/2001/XMLSchema#string">MA:ma</oboInOwl:hasDbXref>
    </owl:Axiom>
    


    <!-- http://purl.obolibrary.org/obo/ENVO_00002264 -->

    <owl:Class rdf:about="http://purl.obolibrary.org/obo/ENVO_00002264">
        <obo:IAO_0000111 xml:lang="en">waste material</obo:IAO_0000111>
        <obo:IAO_0000115>A material which is not the desired output of a process and which is typically the input of a process which removes it from its producer (e.g. a disposal process).</obo:IAO_0000115>
        <obo:IAO_0000116>This seems more like a role than a material. Anything can be waste. Thus, a &quot;waste&quot; role or disposition will be created and this class can then be populated by inference: any environmental material which has [role,disposition] waste will be considered a waste material.</obo:IAO_0000116>
        <oboInOwl:hasDbXref>EcoLexicon:waste</oboInOwl:hasDbXref>
        <oboInOwl:hasDbXref>SWEETRealm:Waste</oboInOwl:hasDbXref>
        <oboInOwl:hasDbXref>https://en.wikipedia.org/wiki/Waste</oboInOwl:hasDbXref>
        <oboInOwl:hasOBONamespace>ENVO</oboInOwl:hasOBONamespace>
        <oboInOwl:id>ENVO:00002264</oboInOwl:id>
        <oboInOwl:inSubset rdf:resource="http://bcodmo/sm#material"/>
        <oboInOwl:inSubset rdf:resource="http://bcodmo/sm#matrix"/>
        <rdfs:label>waste material</rdfs:label>
        <rdfs:label xml:lang="en">waste material</rdfs:label>
    </owl:Class>
    


    <!-- http://purl.obolibrary.org/obo/ENVO_00002982 -->

    <owl:Class rdf:about="http://purl.obolibrary.org/obo/ENVO_00002982">
        <obo:IAO_0000111 xml:lang="en">clay</obo:IAO_0000111>
        <obo:IAO_0000115>A group of hydrous aluminium phyllosilicate (phyllosilicates being a subgroup of silicate minerals) minerals (see clay minerals), that are typically less than 2 micrometres in diameter. Clay consists of a variety of phyllosilicate minerals rich in silicon and aluminium oxides and hydroxides which include variable amounts of structural water.</obo:IAO_0000115>
        <oboInOwl:hasDbXref>EcoLexicon:clay</oboInOwl:hasDbXref>
        <oboInOwl:hasDbXref>SWEETRealm:Clay</oboInOwl:hasDbXref>
        <oboInOwl:hasDbXref>https://en.wikipedia.org/wiki/Clay</oboInOwl:hasDbXref>
        <oboInOwl:inSubset rdf:resource="http://bcodmo/sm#material"/>
        <oboInOwl:inSubset rdf:resource="http://bcodmo/sm#matrix"/>
        <rdfs:label>clay</rdfs:label>
        <rdfs:label xml:lang="en">clay</rdfs:label>
    </owl:Class>
    <owl:Axiom>
        <owl:annotatedSource rdf:resource="http://purl.obolibrary.org/obo/ENVO_00002982"/>
        <owl:annotatedProperty rdf:resource="http://purl.obolibrary.org/obo/IAO_0000115"/>
        <owl:annotatedTarget>A group of hydrous aluminium phyllosilicate (phyllosilicates being a subgroup of silicate minerals) minerals (see clay minerals), that are typically less than 2 micrometres in diameter. Clay consists of a variety of phyllosilicate minerals rich in silicon and aluminium oxides and hydroxides which include variable amounts of structural water.</owl:annotatedTarget>
        <oboInOwl:hasDbXref>https://en.wikipedia.org/wiki/Clay</oboInOwl:hasDbXref>
    </owl:Axiom>
    


    <!-- http://purl.obolibrary.org/obo/ENVO_00002983 -->

    <owl:Class rdf:about="http://purl.obolibrary.org/obo/ENVO_00002983">
        <rdfs:subClassOf rdf:resource="http://purl.obolibrary.org/obo/ENVO_00002985"/>
        <obo:IAO_0000111 xml:lang="en">fuel oil</obo:IAO_0000111>
        <obo:IAO_0000115>An oil which 1) is liquid at room temperature (approximately 20 degrees Celsius) 2) is intended to be burned in a furnace or boiler for the generation of heat or used in an engine for the generation of power, 3) is obtained from petroleum distillation, either as a distillate or a residue, 4) composed of long hydrocarbon chains, particularly alkanes, cycloalkanes and aromatics.</obo:IAO_0000115>
        <oboInOwl:hasExactSynonym>furnace oil</oboInOwl:hasExactSynonym>
        <oboInOwl:hasExactSynonym>heavy oil</oboInOwl:hasExactSynonym>
        <oboInOwl:hasExactSynonym>marine fuel</oboInOwl:hasExactSynonym>
        <oboInOwl:inSubset rdf:resource="http://bcodmo/sm#material"/>
        <oboInOwl:inSubset rdf:resource="http://bcodmo/sm#matrix"/>
        <rdfs:comment>Oils having a flash point of approximately 42 degrees Celsius and oils burned in cotton or wool-wick burners are not typically considered fuel oils. The term fuel oil is also used in a stricter sense to refer only to the heaviest commercial fuel that can be obtained from crude oil, i.e., heavier than gasoline and naphtha.</rdfs:comment>
        <rdfs:label>fuel oil</rdfs:label>
        <rdfs:label xml:lang="en">fuel oil</rdfs:label>
    </owl:Class>
    <owl:Axiom>
        <owl:annotatedSource rdf:resource="http://purl.obolibrary.org/obo/ENVO_00002983"/>
        <owl:annotatedProperty rdf:resource="http://purl.obolibrary.org/obo/IAO_0000115"/>
        <owl:annotatedTarget>An oil which 1) is liquid at room temperature (approximately 20 degrees Celsius) 2) is intended to be burned in a furnace or boiler for the generation of heat or used in an engine for the generation of power, 3) is obtained from petroleum distillation, either as a distillate or a residue, 4) composed of long hydrocarbon chains, particularly alkanes, cycloalkanes and aromatics.</owl:annotatedTarget>
        <oboInOwl:hasDbXref>https://en.wikipedia.org/wiki/Fuel_oil</oboInOwl:hasDbXref>
    </owl:Axiom>
    <owl:Axiom>
        <owl:annotatedSource rdf:resource="http://purl.obolibrary.org/obo/ENVO_00002983"/>
        <owl:annotatedProperty rdf:resource="http://www.w3.org/2000/01/rdf-schema#comment"/>
        <owl:annotatedTarget>Oils having a flash point of approximately 42 degrees Celsius and oils burned in cotton or wool-wick burners are not typically considered fuel oils. The term fuel oil is also used in a stricter sense to refer only to the heaviest commercial fuel that can be obtained from crude oil, i.e., heavier than gasoline and naphtha.</owl:annotatedTarget>
        <oboInOwl:hasDbXref>https://en.wikipedia.org/wiki/Fuel_oil</oboInOwl:hasDbXref>
    </owl:Axiom>
    


    <!-- http://purl.obolibrary.org/obo/ENVO_00002984 -->

    <owl:Class rdf:about="http://purl.obolibrary.org/obo/ENVO_00002984">
        <rdfs:subClassOf rdf:resource="http://purl.obolibrary.org/obo/ENVO_00002985"/>
        <obo:IAO_0000111 xml:lang="en">petroleum</obo:IAO_0000111>
        <obo:IAO_0000115>A naturally occurring flammable liquid consisting of a complex mixture of hydrocarbons of various molecular weights and other liquid organic compounds, that are found in geologic formations beneath the planetary surfaces.</obo:IAO_0000115>
        <oboInOwl:hasDbXref>https://en.wikipedia.org/wiki/Petroleum</oboInOwl:hasDbXref>
        <oboInOwl:hasRelatedSynonym>crude oil</oboInOwl:hasRelatedSynonym>
        <oboInOwl:inSubset rdf:resource="http://bcodmo/sm#material"/>
        <oboInOwl:inSubset rdf:resource="http://bcodmo/sm#matrix"/>
        <rdfs:label>petroleum</rdfs:label>
        <rdfs:label xml:lang="en">petroleum</rdfs:label>
    </owl:Class>
    <owl:Axiom>
        <owl:annotatedSource rdf:resource="http://purl.obolibrary.org/obo/ENVO_00002984"/>
        <owl:annotatedProperty rdf:resource="http://purl.obolibrary.org/obo/IAO_0000115"/>
        <owl:annotatedTarget>A naturally occurring flammable liquid consisting of a complex mixture of hydrocarbons of various molecular weights and other liquid organic compounds, that are found in geologic formations beneath the planetary surfaces.</owl:annotatedTarget>
        <oboInOwl:hasDbXref>https://en.wikipedia.org/wiki/Petroleum</oboInOwl:hasDbXref>
    </owl:Axiom>
    


    <!-- http://purl.obolibrary.org/obo/ENVO_00002985 -->

    <owl:Class rdf:about="http://purl.obolibrary.org/obo/ENVO_00002985">
        <obo:IAO_0000111 xml:lang="en">oil</obo:IAO_0000111>
        <obo:IAO_0000115>A nonpolar, hydrophobic, and lipophilic material which is a viscous liquid at ambient temperatures (about 20 degrees Celsius) or slightly warmer.</obo:IAO_0000115>
        <oboInOwl:hasDbXref>EcoLexicon:oil</oboInOwl:hasDbXref>
        <oboInOwl:inSubset rdf:resource="http://bcodmo/sm#material"/>
        <oboInOwl:inSubset rdf:resource="http://bcodmo/sm#matrix"/>
        <rdfs:label>oil</rdfs:label>
        <rdfs:label xml:lang="en">oil</rdfs:label>
    </owl:Class>
    <owl:Axiom>
        <owl:annotatedSource rdf:resource="http://purl.obolibrary.org/obo/ENVO_00002985"/>
        <owl:annotatedProperty rdf:resource="http://purl.obolibrary.org/obo/IAO_0000115"/>
        <owl:annotatedTarget>A nonpolar, hydrophobic, and lipophilic material which is a viscous liquid at ambient temperatures (about 20 degrees Celsius) or slightly warmer.</owl:annotatedTarget>
        <oboInOwl:hasDbXref>https://en.wikipedia.org/wiki/Oil</oboInOwl:hasDbXref>
    </owl:Axiom>
    


    <!-- http://purl.obolibrary.org/obo/ENVO_00003044 -->

    <owl:Class rdf:about="http://purl.obolibrary.org/obo/ENVO_00003044">
        <rdfs:subClassOf rdf:resource="http://purl.obolibrary.org/obo/ENVO_00002012"/>
        <obo:IAO_0000111 xml:lang="en">brine</obo:IAO_0000111>
        <obo:IAO_0000115>Water saturated or nearly saturated with salt (NaCl).</obo:IAO_0000115>
        <oboInOwl:hasDbXref>EcoLexicon:brine</oboInOwl:hasDbXref>
        <oboInOwl:hasDbXref>SWEETRealm:Brine</oboInOwl:hasDbXref>
        <oboInOwl:hasDbXref>https://en.wikipedia.org/wiki/Brine</oboInOwl:hasDbXref>
        <oboInOwl:inSubset rdf:resource="http://bcodmo/sm#material"/>
        <oboInOwl:inSubset rdf:resource="http://bcodmo/sm#matrix"/>
        <oboInOwl:inSubset>envoPolar</oboInOwl:inSubset>
        <rdfs:comment>It is used (now less popular than historically) to preserve vegetables, fish, and meat.</rdfs:comment>
        <rdfs:label>brine</rdfs:label>
        <rdfs:label xml:lang="en">brine</rdfs:label>
    </owl:Class>
    <owl:Axiom>
        <owl:annotatedSource rdf:resource="http://purl.obolibrary.org/obo/ENVO_00003044"/>
        <owl:annotatedProperty rdf:resource="http://purl.obolibrary.org/obo/IAO_0000115"/>
        <owl:annotatedTarget>Water saturated or nearly saturated with salt (NaCl).</owl:annotatedTarget>
        <oboInOwl:hasDbXref>https://en.wikipedia.org/wiki/Brine</oboInOwl:hasDbXref>
    </owl:Axiom>
    


    <!-- http://purl.obolibrary.org/obo/ENVO_00003064 -->

    <owl:Class rdf:about="http://purl.obolibrary.org/obo/ENVO_00003064">
        <rdfs:subClassOf rdf:resource="http://purl.obolibrary.org/obo/ENVO_00002011"/>
        <obo:IAO_0000111 xml:lang="en">drinking water</obo:IAO_0000111>
        <obo:IAO_0000115>Drinking water is water which may be consumed by humans with no adverse effects on their health.</obo:IAO_0000115>
        <oboInOwl:hasDbXref>EcoLexicon:drinking_water</oboInOwl:hasDbXref>
        <oboInOwl:hasDbXref>SWEETRealm:DrinkingWater</oboInOwl:hasDbXref>
        <oboInOwl:hasDbXref>https://en.wikipedia.org/wiki/Drinking_water</oboInOwl:hasDbXref>
        <oboInOwl:hasExactSynonym>potable water</oboInOwl:hasExactSynonym>
        <oboInOwl:hasOBONamespace>ENVO</oboInOwl:hasOBONamespace>
        <oboInOwl:id>ENVO:00003064</oboInOwl:id>
        <oboInOwl:inSubset rdf:resource="http://bcodmo/sm#material"/>
        <oboInOwl:inSubset rdf:resource="http://bcodmo/sm#matrix"/>
        <rdfs:label>drinking water</rdfs:label>
        <rdfs:label xml:lang="en">drinking water</rdfs:label>
    </owl:Class>
    


    <!-- http://purl.obolibrary.org/obo/ENVO_00005738 -->

    <owl:Class rdf:about="http://purl.obolibrary.org/obo/ENVO_00005738">
        <obo:IAO_0000111 xml:lang="en">foam</obo:IAO_0000111>
        <oboInOwl:hasDbXref>https://en.wikipedia.org/wiki/Foam</oboInOwl:hasDbXref>
        <oboInOwl:inSubset rdf:resource="http://bcodmo/sm#material"/>
        <oboInOwl:inSubset rdf:resource="http://bcodmo/sm#matrix"/>
        <rdfs:comment>This is a state more than a material.</rdfs:comment>
        <rdfs:label>foam</rdfs:label>
        <rdfs:label xml:lang="en">foam</rdfs:label>
    </owl:Class>
    


    <!-- http://purl.obolibrary.org/obo/ENVO_00005791 -->

    <owl:Class rdf:about="http://purl.obolibrary.org/obo/ENVO_00005791">
        <rdfs:subClassOf rdf:resource="http://purl.obolibrary.org/obo/ENVO_00002006"/>
        <obo:IAO_0000111 xml:lang="en">sterile water</obo:IAO_0000111>
        <obo:IAO_0000115>Sterile water is water which does not contain lliving organisms.</obo:IAO_0000115>
        <oboInOwl:inSubset rdf:resource="http://bcodmo/sm#material"/>
        <oboInOwl:inSubset rdf:resource="http://bcodmo/sm#matrix"/>
        <rdfs:label>sterile water</rdfs:label>
        <rdfs:label xml:lang="en">sterile water</rdfs:label>
    </owl:Class>
    


    <!-- http://purl.obolibrary.org/obo/ENVO_00010505 -->

    <owl:Class rdf:about="http://purl.obolibrary.org/obo/ENVO_00010505">
        <obo:IAO_0000111 xml:lang="en">aerosol</obo:IAO_0000111>
        <obo:IAO_0000115>Airborne solid particles (also called dust or particulate matter (PM)) or liquid droplets.</obo:IAO_0000115>
        <oboInOwl:hasDbXref rdf:resource="http://purl.obolibrary.org/obo/envo.owl"/>
        <oboInOwl:hasDbXref>EcoLexicon:aerosol</oboInOwl:hasDbXref>
        <oboInOwl:hasDbXref>SWEETRealm:Aerosol</oboInOwl:hasDbXref>
        <oboInOwl:inSubset rdf:resource="http://bcodmo/sm#material"/>
        <oboInOwl:inSubset rdf:resource="http://bcodmo/sm#matrix"/>
        <oboInOwl:inSubset>envoAtmo</oboInOwl:inSubset>
        <rdfs:comment>Should connect to PATO as &quot;quality of an aerosol&quot;</rdfs:comment>
        <rdfs:label>aerosol</rdfs:label>
        <rdfs:label xml:lang="en">aerosol</rdfs:label>
    </owl:Class>
    <owl:Axiom>
        <owl:annotatedSource rdf:resource="http://purl.obolibrary.org/obo/ENVO_00010505"/>
        <owl:annotatedProperty rdf:resource="http://purl.obolibrary.org/obo/IAO_0000115"/>
        <owl:annotatedTarget>Airborne solid particles (also called dust or particulate matter (PM)) or liquid droplets.</owl:annotatedTarget>
        <oboInOwl:hasDbXref rdf:datatype="http://www.w3.org/2001/XMLSchema#string">https://en.wikipedia.org/wiki/Aerosol</oboInOwl:hasDbXref>
    </owl:Axiom>
    


    <!-- http://purl.obolibrary.org/obo/ENVO_00010506 -->

    <owl:Class rdf:about="http://purl.obolibrary.org/obo/ENVO_00010506">
        <obo:IAO_0000111 xml:lang="en">emulsion</obo:IAO_0000111>
        <obo:IAO_0000115>A mixture of two immiscible (unblendable) substances. One substance (the dispersed phase) is dispersed in the other (the continuous phase).</obo:IAO_0000115>
        <oboInOwl:hasDbXref>https://en.wikipedia.org/wiki/Emulsion</oboInOwl:hasDbXref>
        <oboInOwl:inSubset rdf:resource="http://bcodmo/sm#material"/>
        <oboInOwl:inSubset rdf:resource="http://bcodmo/sm#matrix"/>
        <rdfs:label>emulsion</rdfs:label>
        <rdfs:label xml:lang="en">emulsion</rdfs:label>
    </owl:Class>
    <owl:Axiom>
        <owl:annotatedSource rdf:resource="http://purl.obolibrary.org/obo/ENVO_00010506"/>
        <owl:annotatedProperty rdf:resource="http://purl.obolibrary.org/obo/IAO_0000115"/>
        <owl:annotatedTarget>A mixture of two immiscible (unblendable) substances. One substance (the dispersed phase) is dispersed in the other (the continuous phase).</owl:annotatedTarget>
        <oboInOwl:hasDbXref>https://en.wikipedia.org/wiki/Emulsion</oboInOwl:hasDbXref>
    </owl:Axiom>
    


    <!-- http://purl.obolibrary.org/obo/ENVO_01000001 -->

    <owl:Class rdf:about="http://purl.obolibrary.org/obo/ENVO_01000001">
        <obo:IAO_0000111 xml:lang="en">mud</obo:IAO_0000111>
        <obo:IAO_0000115>A liquid or semi-liquid mixture of water and some combination of soil, silt, and clay.</obo:IAO_0000115>
        <oboInOwl:hasDbXref>EcoLexicon:mud</oboInOwl:hasDbXref>
        <oboInOwl:hasDbXref>LTER:356</oboInOwl:hasDbXref>
        <oboInOwl:hasDbXref>SWEETRealm:Mud</oboInOwl:hasDbXref>
        <oboInOwl:hasDbXref>https://en.wikipedia.org/wiki/Mud</oboInOwl:hasDbXref>
        <oboInOwl:inSubset rdf:resource="http://bcodmo/sm#material"/>
        <oboInOwl:inSubset rdf:resource="http://bcodmo/sm#matrix"/>
        <rdfs:label>mud</rdfs:label>
        <rdfs:label xml:lang="en">mud</rdfs:label>
    </owl:Class>
    <owl:Axiom>
        <owl:annotatedSource rdf:resource="http://purl.obolibrary.org/obo/ENVO_01000001"/>
        <owl:annotatedProperty rdf:resource="http://purl.obolibrary.org/obo/IAO_0000115"/>
        <owl:annotatedTarget>A liquid or semi-liquid mixture of water and some combination of soil, silt, and clay.</owl:annotatedTarget>
        <oboInOwl:hasDbXref>https://en.wikipedia.org/wiki/Mud</oboInOwl:hasDbXref>
    </owl:Axiom>
    


    <!-- http://purl.obolibrary.org/obo/ENVO_01000017 -->

    <owl:Class rdf:about="http://purl.obolibrary.org/obo/ENVO_01000017">
        <obo:IAO_0000111 xml:lang="en">sand</obo:IAO_0000111>
        <obo:IAO_0000115>A naturally occurring granular material composed of finely divided rock and mineral particles.</obo:IAO_0000115>
        <oboInOwl:hasDbXref>EcoLexicon:sand</oboInOwl:hasDbXref>
        <oboInOwl:hasDbXref>LTER:484</oboInOwl:hasDbXref>
        <oboInOwl:hasDbXref>SWEETRealm:Sand</oboInOwl:hasDbXref>
        <oboInOwl:hasDbXref>https://en.wikipedia.org/wiki/Sand</oboInOwl:hasDbXref>
        <oboInOwl:hasOBONamespace>ENVO</oboInOwl:hasOBONamespace>
        <oboInOwl:id>ENVO:01000017</oboInOwl:id>
        <oboInOwl:inSubset rdf:resource="http://bcodmo/sm#material"/>
        <oboInOwl:inSubset rdf:resource="http://bcodmo/sm#matrix"/>
        <rdfs:label>sand</rdfs:label>
        <rdfs:label xml:lang="en">sand</rdfs:label>
    </owl:Class>
    <owl:Axiom>
        <owl:annotatedSource rdf:resource="http://purl.obolibrary.org/obo/ENVO_01000017"/>
        <owl:annotatedProperty rdf:resource="http://purl.obolibrary.org/obo/IAO_0000115"/>
        <owl:annotatedTarget>A naturally occurring granular material composed of finely divided rock and mineral particles.</owl:annotatedTarget>
        <oboInOwl:hasDbXref>https://en.wikipedia.org/wiki/Sand</oboInOwl:hasDbXref>
    </owl:Axiom>
    


    <!-- http://purl.obolibrary.org/obo/ENVO_01000060 -->

    <owl:Class rdf:about="http://purl.obolibrary.org/obo/ENVO_01000060">
        <obo:IAO_0000111 xml:lang="en">particulate matter</obo:IAO_0000111>
        <obo:IAO_0000115>Particulate material is an environmental material which is composed of microscopic portions of solid or liquid material suspended in another environmental material.</obo:IAO_0000115>
        <obo:IAO_0000116>Subclasses should be assigned by inference.</obo:IAO_0000116>
        <oboInOwl:inSubset rdf:resource="http://bcodmo/sm#material"/>
        <oboInOwl:inSubset rdf:resource="http://bcodmo/sm#matrix"/>
        <oboInOwl:inSubset>envoAtmo</oboInOwl:inSubset>
        <oboInOwl:inSubset>envoPolar</oboInOwl:inSubset>
        <rdfs:label xml:lang="en">particulate matter</rdfs:label>
    </owl:Class>
    


    <!-- http://purl.obolibrary.org/obo/ENVO_01000063 -->

    <owl:Class rdf:about="http://purl.obolibrary.org/obo/ENVO_01000063">
        <rdfs:subClassOf rdf:resource="http://purl.obolibrary.org/obo/ENVO_01000155"/>
        <obo:IAO_0000111 xml:lang="en">plankton</obo:IAO_0000111>
        <obo:IAO_0000115>A portion of planktonic material is a portion of environmental material primarily composed of plankton.</obo:IAO_0000115>
        <obo:IAO_0000116>See Issue #251. Awaiting class creation in PCO to attempt logical definitions.</obo:IAO_0000116>
        <oboInOwl:inSubset rdf:resource="http://bcodmo/sm#material"/>
        <oboInOwl:inSubset rdf:resource="http://bcodmo/sm#matrix"/>
        <oboInOwl:inSubset>envoPolar</oboInOwl:inSubset>
        <rdfs:label xml:lang="en">plankton</rdfs:label>
        <rdfs:label xml:lang="en">planktonic material</rdfs:label>
    </owl:Class>
    


    <!-- http://purl.obolibrary.org/obo/ENVO_01000134 -->

    <owl:Class rdf:about="http://purl.obolibrary.org/obo/ENVO_01000134">
        <rdfs:subClassOf rdf:resource="http://purl.obolibrary.org/obo/ENVO_00002141"/>
        <obo:IAO_0000111 xml:lang="en">hydrothermal fluid</obo:IAO_0000111>
        <obo:IAO_0000115>High temperature water ejected from hydrothermal vents and laden with dissolved metals and minerals as a result of percolation through crustal rocks.</obo:IAO_0000115>
        <oboInOwl:created_by rdf:datatype="http://www.w3.org/2001/XMLSchema#string">ORCID:0000-0002-4366-3088</oboInOwl:created_by>
        <oboInOwl:creation_date>2010-03-20T08:19:19Z</oboInOwl:creation_date>
        <oboInOwl:inSubset rdf:resource="http://bcodmo/sm#material"/>
        <oboInOwl:inSubset rdf:resource="http://bcodmo/sm#matrix"/>
        <rdfs:label>hydrothermal fluid</rdfs:label>
        <rdfs:label xml:lang="en">hydrothermal fluid</rdfs:label>
    </owl:Class>
    <owl:Axiom>
        <owl:annotatedSource rdf:resource="http://purl.obolibrary.org/obo/ENVO_01000134"/>
        <owl:annotatedProperty rdf:resource="http://purl.obolibrary.org/obo/IAO_0000115"/>
        <owl:annotatedTarget>High temperature water ejected from hydrothermal vents and laden with dissolved metals and minerals as a result of percolation through crustal rocks.</owl:annotatedTarget>
        <oboInOwl:hasDbXref rdf:datatype="http://www.w3.org/2001/XMLSchema#string">ISBN:978-0-444-82619-0</oboInOwl:hasDbXref>
        <oboInOwl:hasDbXref rdf:datatype="http://www.w3.org/2001/XMLSchema#string">ORCID:0000-0002-4366-3088</oboInOwl:hasDbXref>
    </owl:Axiom>
    


    <!-- http://purl.obolibrary.org/obo/ENVO_01000155 -->

    <owl:Class rdf:about="http://purl.obolibrary.org/obo/ENVO_01000155">
        <obo:IAO_0000111 xml:lang="en">organic material</obo:IAO_0000111>
        <obo:IAO_0000115>Environmental material derived from living organisms and composed primarily of one or more biomacromolecules.</obo:IAO_0000115>
        <oboInOwl:created_by rdf:datatype="http://www.w3.org/2001/XMLSchema#string">ORCID:0000-0002-4366-3088</oboInOwl:created_by>
        <oboInOwl:creation_date>2010-03-20T08:40:04Z</oboInOwl:creation_date>
        <oboInOwl:hasDbXref>EcoLexicon:organic_material</oboInOwl:hasDbXref>
        <oboInOwl:hasExactSynonym>biomass</oboInOwl:hasExactSynonym>
        <oboInOwl:inSubset rdf:resource="http://bcodmo/sm#material"/>
        <oboInOwl:inSubset rdf:resource="http://bcodmo/sm#matrix"/>
        <rdfs:label>organic material</rdfs:label>
        <rdfs:label xml:lang="en">organic material</rdfs:label>
    </owl:Class>
    <owl:Axiom>
        <owl:annotatedSource rdf:resource="http://purl.obolibrary.org/obo/ENVO_01000155"/>
        <owl:annotatedProperty rdf:resource="http://purl.obolibrary.org/obo/IAO_0000115"/>
        <owl:annotatedTarget>Environmental material derived from living organisms and composed primarily of one or more biomacromolecules.</owl:annotatedTarget>
        <oboInOwl:hasDbXref rdf:datatype="http://www.w3.org/2001/XMLSchema#string">ISBN:978-0-618-45504-1</oboInOwl:hasDbXref>
        <oboInOwl:hasDbXref rdf:datatype="http://www.w3.org/2001/XMLSchema#string">ORCID:0000-0002-4366-3088</oboInOwl:hasDbXref>
    </owl:Axiom>
    


    <!-- http://purl.obolibrary.org/obo/ENVO_01000156 -->

    <owl:Class rdf:about="http://purl.obolibrary.org/obo/ENVO_01000156">
        <rdfs:subClassOf rdf:resource="http://purl.obolibrary.org/obo/ENVO_01000155"/>
        <obo:IAO_0000111 xml:lang="en">biofilm material</obo:IAO_0000111>
        <obo:IAO_0000115>Material derived from a biofilm, an aggregate of microorganisms in which cells adhere to each other and/or to a surface. These adherent cells are frequently embedded within a self-produced matrix of extracellular polymeric substance (EPS). Biofilm EPS, which is also referred to as slime, is a polymeric conglomeration generally composed of extracellular DNA, proteins, and polysaccharides in various configurations.</obo:IAO_0000115>
        <oboInOwl:created_by rdf:datatype="http://www.w3.org/2001/XMLSchema#string">ORCID:0000-0002-4366-3088</oboInOwl:created_by>
        <oboInOwl:creation_date>2010-03-20T08:51:49Z</oboInOwl:creation_date>
        <oboInOwl:hasOBONamespace>ENVO</oboInOwl:hasOBONamespace>
        <oboInOwl:id>ENVO:01000156</oboInOwl:id>
        <oboInOwl:inSubset rdf:resource="http://bcodmo/sm#material"/>
        <oboInOwl:inSubset rdf:resource="http://bcodmo/sm#matrix"/>
        <rdfs:label>biofilm material</rdfs:label>
        <rdfs:label xml:lang="en">biofilm material</rdfs:label>
    </owl:Class>
    <owl:Axiom>
        <owl:annotatedSource rdf:resource="http://purl.obolibrary.org/obo/ENVO_01000156"/>
        <owl:annotatedProperty rdf:resource="http://purl.obolibrary.org/obo/IAO_0000115"/>
        <owl:annotatedTarget>Material derived from a biofilm, an aggregate of microorganisms in which cells adhere to each other and/or to a surface. These adherent cells are frequently embedded within a self-produced matrix of extracellular polymeric substance (EPS). Biofilm EPS, which is also referred to as slime, is a polymeric conglomeration generally composed of extracellular DNA, proteins, and polysaccharides in various configurations.</owl:annotatedTarget>
        <oboInOwl:hasDbXref rdf:datatype="http://www.w3.org/2001/XMLSchema#string">ORCID:0000-0002-4366-3088</oboInOwl:hasDbXref>
        <oboInOwl:hasDbXref rdf:datatype="http://www.w3.org/2001/XMLSchema#string">https://en.wikipedia.org/wiki/Biofilm</oboInOwl:hasDbXref>
    </owl:Axiom>
    


    <!-- http://purl.obolibrary.org/obo/ENVO_01000157 -->

    <owl:Class rdf:about="http://purl.obolibrary.org/obo/ENVO_01000157">
        <rdfs:subClassOf rdf:resource="http://purl.obolibrary.org/obo/ENVO_01000155"/>
        <obo:IAO_0000111 xml:lang="en">microbial mat</obo:IAO_0000111>
        <obo:IAO_0000115>Material derived from a microbial mat, a multi-layered sheet of micro-organisms, mainly bacteria and archaea. Microbial mats create a wide range of internal chemical environments.</obo:IAO_0000115>
        <oboInOwl:created_by rdf:datatype="http://www.w3.org/2001/XMLSchema#string">ORCID:0000-0002-4366-3088</oboInOwl:created_by>
        <oboInOwl:creation_date>2010-03-20T08:51:49Z</oboInOwl:creation_date>
        <oboInOwl:hasOBONamespace>ENVO</oboInOwl:hasOBONamespace>
        <oboInOwl:id>ENVO:01000157</oboInOwl:id>
        <oboInOwl:inSubset rdf:resource="http://bcodmo/sm#material"/>
        <oboInOwl:inSubset rdf:resource="http://bcodmo/sm#matrix"/>
        <oboInOwl:inSubset>envoPolar</oboInOwl:inSubset>
        <rdfs:label xml:lang="en">microbial mat</rdfs:label>
        <rdfs:label>microbial mat material</rdfs:label>
    </owl:Class>
    <owl:Axiom>
        <owl:annotatedSource rdf:resource="http://purl.obolibrary.org/obo/ENVO_01000157"/>
        <owl:annotatedProperty rdf:resource="http://purl.obolibrary.org/obo/IAO_0000115"/>
        <owl:annotatedTarget>Material derived from a microbial mat, a multi-layered sheet of micro-organisms, mainly bacteria and archaea. Microbial mats create a wide range of internal chemical environments.</owl:annotatedTarget>
        <oboInOwl:hasDbXref rdf:datatype="http://www.w3.org/2001/XMLSchema#string">ORCID:0000-0002-4366-3088</oboInOwl:hasDbXref>
        <oboInOwl:hasDbXref rdf:datatype="http://www.w3.org/2001/XMLSchema#string">https://en.wikipedia.org/wiki/Microbial_mat</oboInOwl:hasDbXref>
    </owl:Axiom>
    


    <!-- http://purl.obolibrary.org/obo/ENVO_01000158 -->

    <owl:Class rdf:about="http://purl.obolibrary.org/obo/ENVO_01000158">
        <rdfs:subClassOf rdf:resource="http://purl.obolibrary.org/obo/ENVO_01001103"/>
        <obo:IAO_0000111 xml:lang="en">marine snow</obo:IAO_0000111>
        <obo:IAO_0000115>Marine snow is a continuous shower of mostly organic detritus falling from the upper layers of the water column. Its origin lies in activities within the productive photic zone.</obo:IAO_0000115>
        <oboInOwl:created_by rdf:datatype="http://www.w3.org/2001/XMLSchema#string">ORCID:0000-0002-4366-3088</oboInOwl:created_by>
        <oboInOwl:creation_date>2010-03-20T08:51:49Z</oboInOwl:creation_date>
        <oboInOwl:hasDbXref>EcoLexicon:marine_snow</oboInOwl:hasDbXref>
        <oboInOwl:inSubset rdf:resource="http://bcodmo/sm#material"/>
        <oboInOwl:inSubset rdf:resource="http://bcodmo/sm#matrix"/>
        <oboInOwl:inSubset>envoPolar</oboInOwl:inSubset>
        <rdfs:label>marine snow</rdfs:label>
        <rdfs:label xml:lang="en">marine snow</rdfs:label>
    </owl:Class>
    <owl:Axiom>
        <owl:annotatedSource rdf:resource="http://purl.obolibrary.org/obo/ENVO_01000158"/>
        <owl:annotatedProperty rdf:resource="http://purl.obolibrary.org/obo/IAO_0000115"/>
        <owl:annotatedTarget>Marine snow is a continuous shower of mostly organic detritus falling from the upper layers of the water column. Its origin lies in activities within the productive photic zone.</owl:annotatedTarget>
        <oboInOwl:hasDbXref rdf:datatype="http://www.w3.org/2001/XMLSchema#string">ORCID:0000-0002-4366-3088</oboInOwl:hasDbXref>
        <oboInOwl:hasDbXref rdf:datatype="http://www.w3.org/2001/XMLSchema#string">https://en.wikipedia.org/wiki/Marine_snow</oboInOwl:hasDbXref>
    </owl:Axiom>
    


    <!-- http://purl.obolibrary.org/obo/ENVO_01000231 -->

    <owl:Class rdf:about="http://purl.obolibrary.org/obo/ENVO_01000231">
        <obo:IAO_0000111 xml:lang="en">lava</obo:IAO_0000111>
        <obo:IAO_0000115>Lava is a mixture of molten or semi-molten rock, volatiles, and solids which has extruded beyond a planetary crust.</obo:IAO_0000115>
        <oboInOwl:created_by>PLB</oboInOwl:created_by>
        <oboInOwl:creation_date>2013-05-05T16:52:47Z</oboInOwl:creation_date>
        <oboInOwl:hasDbXref>EcoLexicon:lava</oboInOwl:hasDbXref>
        <oboInOwl:hasDbXref>SWEETRealm:Lava</oboInOwl:hasDbXref>
        <oboInOwl:inSubset rdf:resource="http://bcodmo/sm#material"/>
        <oboInOwl:inSubset rdf:resource="http://bcodmo/sm#matrix"/>
        <rdfs:comment>Some use &apos;lava&apos; to refer to rock that is formed when lava cools. This is not the intended meaning of this class. See &apos;igneous rock&apos; or similar.</rdfs:comment>
        <rdfs:label>lava</rdfs:label>
        <rdfs:label xml:lang="en">lava</rdfs:label>
    </owl:Class>
    <owl:Axiom>
        <owl:annotatedSource rdf:resource="http://purl.obolibrary.org/obo/ENVO_01000231"/>
        <owl:annotatedProperty rdf:resource="http://purl.obolibrary.org/obo/IAO_0000115"/>
        <owl:annotatedTarget>Lava is a mixture of molten or semi-molten rock, volatiles, and solids which has extruded beyond a planetary crust.</owl:annotatedTarget>
        <oboInOwl:hasDbXref rdf:datatype="http://www.w3.org/2001/XMLSchema#string">https://en.wikipedia.org/wiki/Lava</oboInOwl:hasDbXref>
    </owl:Axiom>
    


    <!-- http://purl.obolibrary.org/obo/ENVO_01000256 -->

    <owl:Class rdf:about="http://purl.obolibrary.org/obo/ENVO_01000256">
        <obo:IAO_0000111 xml:lang="en">mineral</obo:IAO_0000111>
        <obo:IAO_0000115>A mineral material is an environmental material which is primarily composed of some substance that is naturally occurring, solid and stable at room temperature, representable by a chemical formula, usually abiogenic, and that has an ordered atomic structure.</obo:IAO_0000115>
        <obo:IAO_0000116>Look for &quot;mineral&quot; in a chemical or geochemical ontology to formalise the composed primarily of link.
From https://en.wikipedia.org/wiki/ [A mineral] is different from a rock, which can be an aggregate of minerals or non-minerals and does not have a specific chemical composition. The exact definition of a mineral is under debate, especially with respect to the requirement a valid species be abiogenic, and to a lesser extent with regards to it having an ordered atomic structure.</obo:IAO_0000116>
        <oboInOwl:created_by>ORCID:0000-0002-4366-3088</oboInOwl:created_by>
        <oboInOwl:creation_date>2013-10-05T12:37:41Z</oboInOwl:creation_date>
        <oboInOwl:hasDbXref>LTER:341</oboInOwl:hasDbXref>
        <oboInOwl:inSubset rdf:resource="http://bcodmo/sm#material"/>
        <oboInOwl:inSubset rdf:resource="http://bcodmo/sm#matrix"/>
        <rdfs:label xml:lang="en">mineral</rdfs:label>
        <rdfs:label>mineral material</rdfs:label>
    </owl:Class>
    <owl:Axiom>
        <owl:annotatedSource rdf:resource="http://purl.obolibrary.org/obo/ENVO_01000256"/>
        <owl:annotatedProperty rdf:resource="http://purl.obolibrary.org/obo/IAO_0000115"/>
        <owl:annotatedTarget>A mineral material is an environmental material which is primarily composed of some substance that is naturally occurring, solid and stable at room temperature, representable by a chemical formula, usually abiogenic, and that has an ordered atomic structure.</owl:annotatedTarget>
        <oboInOwl:hasDbXref>https://en.wikipedia.org/wiki/Mineral</oboInOwl:hasDbXref>
    </owl:Axiom>
    


    <!-- http://purl.obolibrary.org/obo/ENVO_01000266 -->

    <owl:Class rdf:about="http://purl.obolibrary.org/obo/ENVO_01000266">
        <rdfs:subClassOf rdf:resource="http://purl.obolibrary.org/obo/ENVO_01000797"/>
        <obo:IAO_0000111 xml:lang="en">vapor</obo:IAO_0000111>
        <obo:IAO_0000115>Water vapour is a vapour which is the gas phase of water.</obo:IAO_0000115>
        <oboInOwl:created_by>ORCID:0000-0002-4366-3088</oboInOwl:created_by>
        <oboInOwl:creation_date>2013-10-10T07:58:18Z</oboInOwl:creation_date>
        <oboInOwl:hasExactSynonym>aqueous vapor</oboInOwl:hasExactSynonym>
        <oboInOwl:hasExactSynonym>aqueous vapour</oboInOwl:hasExactSynonym>
        <oboInOwl:hasExactSynonym>water vapor</oboInOwl:hasExactSynonym>
        <oboInOwl:inSubset rdf:resource="http://bcodmo/sm#material"/>
        <oboInOwl:inSubset rdf:resource="http://bcodmo/sm#matrix"/>
        <rdfs:comment>Perhaps a better relation between water vapour and water can be found in or added to RO?</rdfs:comment>
        <rdfs:label xml:lang="en">vapor</rdfs:label>
        <rdfs:label>water vapour</rdfs:label>
    </owl:Class>
    <owl:Axiom>
        <owl:annotatedSource rdf:resource="http://purl.obolibrary.org/obo/ENVO_01000266"/>
        <owl:annotatedProperty rdf:resource="http://purl.obolibrary.org/obo/IAO_0000115"/>
        <owl:annotatedTarget>Water vapour is a vapour which is the gas phase of water.</owl:annotatedTarget>
        <oboInOwl:hasDbXref rdf:datatype="http://www.w3.org/2001/XMLSchema#string">https://en.wikipedia.org/wiki/Water_vapor</oboInOwl:hasDbXref>
    </owl:Axiom>
    <owl:Axiom>
        <owl:annotatedSource rdf:resource="http://purl.obolibrary.org/obo/ENVO_01000266"/>
        <owl:annotatedProperty rdf:resource="http://www.geneontology.org/formats/oboInOwl#hasExactSynonym"/>
        <owl:annotatedTarget>aqueous vapor</owl:annotatedTarget>
        <oboInOwl:hasDbXref rdf:datatype="http://www.w3.org/2001/XMLSchema#string">https://en.wikipedia.org/wiki/Water_vapor</oboInOwl:hasDbXref>
    </owl:Axiom>
    <owl:Axiom>
        <owl:annotatedSource rdf:resource="http://purl.obolibrary.org/obo/ENVO_01000266"/>
        <owl:annotatedProperty rdf:resource="http://www.geneontology.org/formats/oboInOwl#hasExactSynonym"/>
        <owl:annotatedTarget>aqueous vapour</owl:annotatedTarget>
        <oboInOwl:hasDbXref rdf:datatype="http://www.w3.org/2001/XMLSchema#string">https://en.wikipedia.org/wiki/Water_vapor</oboInOwl:hasDbXref>
    </owl:Axiom>
    <owl:Axiom>
        <owl:annotatedSource rdf:resource="http://purl.obolibrary.org/obo/ENVO_01000266"/>
        <owl:annotatedProperty rdf:resource="http://www.geneontology.org/formats/oboInOwl#hasExactSynonym"/>
        <owl:annotatedTarget>water vapor</owl:annotatedTarget>
        <oboInOwl:hasDbXref rdf:datatype="http://www.w3.org/2001/XMLSchema#string">https://en.wikipedia.org/wiki/Water_vapor</oboInOwl:hasDbXref>
    </owl:Axiom>
    


    <!-- http://purl.obolibrary.org/obo/ENVO_01000277 -->

    <owl:Class rdf:about="http://purl.obolibrary.org/obo/ENVO_01000277">
        <obo:IAO_0000111 xml:lang="en">ice</obo:IAO_0000111>
        <obo:IAO_0000115>Ice is water frozen into a solid state. It can appear transparent or opaque bluish-white color, depending on the presence of impurities or air inclusions. The addition of other materials such as soil may further alter its appearance.</obo:IAO_0000115>
        <oboInOwl:created_by>ORCID:0000-0002-4366-3088</oboInOwl:created_by>
        <oboInOwl:creation_date>2013-10-13T12:01:28Z</oboInOwl:creation_date>
        <oboInOwl:hasDbXref>LTER:262</oboInOwl:hasDbXref>
        <oboInOwl:hasRelatedSynonym>ice</oboInOwl:hasRelatedSynonym>
        <oboInOwl:inSubset rdf:resource="http://bcodmo/sm#material"/>
        <oboInOwl:inSubset rdf:resource="http://bcodmo/sm#matrix"/>
        <oboInOwl:inSubset>envoPolar</oboInOwl:inSubset>
        <rdfs:label xml:lang="en">ice</rdfs:label>
        <rdfs:label>water ice</rdfs:label>
    </owl:Class>
    <owl:Axiom>
        <owl:annotatedSource rdf:resource="http://purl.obolibrary.org/obo/ENVO_01000277"/>
        <owl:annotatedProperty rdf:resource="http://purl.obolibrary.org/obo/IAO_0000115"/>
        <owl:annotatedTarget>Ice is water frozen into a solid state. It can appear transparent or opaque bluish-white color, depending on the presence of impurities or air inclusions. The addition of other materials such as soil may further alter its appearance.</owl:annotatedTarget>
        <oboInOwl:hasDbXref rdf:datatype="http://www.w3.org/2001/XMLSchema#string">https://en.wikipedia.org/wiki/Ice</oboInOwl:hasDbXref>
    </owl:Axiom>
    <owl:Axiom>
        <owl:annotatedSource rdf:resource="http://purl.obolibrary.org/obo/ENVO_01000277"/>
        <owl:annotatedProperty rdf:resource="http://www.geneontology.org/formats/oboInOwl#hasRelatedSynonym"/>
        <owl:annotatedTarget>ice</owl:annotatedTarget>
        <oboInOwl:hasDbXref>http://www.eionet.europa.eu/gemet/concept/4131</oboInOwl:hasDbXref>
    </owl:Axiom>
    


    <!-- http://purl.obolibrary.org/obo/ENVO_01000301 -->

    <owl:Class rdf:about="http://purl.obolibrary.org/obo/ENVO_01000301">
        <rdfs:subClassOf rdf:resource="http://purl.obolibrary.org/obo/ENVO_00002019"/>
        <obo:IAO_0000111 xml:lang="en">estuarine water</obo:IAO_0000111>
        <obo:IAO_0000115>Brackish water which is part of an estuary.</obo:IAO_0000115>
        <oboInOwl:created_by>ORCID:0000-0002-4366-3088</oboInOwl:created_by>
        <oboInOwl:creation_date>2013-10-19T11:30:46Z</oboInOwl:creation_date>
        <oboInOwl:hasOBONamespace>ENVO</oboInOwl:hasOBONamespace>
        <oboInOwl:id>ENVO:01000301</oboInOwl:id>
        <oboInOwl:inSubset rdf:resource="http://bcodmo/sm#material"/>
        <oboInOwl:inSubset rdf:resource="http://bcodmo/sm#matrix"/>
        <rdfs:label>estuarine water</rdfs:label>
        <rdfs:label xml:lang="en">estuarine water</rdfs:label>
    </owl:Class>
    <owl:Axiom>
        <owl:annotatedSource rdf:resource="http://purl.obolibrary.org/obo/ENVO_01000301"/>
        <owl:annotatedProperty rdf:resource="http://purl.obolibrary.org/obo/IAO_0000115"/>
        <owl:annotatedTarget>Brackish water which is part of an estuary.</owl:annotatedTarget>
        <oboInOwl:hasDbXref rdf:datatype="http://www.w3.org/2001/XMLSchema#string">https://en.wikipedia.org/wiki/Estuary</oboInOwl:hasDbXref>
    </owl:Axiom>
    


    <!-- http://purl.obolibrary.org/obo/ENVO_01000404 -->

    <owl:Class rdf:about="http://purl.obolibrary.org/obo/ENVO_01000404">
        <obo:IAO_0000111 xml:lang="en">plastic</obo:IAO_0000111>
        <obo:IAO_0000115>A (portion of) plastic is an (portion of) anthropogenic environmental material including any of numerous organic synthetic or processed materials which are primarily composed of thermoplastic or thermosetting polymers of high molecular weight.</obo:IAO_0000115>
        <oboInOwl:hasDbXref>URL:http://aims.fao.org/aos/agrovoc/c_5998</oboInOwl:hasDbXref>
        <oboInOwl:hasDbXref>URL:http://eurovoc.europa.eu/1837</oboInOwl:hasDbXref>
        <oboInOwl:inSubset rdf:resource="http://bcodmo/sm#material"/>
        <oboInOwl:inSubset rdf:resource="http://bcodmo/sm#matrix"/>
        <oboInOwl:inSubset>envoPolar</oboInOwl:inSubset>
        <rdfs:label>manufactured plastic</rdfs:label>
        <rdfs:label xml:lang="en">plastic</rdfs:label>
    </owl:Class>
    <owl:Axiom>
        <owl:annotatedSource rdf:resource="http://purl.obolibrary.org/obo/ENVO_01000404"/>
        <owl:annotatedProperty rdf:resource="http://purl.obolibrary.org/obo/IAO_0000115"/>
        <owl:annotatedTarget>A (portion of) plastic is an (portion of) anthropogenic environmental material including any of numerous organic synthetic or processed materials which are primarily composed of thermoplastic or thermosetting polymers of high molecular weight.</owl:annotatedTarget>
        <oboInOwl:hasDbXref>http://www.merriam-webster.com/dictionary/plastic</oboInOwl:hasDbXref>
    </owl:Axiom>
    


    <!-- http://purl.obolibrary.org/obo/ENVO_01000406 -->

    <owl:Class rdf:about="http://purl.obolibrary.org/obo/ENVO_01000406">
        <obo:IAO_0000111 xml:lang="en">snow</obo:IAO_0000111>
        <obo:IAO_0000115>Snow is an environmental material which is primarily composed of flakes of crystalline water ice.</obo:IAO_0000115>
        <oboInOwl:inSubset rdf:resource="http://bcodmo/sm#material"/>
        <oboInOwl:inSubset rdf:resource="http://bcodmo/sm#matrix"/>
        <oboInOwl:inSubset>envoPolar</oboInOwl:inSubset>
        <rdfs:label>snow</rdfs:label>
        <rdfs:label xml:lang="en">snow</rdfs:label>
    </owl:Class>
    <owl:Axiom>
        <owl:annotatedSource rdf:resource="http://purl.obolibrary.org/obo/ENVO_01000406"/>
        <owl:annotatedProperty rdf:resource="http://purl.obolibrary.org/obo/IAO_0000115"/>
        <owl:annotatedTarget>Snow is an environmental material which is primarily composed of flakes of crystalline water ice.</owl:annotatedTarget>
        <oboInOwl:hasDbXref>http://www.eionet.europa.eu/gemet/concept/7769</oboInOwl:hasDbXref>
        <oboInOwl:hasDbXref>https://en.wikipedia.org/wiki/Snow</oboInOwl:hasDbXref>
    </owl:Axiom>
    


    <!-- http://purl.obolibrary.org/obo/ENVO_01000480 -->

    <owl:Class rdf:about="http://purl.obolibrary.org/obo/ENVO_01000480">
        <obo:IAO_0000111 xml:lang="en">glass</obo:IAO_0000111>
        <obo:IAO_0000115>Glass is an amorphous (non-crystalline) solid which is often transparent.</obo:IAO_0000115>
        <oboInOwl:created_by>ORCID:0000-0002-4366-3088</oboInOwl:created_by>
        <oboInOwl:inSubset rdf:resource="http://bcodmo/sm#material"/>
        <oboInOwl:inSubset rdf:resource="http://bcodmo/sm#matrix"/>
        <rdfs:comment>This class refers to all forms of glass. For the familiar form present in window panes and drinking glasses, consider silica-based glass.</rdfs:comment>
        <rdfs:label>glass</rdfs:label>
        <rdfs:label xml:lang="en">glass</rdfs:label>
    </owl:Class>
    <owl:Axiom>
        <owl:annotatedSource rdf:resource="http://purl.obolibrary.org/obo/ENVO_01000480"/>
        <owl:annotatedProperty rdf:resource="http://purl.obolibrary.org/obo/IAO_0000115"/>
        <owl:annotatedTarget>Glass is an amorphous (non-crystalline) solid which is often transparent.</owl:annotatedTarget>
        <oboInOwl:hasDbXref>https://en.wikipedia.org/wiki/Glass</oboInOwl:hasDbXref>
    </owl:Axiom>
    


    <!-- http://purl.obolibrary.org/obo/ENVO_01000552 -->

    <owl:Class rdf:about="http://purl.obolibrary.org/obo/ENVO_01000552">
        <rdfs:subClassOf rdf:resource="http://purl.obolibrary.org/obo/ENVO_01000554"/>
        <obo:IAO_0000111 xml:lang="en">natural gas</obo:IAO_0000111>
        <obo:IAO_0000115>Natural gas is a hydrocarbon gas mixture consisting primarily of methane, but commonly includes varying amounts of other higher alkanes and sometimes a usually lesser percentage of carbon dioxide, nitrogen, and/or hydrogen sulfide. Natural gas is a fossil fuel formed when layers of buried plants and gases are exposed to intense heat and pressure over thousands of years.</obo:IAO_0000115>
        <oboInOwl:inSubset rdf:resource="http://bcodmo/sm#material"/>
        <oboInOwl:inSubset rdf:resource="http://bcodmo/sm#matrix"/>
        <rdfs:label xml:lang="en">natural gas</rdfs:label>
    </owl:Class>
    <owl:Axiom>
        <owl:annotatedSource rdf:resource="http://purl.obolibrary.org/obo/ENVO_01000552"/>
        <owl:annotatedProperty rdf:resource="http://purl.obolibrary.org/obo/IAO_0000115"/>
        <owl:annotatedTarget>Natural gas is a hydrocarbon gas mixture consisting primarily of methane, but commonly includes varying amounts of other higher alkanes and sometimes a usually lesser percentage of carbon dioxide, nitrogen, and/or hydrogen sulfide. Natural gas is a fossil fuel formed when layers of buried plants and gases are exposed to intense heat and pressure over thousands of years.</owl:annotatedTarget>
        <oboInOwl:hasDbXref>https://en.wikipedia.org/wiki/Natural_gas</oboInOwl:hasDbXref>
    </owl:Axiom>
    


    <!-- http://purl.obolibrary.org/obo/ENVO_01000553 -->

    <owl:Class rdf:about="http://purl.obolibrary.org/obo/ENVO_01000553">
        <rdfs:subClassOf rdf:resource="http://purl.obolibrary.org/obo/ENVO_01000558"/>
        <obo:IAO_0000111 xml:lang="en">liquified petroleum gas</obo:IAO_0000111>
        <obo:IAO_0000115>Liquified petroleum gas or liquid petroleum gas (LPG or LP gas), also referred to as simply propane or butane, are flammable mixtures of hydrocarbon gases used as fuel in heating appliances, cooking equipment, and vehicles.</obo:IAO_0000115>
        <oboInOwl:hasExactSynonym>LP gas</oboInOwl:hasExactSynonym>
        <oboInOwl:hasExactSynonym>LPG</oboInOwl:hasExactSynonym>
        <oboInOwl:hasExactSynonym>liquid petroleum gas</oboInOwl:hasExactSynonym>
        <oboInOwl:hasRelatedSynonym>liquified natural gas</oboInOwl:hasRelatedSynonym>
        <oboInOwl:inSubset rdf:resource="http://bcodmo/sm#material"/>
        <oboInOwl:inSubset rdf:resource="http://bcodmo/sm#matrix"/>
        <rdfs:label xml:lang="en">liquefied petroleum gas</rdfs:label>
        <rdfs:label xml:lang="en">liquified petroleum gas</rdfs:label>
    </owl:Class>
    <owl:Axiom>
        <owl:annotatedSource rdf:resource="http://purl.obolibrary.org/obo/ENVO_01000553"/>
        <owl:annotatedProperty rdf:resource="http://purl.obolibrary.org/obo/IAO_0000115"/>
        <owl:annotatedTarget>Liquified petroleum gas or liquid petroleum gas (LPG or LP gas), also referred to as simply propane or butane, are flammable mixtures of hydrocarbon gases used as fuel in heating appliances, cooking equipment, and vehicles.</owl:annotatedTarget>
        <oboInOwl:hasDbXref>https://en.wikipedia.org/wiki/Liquefied_petroleum_gas</oboInOwl:hasDbXref>
    </owl:Axiom>
    


    <!-- http://purl.obolibrary.org/obo/ENVO_01000554 -->

    <owl:Class rdf:about="http://purl.obolibrary.org/obo/ENVO_01000554">
        <rdfs:subClassOf rdf:resource="http://purl.obolibrary.org/obo/ENVO_2000045"/>
        <obo:IAO_0000111 xml:lang="en">hydrocarbon gas</obo:IAO_0000111>
        <obo:IAO_0000115>A gas that is primarily composed of hydrocarbon molecules.</obo:IAO_0000115>
        <oboInOwl:inSubset rdf:resource="http://bcodmo/sm#material"/>
        <oboInOwl:inSubset rdf:resource="http://bcodmo/sm#matrix"/>
        <oboInOwl:inSubset>envoPolar</oboInOwl:inSubset>
        <rdfs:label xml:lang="en">hydrocarbon gas</rdfs:label>
    </owl:Class>
    


    <!-- http://purl.obolibrary.org/obo/ENVO_01000556 -->

    <owl:Class rdf:about="http://purl.obolibrary.org/obo/ENVO_01000556">
        <rdfs:subClassOf rdf:resource="http://purl.obolibrary.org/obo/ENVO_01000554"/>
        <obo:IAO_0000111 xml:lang="en">biogas</obo:IAO_0000111>
        <obo:IAO_0000115>Biogas is a mixture of different gases produced by the breakdown of organic matter in the absence of oxygen,  is primarily composed of methane and carbon dioxide, and may have small amounts of hydrogen sulfide, water, and siloxanes.</obo:IAO_0000115>
        <oboInOwl:inSubset rdf:resource="http://bcodmo/sm#material"/>
        <oboInOwl:inSubset rdf:resource="http://bcodmo/sm#matrix"/>
        <rdfs:comment>This is distinct from natural gas which is a fossil fuel product.</rdfs:comment>
        <rdfs:label xml:lang="en">biogas</rdfs:label>
    </owl:Class>
    <owl:Axiom>
        <owl:annotatedSource rdf:resource="http://purl.obolibrary.org/obo/ENVO_01000556"/>
        <owl:annotatedProperty rdf:resource="http://purl.obolibrary.org/obo/IAO_0000115"/>
        <owl:annotatedTarget>Biogas is a mixture of different gases produced by the breakdown of organic matter in the absence of oxygen,  is primarily composed of methane and carbon dioxide, and may have small amounts of hydrogen sulfide, water, and siloxanes.</owl:annotatedTarget>
        <oboInOwl:hasDbXref>https://en.wikipedia.org/wiki/</oboInOwl:hasDbXref>
    </owl:Axiom>
    


    <!-- http://purl.obolibrary.org/obo/ENVO_01000557 -->

    <owl:Class rdf:about="http://purl.obolibrary.org/obo/ENVO_01000557">
        <rdfs:subClassOf rdf:resource="http://purl.obolibrary.org/obo/ENVO_01000558"/>
        <obo:IAO_0000111 xml:lang="en">liquified natural gas</obo:IAO_0000111>
        <obo:IAO_0000115>Liquefied natural gas (LNG) is natural gas (predominantly methane, CH4) that has been converted to liquid form for ease of storage or transport. It takes up about 1/600th the volume of natural gas in the gaseous state. It is odorless, colorless, non-toxic and non-corrosive. LNG achieves a higher reduction in volume than compressed natural gas (CNG) so that the (volumetric) energy density of LNG is 2.4 times greater than that of CNG or 60 percent of that of diesel fuel.</obo:IAO_0000115>
        <oboInOwl:hasExactSynonym>LNG</oboInOwl:hasExactSynonym>
        <oboInOwl:hasExactSynonym>liquified natural gas</oboInOwl:hasExactSynonym>
        <oboInOwl:inSubset rdf:resource="http://bcodmo/sm#material"/>
        <oboInOwl:inSubset rdf:resource="http://bcodmo/sm#matrix"/>
        <rdfs:label xml:lang="en">liquefied natural gas</rdfs:label>
        <rdfs:label xml:lang="en">liquified natural gas</rdfs:label>
    </owl:Class>
    <owl:Axiom>
        <owl:annotatedSource rdf:resource="http://purl.obolibrary.org/obo/ENVO_01000557"/>
        <owl:annotatedProperty rdf:resource="http://purl.obolibrary.org/obo/IAO_0000115"/>
        <owl:annotatedTarget>Liquefied natural gas (LNG) is natural gas (predominantly methane, CH4) that has been converted to liquid form for ease of storage or transport. It takes up about 1/600th the volume of natural gas in the gaseous state. It is odorless, colorless, non-toxic and non-corrosive. LNG achieves a higher reduction in volume than compressed natural gas (CNG) so that the (volumetric) energy density of LNG is 2.4 times greater than that of CNG or 60 percent of that of diesel fuel.</owl:annotatedTarget>
        <oboInOwl:hasDbXref>https://en.wikipedia.org/wiki/Liquefied_natural_gas</oboInOwl:hasDbXref>
    </owl:Axiom>
    


    <!-- http://purl.obolibrary.org/obo/ENVO_01000558 -->

    <owl:Class rdf:about="http://purl.obolibrary.org/obo/ENVO_01000558">
        <rdfs:subClassOf rdf:resource="http://purl.obolibrary.org/obo/ENVO_2000045"/>
        <obo:IAO_0000111 xml:lang="en">liquified hydrocarbon gas</obo:IAO_0000111>
        <oboInOwl:inSubset rdf:resource="http://bcodmo/sm#material"/>
        <oboInOwl:inSubset rdf:resource="http://bcodmo/sm#matrix"/>
        <oboInOwl:inSubset>envoPolar</oboInOwl:inSubset>
        <rdfs:label xml:lang="en">liquefied hydrocarbon gas</rdfs:label>
        <rdfs:label xml:lang="en">liquified hydrocarbon gas</rdfs:label>
    </owl:Class>
    


    <!-- http://purl.obolibrary.org/obo/ENVO_01000560 -->

    <owl:Class rdf:about="http://purl.obolibrary.org/obo/ENVO_01000560">
        <rdfs:subClassOf rdf:resource="http://purl.obolibrary.org/obo/ENVO_2000045"/>
        <obo:IAO_0000111 xml:lang="en">charcoal</obo:IAO_0000111>
        <obo:IAO_0000115>Charcoal is a light, black residue, consisting of carbon and any remaining ash, obtained by removing water and other volatile constituents from animal and vegetation substances. Charcoal is usually produced by slow pyrolysis, the heating of wood or other substances in the absence of oxygen.</obo:IAO_0000115>
        <oboInOwl:inSubset rdf:resource="http://bcodmo/sm#material"/>
        <oboInOwl:inSubset rdf:resource="http://bcodmo/sm#matrix"/>
        <rdfs:label xml:lang="en">charcoal</rdfs:label>
    </owl:Class>
    <owl:Axiom>
        <owl:annotatedSource rdf:resource="http://purl.obolibrary.org/obo/ENVO_01000560"/>
        <owl:annotatedProperty rdf:resource="http://purl.obolibrary.org/obo/IAO_0000115"/>
        <owl:annotatedTarget>Charcoal is a light, black residue, consisting of carbon and any remaining ash, obtained by removing water and other volatile constituents from animal and vegetation substances. Charcoal is usually produced by slow pyrolysis, the heating of wood or other substances in the absence of oxygen.</owl:annotatedTarget>
        <oboInOwl:hasDbXref>https://en.wikipedia.org/wiki/Charcoal</oboInOwl:hasDbXref>
    </owl:Axiom>
    


    <!-- http://purl.obolibrary.org/obo/ENVO_01000575 -->

    <owl:Class rdf:about="http://purl.obolibrary.org/obo/ENVO_01000575">
        <obo:IAO_0000111 xml:lang="en">wax</obo:IAO_0000111>
        <obo:IAO_0000115>A wax is an environmental material which is primarily composed of lipids or other organic compounds that consist of long alkyl chains. Waxes are are malleable near ambient temperatures and melt at approximately 45 degrees Celsius.</obo:IAO_0000115>
        <oboInOwl:inSubset rdf:resource="http://bcodmo/sm#material"/>
        <oboInOwl:inSubset rdf:resource="http://bcodmo/sm#matrix"/>
        <rdfs:label xml:lang="en">wax</rdfs:label>
    </owl:Class>
    <owl:Axiom>
        <owl:annotatedSource rdf:resource="http://purl.obolibrary.org/obo/ENVO_01000575"/>
        <owl:annotatedProperty rdf:resource="http://purl.obolibrary.org/obo/IAO_0000115"/>
        <owl:annotatedTarget>A wax is an environmental material which is primarily composed of lipids or other organic compounds that consist of long alkyl chains. Waxes are are malleable near ambient temperatures and melt at approximately 45 degrees Celsius.</owl:annotatedTarget>
        <oboInOwl:hasDbXref>https://en.wikipedia.org/wiki/Wax</oboInOwl:hasDbXref>
    </owl:Axiom>
    


    <!-- http://purl.obolibrary.org/obo/ENVO_01000599 -->

    <owl:Class rdf:about="http://purl.obolibrary.org/obo/ENVO_01000599">
        <rdfs:subClassOf rdf:resource="http://purl.obolibrary.org/obo/ENVO_00002006"/>
        <obo:IAO_0000111 xml:lang="en">river water</obo:IAO_0000111>
        <oboInOwl:inSubset rdf:resource="http://bcodmo/sm#material"/>
        <oboInOwl:inSubset rdf:resource="http://bcodmo/sm#matrix"/>
        <rdfs:label xml:lang="en">river water</rdfs:label>
    </owl:Class>
    


    <!-- http://purl.obolibrary.org/obo/ENVO_01000600 -->

    <owl:Class rdf:about="http://purl.obolibrary.org/obo/ENVO_01000600">
        <rdfs:subClassOf rdf:resource="http://purl.obolibrary.org/obo/ENVO_00002011"/>
        <obo:IAO_0000111 xml:lang="en">rainwater</obo:IAO_0000111>
        <obo:IAO_0000115>Rainwater is liquid water which has precipitated in the form of droplets through the condensation of atmospheric water vapour.</obo:IAO_0000115>
        <oboInOwl:inSubset rdf:resource="http://bcodmo/sm#material"/>
        <oboInOwl:inSubset rdf:resource="http://bcodmo/sm#matrix"/>
        <rdfs:label xml:lang="en">rainwater</rdfs:label>
    </owl:Class>
    <owl:Axiom>
        <owl:annotatedSource rdf:resource="http://purl.obolibrary.org/obo/ENVO_01000600"/>
        <owl:annotatedProperty rdf:resource="http://purl.obolibrary.org/obo/IAO_0000115"/>
        <owl:annotatedTarget>Rainwater is liquid water which has precipitated in the form of droplets through the condensation of atmospheric water vapour.</owl:annotatedTarget>
        <oboInOwl:hasDbXref>https://en.wikipedia.org/wiki/Rain</oboInOwl:hasDbXref>
    </owl:Axiom>
    


    <!-- http://purl.obolibrary.org/obo/ENVO_01000722 -->

    <owl:Class rdf:about="http://purl.obolibrary.org/obo/ENVO_01000722">
        <rdfs:subClassOf rdf:resource="http://purl.obolibrary.org/obo/ENVO_00002006"/>
        <obo:IAO_0000111 xml:lang="en">meltwater</obo:IAO_0000111>
        <obo:IAO_0000115>Meltwater is the water released by the melting of snow or ice, including glacial ice, tabular icebergs and ice shelves over oceans.</obo:IAO_0000115>
        <oboInOwl:inSubset rdf:resource="http://bcodmo/sm#material"/>
        <oboInOwl:inSubset rdf:resource="http://bcodmo/sm#matrix"/>
        <rdfs:label xml:lang="en">meltwater</rdfs:label>
    </owl:Class>
    <owl:Axiom>
        <owl:annotatedSource rdf:resource="http://purl.obolibrary.org/obo/ENVO_01000722"/>
        <owl:annotatedProperty rdf:resource="http://purl.obolibrary.org/obo/IAO_0000115"/>
        <owl:annotatedTarget>Meltwater is the water released by the melting of snow or ice, including glacial ice, tabular icebergs and ice shelves over oceans.</owl:annotatedTarget>
        <oboInOwl:hasDbXref>https://en.wikipedia.org/wiki/Meltwater</oboInOwl:hasDbXref>
    </owl:Axiom>
    


    <!-- http://purl.obolibrary.org/obo/ENVO_01000797 -->

    <owl:Class rdf:about="http://purl.obolibrary.org/obo/ENVO_01000797">
        <obo:IAO_0000111 xml:lang="en">gas</obo:IAO_0000111>
        <obo:IAO_0000115>A material entity which is composed of one or more chemical entities and has neither independent shape nor volume but tends to expand indefinitely.</obo:IAO_0000115>
        <obo:IAO_0000116>This class is to be populated by inference.</obo:IAO_0000116>
        <oboInOwl:hasNarrowSynonym>gas</oboInOwl:hasNarrowSynonym>
        <oboInOwl:inSubset rdf:resource="http://bcodmo/sm#material"/>
        <oboInOwl:inSubset rdf:resource="http://bcodmo/sm#matrix"/>
        <rdfs:label xml:lang="en">gas</rdfs:label>
        <rdfs:label xml:lang="en">gaseous environmental material</rdfs:label>
    </owl:Class>
    <owl:Axiom>
        <owl:annotatedSource rdf:resource="http://purl.obolibrary.org/obo/ENVO_01000797"/>
        <owl:annotatedProperty rdf:resource="http://purl.obolibrary.org/obo/IAO_0000115"/>
        <owl:annotatedTarget>A material entity which is composed of one or more chemical entities and has neither independent shape nor volume but tends to expand indefinitely.</owl:annotatedTarget>
        <oboInOwl:hasDbXref>http://www.merriam-webster.com/dictionary/gas</oboInOwl:hasDbXref>
    </owl:Axiom>
    


    <!-- http://purl.obolibrary.org/obo/ENVO_01000838 -->

    <owl:Class rdf:about="http://purl.obolibrary.org/obo/ENVO_01000838">
        <rdfs:subClassOf rdf:resource="http://purl.obolibrary.org/obo/ENVO_00010505"/>
        <obo:IAO_0000111 xml:lang="en">smoke</obo:IAO_0000111>
        <oboInOwl:inSubset rdf:resource="http://bcodmo/sm#material"/>
        <oboInOwl:inSubset rdf:resource="http://bcodmo/sm#matrix"/>
        <rdfs:comment>Smoke is a collection of airborne solid and liquid particulates and gases emitted when a material undergoes combustion or pyrolysis, together with the quantity of gas that is entrained or otherwise mixed into the mass</rdfs:comment>
        <rdfs:label xml:lang="en">smoke</rdfs:label>
    </owl:Class>
    <owl:Axiom>
        <owl:annotatedSource rdf:resource="http://purl.obolibrary.org/obo/ENVO_01000838"/>
        <owl:annotatedProperty rdf:resource="http://www.w3.org/2000/01/rdf-schema#comment"/>
        <owl:annotatedTarget>Smoke is a collection of airborne solid and liquid particulates and gases emitted when a material undergoes combustion or pyrolysis, together with the quantity of gas that is entrained or otherwise mixed into the mass</owl:annotatedTarget>
        <oboInOwl:hasDbXref>https://en.wikipedia.org/wiki/Smoke</oboInOwl:hasDbXref>
    </owl:Axiom>
    


    <!-- http://purl.obolibrary.org/obo/ENVO_01000844 -->

    <owl:Class rdf:about="http://purl.obolibrary.org/obo/ENVO_01000844">
        <rdfs:subClassOf rdf:resource="http://purl.obolibrary.org/obo/ENVO_00010505"/>
        <obo:IAO_0000111 xml:lang="en">fog</obo:IAO_0000111>
        <obo:IAO_0000115>A visible mass of cloud water droplets or ice crystals suspended in the air at or near a planetary surface.</obo:IAO_0000115>
        <oboInOwl:hasRelatedSynonym>haar</oboInOwl:hasRelatedSynonym>
        <oboInOwl:inSubset rdf:resource="http://bcodmo/sm#material"/>
        <oboInOwl:inSubset rdf:resource="http://bcodmo/sm#matrix"/>
        <rdfs:comment>Fog is more opaque than mist, reducing visibility to under one kilometre. This class refers only to fog formed by materials primarily composed of water. &quot;Fog can be considered a type of low-lying cloud and is heavily influenced by nearby bodies of water, topography, and wind conditions. In turn, fog has affected many human activities, such as shipping, travel, and warfare.&quot; https://en.wikipedia.org/wiki/Fog</rdfs:comment>
        <rdfs:label xml:lang="en">fog</rdfs:label>
    </owl:Class>
    <owl:Axiom>
        <owl:annotatedSource rdf:resource="http://purl.obolibrary.org/obo/ENVO_01000844"/>
        <owl:annotatedProperty rdf:resource="http://purl.obolibrary.org/obo/IAO_0000115"/>
        <owl:annotatedTarget>A visible mass of cloud water droplets or ice crystals suspended in the air at or near a planetary surface.</owl:annotatedTarget>
        <oboInOwl:hasDbXref>https://en.wikipedia.org/wiki/Fog</oboInOwl:hasDbXref>
    </owl:Axiom>
    


    <!-- http://purl.obolibrary.org/obo/ENVO_01000851 -->

    <owl:Class rdf:about="http://purl.obolibrary.org/obo/ENVO_01000851">
        <obo:IAO_0000111 xml:lang="en">methane clathrate</obo:IAO_0000111>
        <obo:IAO_0000115>A clathrate material in which a large amount of methane is trapped within a crystal structure of water, forming a solid similar to ice.</obo:IAO_0000115>
        <oboInOwl:hasExactSynonym>fire ice</oboInOwl:hasExactSynonym>
        <oboInOwl:hasExactSynonym>gas hydrate</oboInOwl:hasExactSynonym>
        <oboInOwl:hasExactSynonym>hydromethane</oboInOwl:hasExactSynonym>
        <oboInOwl:hasExactSynonym>methane hydrate</oboInOwl:hasExactSynonym>
        <oboInOwl:hasExactSynonym>methane ice</oboInOwl:hasExactSynonym>
        <oboInOwl:hasExactSynonym>natural gas hydrate</oboInOwl:hasExactSynonym>
        <oboInOwl:inSubset rdf:resource="http://bcodmo/sm#material"/>
        <oboInOwl:inSubset rdf:resource="http://bcodmo/sm#matrix"/>
        <oboInOwl:inSubset>envoPolar</oboInOwl:inSubset>
        <rdfs:label xml:lang="en">methane clathrate</rdfs:label>
    </owl:Class>
    <owl:Axiom>
        <owl:annotatedSource rdf:resource="http://purl.obolibrary.org/obo/ENVO_01000851"/>
        <owl:annotatedProperty rdf:resource="http://purl.obolibrary.org/obo/IAO_0000115"/>
        <owl:annotatedTarget>A clathrate material in which a large amount of methane is trapped within a crystal structure of water, forming a solid similar to ice.</owl:annotatedTarget>
        <oboInOwl:hasDbXref>https://en.wikipedia.org/wiki/Methane_clathrate</oboInOwl:hasDbXref>
    </owl:Axiom>
    


    <!-- http://purl.obolibrary.org/obo/ENVO_01000872 -->

    <owl:Class rdf:about="http://purl.obolibrary.org/obo/ENVO_01000872">
        <rdfs:subClassOf rdf:resource="http://purl.obolibrary.org/obo/ENVO_00002006"/>
        <obo:IAO_0000111 xml:lang="en">ballast water</obo:IAO_0000111>
        <obo:IAO_0000115>Ballast water is water contained in the ballast tanks of sea-going vessels.</obo:IAO_0000115>
        <oboInOwl:inSubset rdf:resource="http://bcodmo/sm#material"/>
        <oboInOwl:inSubset rdf:resource="http://bcodmo/sm#matrix"/>
        <rdfs:comment>This definition could be improved, as ballast water is often used in more general ways, beyond the water contained in a ballast tank at any given time. For example, water which has just been released from a ballast tank is often still refered to as ballast water.</rdfs:comment>
        <rdfs:label xml:lang="en">ballast water</rdfs:label>
    </owl:Class>
    <owl:Axiom>
        <owl:annotatedSource rdf:resource="http://purl.obolibrary.org/obo/ENVO_01000872"/>
        <owl:annotatedProperty rdf:resource="http://purl.obolibrary.org/obo/IAO_0000115"/>
        <owl:annotatedTarget>Ballast water is water contained in the ballast tanks of sea-going vessels.</owl:annotatedTarget>
        <oboInOwl:hasDbXref>http://www.nature.com/news/four-routes-to-better-maritime-governance-1.21051?WT.mc_id=TWT_NatureNews</oboInOwl:hasDbXref>
        <oboInOwl:hasDbXref>https://en.wikipedia.org/wiki/Ballast_water_discharge_and_the_environment</oboInOwl:hasDbXref>
        <oboInOwl:hasDbXref>https://en.wikipedia.org/wiki/Sailing_ballast#Water_ballast</oboInOwl:hasDbXref>
    </owl:Axiom>
    


    <!-- http://purl.obolibrary.org/obo/ENVO_01000940 -->

    <owl:Class rdf:about="http://purl.obolibrary.org/obo/ENVO_01000940">
        <rdfs:subClassOf rdf:resource="http://purl.obolibrary.org/obo/ENVO_00002006"/>
        <obo:IAO_0000111 xml:lang="en">fissure water</obo:IAO_0000111>
        <obo:IAO_0000115>Water which is partially contained within a fissure or a geological fracture.</obo:IAO_0000115>
        <obo:IAO_0000116>The axiomatisation should be more tuned to the site within the fissure.</obo:IAO_0000116>
        <oboInOwl:hasExactSynonym>fracture water</oboInOwl:hasExactSynonym>
        <oboInOwl:inSubset rdf:resource="http://bcodmo/sm#material"/>
        <oboInOwl:inSubset rdf:resource="http://bcodmo/sm#matrix"/>
        <rdfs:comment>While containment is often enough to classify this subtype of water, it is expected that the water&apos;s composition is altered by contact with the solid material bounding the fissure&apos;s site.</rdfs:comment>
        <rdfs:label xml:lang="en">fissure water</rdfs:label>
    </owl:Class>
    <owl:Axiom>
        <owl:annotatedSource rdf:resource="http://purl.obolibrary.org/obo/ENVO_01000940"/>
        <owl:annotatedProperty rdf:resource="http://purl.obolibrary.org/obo/IAO_0000115"/>
        <owl:annotatedTarget>Water which is partially contained within a fissure or a geological fracture.</owl:annotatedTarget>
        <oboInOwl:hasDbXref>https://github.com/EnvironmentOntology/envo/issues/466</oboInOwl:hasDbXref>
    </owl:Axiom>
    


    <!-- http://purl.obolibrary.org/obo/ENVO_01000964 -->

    <owl:Class rdf:about="http://purl.obolibrary.org/obo/ENVO_01000964">
        <rdfs:subClassOf rdf:resource="http://purl.obolibrary.org/obo/ENVO_00002001"/>
        <obo:IAO_0000111 xml:lang="en">industrial wastewater</obo:IAO_0000111>
        <obo:IAO_0000115>Wastewater which is produced by industrial activity and which contains chemical contaminants other than those associated with urine and fecal matter.</obo:IAO_0000115>
        <oboInOwl:inSubset rdf:resource="http://bcodmo/sm#material"/>
        <oboInOwl:inSubset rdf:resource="http://bcodmo/sm#matrix"/>
        <rdfs:label xml:lang="en">industrial wastewater</rdfs:label>
    </owl:Class>
    


    <!-- http://purl.obolibrary.org/obo/ENVO_01001004 -->

    <owl:Class rdf:about="http://purl.obolibrary.org/obo/ENVO_01001004">
        <rdfs:subClassOf rdf:resource="http://purl.obolibrary.org/obo/ENVO_00002006"/>
        <obo:IAO_0000111 xml:lang="en">groundwater</obo:IAO_0000111>
        <obo:IAO_0000115>Underground water which is located in pore spaces found in rock or unconsolidated deposits such as soil, clay, or gravel.</obo:IAO_0000115>
        <oboInOwl:hasExactSynonym>ground water</oboInOwl:hasExactSynonym>
        <oboInOwl:inSubset rdf:resource="http://bcodmo/sm#material"/>
        <oboInOwl:inSubset rdf:resource="http://bcodmo/sm#matrix"/>
        <rdfs:comment>The definition of aquifer is quite permissive, referencing any water bearing rock or unconsolidated material.</rdfs:comment>
        <rdfs:label xml:lang="en">groundwater</rdfs:label>
    </owl:Class>
    <owl:Axiom>
        <owl:annotatedSource rdf:resource="http://purl.obolibrary.org/obo/ENVO_01001004"/>
        <owl:annotatedProperty rdf:resource="http://purl.obolibrary.org/obo/IAO_0000115"/>
        <owl:annotatedTarget>Underground water which is located in pore spaces found in rock or unconsolidated deposits such as soil, clay, or gravel.</owl:annotatedTarget>
        <oboInOwl:hasDbXref>https://en.wikipedia.org/wiki/Groundwater</oboInOwl:hasDbXref>
    </owl:Axiom>
    


    <!-- http://purl.obolibrary.org/obo/ENVO_01001063 -->

    <owl:Class rdf:about="http://purl.obolibrary.org/obo/ENVO_01001063">
        <rdfs:subClassOf rdf:resource="http://purl.obolibrary.org/obo/ENVO_00002006"/>
        <obo:IAO_0000111 xml:lang="en">oxic water</obo:IAO_0000111>
        <obo:IAO_0000115>Water which has an appreciable concentration of dissolved oxygen.</obo:IAO_0000115>
        <oboInOwl:created_by rdf:datatype="http://www.w3.org/2001/XMLSchema#string">ORCID:0000-0002-4366-3088</oboInOwl:created_by>
        <oboInOwl:creation_date>2010-03-21T06:05:53Z</oboInOwl:creation_date>
        <oboInOwl:inSubset rdf:resource="http://bcodmo/sm#material"/>
        <oboInOwl:inSubset rdf:resource="http://bcodmo/sm#matrix"/>
        <rdfs:comment>The threshold dissolved oxygen concentration past which water is considered oxic is variable. Typically, this is understood as the concentration at and beyond which organisms inhabiting that water can sustain aerobic metabolism and good health. For most systems, this is above 80% oxygen saturation. Input is welcome here https://github.com/EnvironmentOntology/envo/issues/536</rdfs:comment>
        <rdfs:label xml:lang="en">oxic water</rdfs:label>
    </owl:Class>
    <owl:Axiom>
        <owl:annotatedSource rdf:resource="http://purl.obolibrary.org/obo/ENVO_01001063"/>
        <owl:annotatedProperty rdf:resource="http://purl.obolibrary.org/obo/IAO_0000115"/>
        <owl:annotatedTarget>Water which has an appreciable concentration of dissolved oxygen.</owl:annotatedTarget>
        <oboInOwl:hasDbXref rdf:datatype="http://www.w3.org/2001/XMLSchema#string">ORCID:0000-0002-4366-3088</oboInOwl:hasDbXref>
        <oboInOwl:hasDbXref>https://en.wikipedia.org/wiki/Hypoxia_(environmental)</oboInOwl:hasDbXref>
    </owl:Axiom>
    


    <!-- http://purl.obolibrary.org/obo/ENVO_01001064 -->

    <owl:Class rdf:about="http://purl.obolibrary.org/obo/ENVO_01001064">
        <rdfs:subClassOf rdf:resource="http://purl.obolibrary.org/obo/ENVO_00002006"/>
        <obo:IAO_0000111 xml:lang="en">hypoxic water</obo:IAO_0000111>
        <obo:IAO_0000115>Water which has low levels of dissolved oxygen.</obo:IAO_0000115>
        <oboInOwl:created_by rdf:datatype="http://www.w3.org/2001/XMLSchema#string">ORCID:0000-0002-4366-3088</oboInOwl:created_by>
        <oboInOwl:creation_date>2010-03-21T06:05:53Z</oboInOwl:creation_date>
        <oboInOwl:inSubset rdf:resource="http://bcodmo/sm#material"/>
        <oboInOwl:inSubset rdf:resource="http://bcodmo/sm#matrix"/>
        <rdfs:comment>As with oxic and anoxic water, the thresholds for hypoxia are variable. Typically, a hypoxic state is asserted when dissolved oxygen levels decrease to a level where they have detrimental effects on aerobic aquatic organisms, typically below 30% oxygen saturation.</rdfs:comment>
        <rdfs:label xml:lang="en">hypoxic water</rdfs:label>
    </owl:Class>
    <owl:Axiom>
        <owl:annotatedSource rdf:resource="http://purl.obolibrary.org/obo/ENVO_01001064"/>
        <owl:annotatedProperty rdf:resource="http://purl.obolibrary.org/obo/IAO_0000115"/>
        <owl:annotatedTarget>Water which has low levels of dissolved oxygen.</owl:annotatedTarget>
        <oboInOwl:hasDbXref rdf:datatype="http://www.w3.org/2001/XMLSchema#string">ORCID:0000-0002-4366-3088</oboInOwl:hasDbXref>
        <oboInOwl:hasDbXref>https://en.wikipedia.org/wiki/Hypoxia_(environmental)</oboInOwl:hasDbXref>
    </owl:Axiom>
    


    <!-- http://purl.obolibrary.org/obo/ENVO_01001103 -->

    <owl:Class rdf:about="http://purl.obolibrary.org/obo/ENVO_01001103">
        <rdfs:subClassOf rdf:resource="http://purl.obolibrary.org/obo/ENVO_01000155"/>
        <obo:IAO_0000111 xml:lang="en">detritus</obo:IAO_0000111>
        <obo:IAO_0000115 xml:lang="en">An organic material which is primarily composed of dead particulate matter.</obo:IAO_0000115>
        <oboInOwl:inSubset rdf:resource="http://bcodmo/sm#material"/>
        <oboInOwl:inSubset rdf:resource="http://bcodmo/sm#matrix"/>
        <rdfs:label>detritus</rdfs:label>
        <rdfs:label xml:lang="en">detritus</rdfs:label>
    </owl:Class>
    <owl:Axiom>
        <owl:annotatedSource rdf:resource="http://purl.obolibrary.org/obo/ENVO_01001103"/>
        <owl:annotatedProperty rdf:resource="http://purl.obolibrary.org/obo/IAO_0000115"/>
        <owl:annotatedTarget xml:lang="en">An organic material which is primarily composed of dead particulate matter.</owl:annotatedTarget>
        <oboInOwl:hasDbXref>https://en.wikipedia.org/wiki/Detritus</oboInOwl:hasDbXref>
    </owl:Axiom>
    


    <!-- http://purl.obolibrary.org/obo/ENVO_01001121 -->

    <owl:Class rdf:about="http://purl.obolibrary.org/obo/ENVO_01001121">
        <rdfs:subClassOf rdf:resource="http://purl.obolibrary.org/obo/ENVO_01000155"/>
        <obo:IAO_0000111 xml:lang="en">plant matter</obo:IAO_0000111>
        <obo:IAO_0000115>Organic material which is primarily composed of plant structures, living or dead.</obo:IAO_0000115>
        <oboInOwl:inSubset rdf:resource="http://bcodmo/sm#material"/>
        <oboInOwl:inSubset rdf:resource="http://bcodmo/sm#matrix"/>
        <rdfs:label xml:lang="en">plant matter</rdfs:label>
    </owl:Class>
    


    <!-- http://purl.obolibrary.org/obo/ENVO_01001139 -->

    <owl:Class rdf:about="http://purl.obolibrary.org/obo/ENVO_01001139">
        <rdfs:subClassOf rdf:resource="http://purl.obolibrary.org/obo/ENVO_01000277"/>
        <obo:IAO_0000111 xml:lang="en">methane ice</obo:IAO_0000111>
        <obo:IAO_0000115>Ice which is primarily composed of methane.</obo:IAO_0000115>
        <oboInOwl:inSubset rdf:resource="http://bcodmo/sm#material"/>
        <oboInOwl:inSubset rdf:resource="http://bcodmo/sm#matrix"/>
        <oboInOwl:inSubset>envoAstro</oboInOwl:inSubset>
        <rdfs:label xml:lang="en">methane ice</rdfs:label>
    </owl:Class>
    <owl:Axiom>
        <owl:annotatedSource rdf:resource="http://purl.obolibrary.org/obo/ENVO_01001139"/>
        <owl:annotatedProperty rdf:resource="http://purl.obolibrary.org/obo/IAO_0000115"/>
        <owl:annotatedTarget>Ice which is primarily composed of methane.</owl:annotatedTarget>
        <oboInOwl:hasDbXref rdf:datatype="http://www.w3.org/2001/XMLSchema#string">https://en.wikipedia.org/wiki/Ice</oboInOwl:hasDbXref>
    </owl:Axiom>
    


    <!-- http://purl.obolibrary.org/obo/ENVO_01001189 -->

    <owl:Class rdf:about="http://purl.obolibrary.org/obo/ENVO_01001189">
        <rdfs:subClassOf rdf:resource="http://purl.obolibrary.org/obo/ENVO_01000155"/>
        <obo:IAO_0000111 xml:lang="en">algal material</obo:IAO_0000111>
        <obo:IAO_0000116>This class will be axiomatised with &quot;alga&quot; once an approach to handle this term&apos;s ambiguous semantics has been agreed with PCO.</obo:IAO_0000116>
        <oboInOwl:inSubset rdf:resource="http://bcodmo/sm#material"/>
        <oboInOwl:inSubset rdf:resource="http://bcodmo/sm#matrix"/>
        <rdfs:comment>An organic material which is primarily composed of living or dead algae, along with their exudates.</rdfs:comment>
        <rdfs:label xml:lang="en">algal material</rdfs:label>
    </owl:Class>
    <owl:Axiom>
        <owl:annotatedSource rdf:resource="http://purl.obolibrary.org/obo/ENVO_01001189"/>
        <owl:annotatedProperty rdf:resource="http://www.w3.org/2000/01/rdf-schema#comment"/>
        <owl:annotatedTarget>An organic material which is primarily composed of living or dead algae, along with their exudates.</owl:annotatedTarget>
        <oboInOwl:hasDbXref>https://en.wikipedia.org/wiki/Algae</oboInOwl:hasDbXref>
    </owl:Axiom>
    


    <!-- http://purl.obolibrary.org/obo/ENVO_01001190 -->

    <owl:Class rdf:about="http://purl.obolibrary.org/obo/ENVO_01001190">
        <rdfs:subClassOf rdf:resource="http://purl.obolibrary.org/obo/ENVO_00002200"/>
        <obo:IAO_0000111 xml:lang="en">brown sea ice</obo:IAO_0000111>
        <obo:IAO_0000115>Sea ice which has a brown colouration, either due to 1) the presence of pigments which are or were contained in the members of ecological assemblages, such as algal communities, living or trapped within the ice or 2) due to the presence of trapped sediments.</obo:IAO_0000115>
        <oboInOwl:hasExactSynonym>brownish colored sea ice</oboInOwl:hasExactSynonym>
        <oboInOwl:inSubset rdf:resource="http://bcodmo/sm#material"/>
        <oboInOwl:inSubset rdf:resource="http://bcodmo/sm#matrix"/>
        <rdfs:label xml:lang="en">brown sea ice</rdfs:label>
    </owl:Class>
    <owl:Axiom>
        <owl:annotatedSource rdf:resource="http://purl.obolibrary.org/obo/ENVO_01001190"/>
        <owl:annotatedProperty rdf:resource="http://purl.obolibrary.org/obo/IAO_0000115"/>
        <owl:annotatedTarget>Sea ice which has a brown colouration, either due to 1) the presence of pigments which are or were contained in the members of ecological assemblages, such as algal communities, living or trapped within the ice or 2) due to the presence of trapped sediments.</owl:annotatedTarget>
        <oboInOwl:hasDbXref>http://dx.doi.org/10.1016/j.csr.2017.04.010</oboInOwl:hasDbXref>
        <oboInOwl:hasDbXref>http://dx.doi.org/10.1038/nrmicro3522</oboInOwl:hasDbXref>
        <oboInOwl:hasDbXref>http://dx.doi.org/10.1371/journal.pone.0122418</oboInOwl:hasDbXref>
        <oboInOwl:hasDbXref>https://github.com/EnvironmentOntology/envo/issues/564</oboInOwl:hasDbXref>
    </owl:Axiom>
    


    <!-- http://purl.obolibrary.org/obo/ENVO_01001231 -->

    <owl:Class rdf:about="http://purl.obolibrary.org/obo/ENVO_01001231">
        <rdfs:subClassOf rdf:resource="http://purl.obolibrary.org/obo/ENVO_01000155"/>
        <obo:IAO_0000111 xml:lang="en">kerogen</obo:IAO_0000111>
        <obo:IAO_0000115>Organic material which is in a solid phase and contained in sedimentary rock.</obo:IAO_0000115>
        <oboInOwl:inSubset rdf:resource="http://bcodmo/sm#material"/>
        <oboInOwl:inSubset rdf:resource="http://bcodmo/sm#matrix"/>
        <rdfs:label xml:lang="en">kerogen</rdfs:label>
    </owl:Class>
    <owl:Axiom>
        <owl:annotatedSource rdf:resource="http://purl.obolibrary.org/obo/ENVO_01001231"/>
        <owl:annotatedProperty rdf:resource="http://purl.obolibrary.org/obo/IAO_0000115"/>
        <owl:annotatedTarget>Organic material which is in a solid phase and contained in sedimentary rock.</owl:annotatedTarget>
        <oboInOwl:hasDbXref>https://en.wikipedia.org/wiki/Kerogen</oboInOwl:hasDbXref>
    </owl:Axiom>
    


    <!-- http://purl.obolibrary.org/obo/ENVO_01001267 -->

    <owl:Class rdf:about="http://purl.obolibrary.org/obo/ENVO_01001267">
        <rdfs:subClassOf rdf:resource="http://purl.obolibrary.org/obo/ENVO_00002006"/>
        <obo:IAO_0000111 xml:lang="en">stormwater</obo:IAO_0000111>
        <obo:IAO_0000115>Water which accumulates on a solid surface during precipitation events and snow/ice melt.</obo:IAO_0000115>
        <oboInOwl:hasExactSynonym>storm water</oboInOwl:hasExactSynonym>
        <oboInOwl:inSubset rdf:resource="http://bcodmo/sm#material"/>
        <oboInOwl:inSubset rdf:resource="http://bcodmo/sm#matrix"/>
        <rdfs:comment>&quot;Stormwater can soak into the soil (infiltrate), be held on the surface and evaporate, or runoff and end up in nearby streams, rivers, or other water bodies (surface water).&quot;</rdfs:comment>
        <rdfs:label xml:lang="en">stormwater</rdfs:label>
    </owl:Class>
    <owl:Axiom>
        <owl:annotatedSource rdf:resource="http://purl.obolibrary.org/obo/ENVO_01001267"/>
        <owl:annotatedProperty rdf:resource="http://purl.obolibrary.org/obo/IAO_0000115"/>
        <owl:annotatedTarget>Water which accumulates on a solid surface during precipitation events and snow/ice melt.</owl:annotatedTarget>
        <oboInOwl:hasDbXref>https://en.wikipedia.org/wiki/Stormwater</oboInOwl:hasDbXref>
    </owl:Axiom>
    <owl:Axiom>
        <owl:annotatedSource rdf:resource="http://purl.obolibrary.org/obo/ENVO_01001267"/>
        <owl:annotatedProperty rdf:resource="http://www.w3.org/2000/01/rdf-schema#comment"/>
        <owl:annotatedTarget>&quot;Stormwater can soak into the soil (infiltrate), be held on the surface and evaporate, or runoff and end up in nearby streams, rivers, or other water bodies (surface water).&quot;</owl:annotatedTarget>
        <oboInOwl:hasDbXref>https://en.wikipedia.org/wiki/Stormwater</oboInOwl:hasDbXref>
    </owl:Axiom>
    


    <!-- http://purl.obolibrary.org/obo/ENVO_01001395 -->

    <owl:Class rdf:about="http://purl.obolibrary.org/obo/ENVO_01001395">
        <rdfs:subClassOf rdf:resource="http://purl.obolibrary.org/obo/ENVO_01000155"/>
        <obo:IAO_0000111 xml:lang="en">necromass</obo:IAO_0000111>
        <obo:IAO_0000115>Biomass which is composed primarily of dead organisms, their parts, or their organic derivatives.</obo:IAO_0000115>
        <oboInOwl:created_by rdf:resource="http://orcid.org/0000-0002-4366-3088"/>
        <oboInOwl:hasExactSynonym>dead biological matter</oboInOwl:hasExactSynonym>
        <oboInOwl:hasExactSynonym>dead biomass</oboInOwl:hasExactSynonym>
        <oboInOwl:inSubset rdf:resource="http://bcodmo/sm#material"/>
        <oboInOwl:inSubset rdf:resource="http://bcodmo/sm#matrix"/>
        <rdfs:label xml:lang="en">necromass</rdfs:label>
    </owl:Class>
    


    <!-- http://purl.obolibrary.org/obo/ENVO_01001402 -->

    <owl:Class rdf:about="http://purl.obolibrary.org/obo/ENVO_01001402">
        <rdfs:subClassOf rdf:resource="http://purl.obolibrary.org/obo/ENVO_00010505"/>
        <obo:IAO_0000111 xml:lang="en">haze</obo:IAO_0000111>
        <obo:IAO_0000115>An aersolised mass of dust, smoke, or other dry particulates which scatters visible light thus obsscuring visibility through an atmosphere.</obo:IAO_0000115>
        <oboInOwl:created_by rdf:resource="http://orcid.org/0000-0002-4366-3088"/>
        <oboInOwl:inSubset rdf:resource="http://bcodmo/sm#material"/>
        <oboInOwl:inSubset rdf:resource="http://bcodmo/sm#matrix"/>
        <oboInOwl:inSubset>envoAtmo</oboInOwl:inSubset>
        <rdfs:label xml:lang="en">haze</rdfs:label>
    </owl:Class>
    <owl:Axiom>
        <owl:annotatedSource rdf:resource="http://purl.obolibrary.org/obo/ENVO_01001402"/>
        <owl:annotatedProperty rdf:resource="http://purl.obolibrary.org/obo/IAO_0000115"/>
        <owl:annotatedTarget>An aersolised mass of dust, smoke, or other dry particulates which scatters visible light thus obsscuring visibility through an atmosphere.</owl:annotatedTarget>
        <oboInOwl:hasDbXref>https://en.wikipedia.org/wiki/Haze</oboInOwl:hasDbXref>
    </owl:Axiom>
    


    <!-- http://purl.obolibrary.org/obo/ENVO_01001428 -->

    <owl:Class rdf:about="http://purl.obolibrary.org/obo/ENVO_01001428">
        <rdfs:subClassOf rdf:resource="http://purl.obolibrary.org/obo/ENVO_00010505"/>
        <obo:IAO_0000111 xml:lang="en">cloud</obo:IAO_0000111>
        <obo:IAO_0000115>A cloud which is primarily composed of water-based aerosols.</obo:IAO_0000115>
        <oboInOwl:created_by rdf:resource="http://orcid.org/0000-0002-4366-3088"/>
        <oboInOwl:hasBroadSynonym>cloud mass</oboInOwl:hasBroadSynonym>
        <oboInOwl:inSubset rdf:resource="http://bcodmo/sm#material"/>
        <oboInOwl:inSubset rdf:resource="http://bcodmo/sm#matrix"/>
        <oboInOwl:inSubset>envoAtmo</oboInOwl:inSubset>
        <rdfs:comment>On Earth clouds are formed by the saturation of air in the homosphere when air cools or gains water vapor. Note that this class describes clouds as countable objects, rather than &apos;cloud material&apos;. It also refers only to clouds made up of a water-based material.</rdfs:comment>
        <rdfs:label xml:lang="en">cloud</rdfs:label>
        <rdfs:label xml:lang="en">water-based cloud</rdfs:label>
    </owl:Class>
    <owl:Axiom>
        <owl:annotatedSource rdf:resource="http://purl.obolibrary.org/obo/ENVO_01001428"/>
        <owl:annotatedProperty rdf:resource="http://purl.obolibrary.org/obo/IAO_0000115"/>
        <owl:annotatedTarget>A cloud which is primarily composed of water-based aerosols.</owl:annotatedTarget>
        <oboInOwl:hasDbXref>https://cloudatlas.wmo.int/introduction-and-principles-of-cloud-classification.html</oboInOwl:hasDbXref>
        <oboInOwl:hasDbXref>https://en.wikipedia.org/wiki/Cloud</oboInOwl:hasDbXref>
    </owl:Axiom>
    


    <!-- http://purl.obolibrary.org/obo/ENVO_01001458 -->

    <owl:Class rdf:about="http://purl.obolibrary.org/obo/ENVO_01001458">
        <rdfs:subClassOf rdf:resource="http://purl.obolibrary.org/obo/ENVO_00010505"/>
        <obo:IAO_0000111 xml:lang="en">mist</obo:IAO_0000111>
        <obo:IAO_0000115>A visible mass of water droplets or ice crystals suspended in the air at or near a planetary surface, formed when humid air cools rapidly.</obo:IAO_0000115>
        <oboInOwl:created_by rdf:resource="http://orcid.org/0000-0002-4366-3088"/>
        <oboInOwl:inSubset rdf:resource="http://bcodmo/sm#material"/>
        <oboInOwl:inSubset rdf:resource="http://bcodmo/sm#matrix"/>
        <rdfs:comment>This class refers only to mist formed by materials primarily composed of water. Mist is less dense than fog, and visibility is typically greater than one kilometre.</rdfs:comment>
        <rdfs:label xml:lang="en">mist</rdfs:label>
    </owl:Class>
    <owl:Axiom>
        <owl:annotatedSource rdf:resource="http://purl.obolibrary.org/obo/ENVO_01001458"/>
        <owl:annotatedProperty rdf:resource="http://purl.obolibrary.org/obo/IAO_0000115"/>
        <owl:annotatedTarget>A visible mass of water droplets or ice crystals suspended in the air at or near a planetary surface, formed when humid air cools rapidly.</owl:annotatedTarget>
        <oboInOwl:hasDbXref>https://en.wikipedia.org/wiki/Mist</oboInOwl:hasDbXref>
    </owl:Axiom>
    


    <!-- http://purl.obolibrary.org/obo/ENVO_01001511 -->

    <owl:Class rdf:about="http://purl.obolibrary.org/obo/ENVO_01001511">
        <rdfs:subClassOf rdf:resource="http://purl.obolibrary.org/obo/ENVO_01000277"/>
        <obo:IAO_0000111 xml:lang="en">freshwater ice</obo:IAO_0000111>
        <oboInOwl:created_by rdf:resource="http://orcid.org/0000-0002-4366-3088"/>
        <oboInOwl:creation_date rdf:datatype="http://www.w3.org/2001/XMLSchema#dateTime">2019-01-14T18:55:42Z</oboInOwl:creation_date>
        <oboInOwl:inSubset rdf:resource="http://bcodmo/sm#material"/>
        <oboInOwl:inSubset rdf:resource="http://bcodmo/sm#matrix"/>
        <rdfs:comment>Water ice which is formed by the freezing of fresh water.</rdfs:comment>
        <rdfs:label xml:lang="en">freshwater ice</rdfs:label>
    </owl:Class>
    


    <!-- http://purl.obolibrary.org/obo/ENVO_01001512 -->

    <owl:Class rdf:about="http://purl.obolibrary.org/obo/ENVO_01001512">
        <rdfs:subClassOf rdf:resource="http://purl.obolibrary.org/obo/ENVO_00002200"/>
        <obo:IAO_0000111 xml:lang="en">congelation sea ice</obo:IAO_0000111>
        <obo:IAO_0000115>Sea ice which 1) has formed on the submerged surface (i.e. the base) of an existing mass of sea ice and 2) is composed of columnar crystals due to the downward growth of the crystals into the water.</obo:IAO_0000115>
        <oboInOwl:created_by rdf:resource="http://orcid.org/0000-0002-4366-3088"/>
        <oboInOwl:creation_date rdf:datatype="http://www.w3.org/2001/XMLSchema#dateTime">2019-01-14T18:56:29Z</oboInOwl:creation_date>
        <oboInOwl:hasDbXref rdf:resource="http://sweetontology.net/realmCryo/CongelationIce"/>
        <oboInOwl:hasRelatedSynonym>black ice</oboInOwl:hasRelatedSynonym>
        <oboInOwl:inSubset rdf:resource="http://bcodmo/sm#material"/>
        <oboInOwl:inSubset rdf:resource="http://bcodmo/sm#matrix"/>
        <rdfs:comment>Congelation ice usually forms through the fusion/coalescence of platelets into solid ice.</rdfs:comment>
        <rdfs:label xml:lang="en">congelation sea ice</rdfs:label>
    </owl:Class>
    <owl:Axiom>
        <owl:annotatedSource rdf:resource="http://purl.obolibrary.org/obo/ENVO_01001512"/>
        <owl:annotatedProperty rdf:resource="http://purl.obolibrary.org/obo/IAO_0000115"/>
        <owl:annotatedTarget>Sea ice which 1) has formed on the submerged surface (i.e. the base) of an existing mass of sea ice and 2) is composed of columnar crystals due to the downward growth of the crystals into the water.</owl:annotatedTarget>
        <oboInOwl:hasDbXref>https://en.wikipedia.org/wiki/Congelation_ice</oboInOwl:hasDbXref>
        <oboInOwl:hasDbXref>https://orcid.org/0000-0003-4808-4736</oboInOwl:hasDbXref>
    </owl:Axiom>
    <owl:Axiom>
        <owl:annotatedSource rdf:resource="http://purl.obolibrary.org/obo/ENVO_01001512"/>
        <owl:annotatedProperty rdf:resource="http://www.geneontology.org/formats/oboInOwl#hasRelatedSynonym"/>
        <owl:annotatedTarget>black ice</owl:annotatedTarget>
        <rdfs:comment>Common in limnology, but frequently used in other contexts (e.g. on roads).</rdfs:comment>
    </owl:Axiom>
    


    <!-- http://purl.obolibrary.org/obo/ENVO_01001523 -->

    <owl:Class rdf:about="http://purl.obolibrary.org/obo/ENVO_01001523">
        <rdfs:subClassOf rdf:resource="http://purl.obolibrary.org/obo/ENVO_03000063"/>
        <obo:IAO_0000111 xml:lang="en">frazil</obo:IAO_0000111>
        <obo:IAO_0000115>Small, needle-like (spicules), plate-like, or discoid crystals derived from nearly pure fresh water, suspended in a water body.</obo:IAO_0000115>
        <obo:IAO_0000116>Needs to have axioms added pertaining to the semantics of colloids and suspensions once they have been resolved see: https://github.com/pato-ontology/pato/issues/91#issuecomment-290711238

Currently the new ice classes are not specific to sea water as they may form in non marine systems, but it would be good to confirm this especially for frazil ice.</obo:IAO_0000116>
        <oboInOwl:created_by rdf:resource="http://orcid.org/0000-0002-4366-3088"/>
        <oboInOwl:creation_date rdf:datatype="http://www.w3.org/2001/XMLSchema#dateTime">2019-01-14T21:09:21Z</oboInOwl:creation_date>
        <oboInOwl:hasExactSynonym>frazil crystals</oboInOwl:hasExactSynonym>
        <oboInOwl:hasExactSynonym>needle ice</oboInOwl:hasExactSynonym>
        <oboInOwl:inSubset rdf:resource="http://bcodmo/sm#material"/>
        <oboInOwl:inSubset rdf:resource="http://bcodmo/sm#matrix"/>
        <oboInOwl:inSubset>envoPolar</oboInOwl:inSubset>
        <rdfs:comment>Typically 3 to 4 millimeters in diameter. These may form in both marine water and fresh water. They represent the first stages of sea ice growth; they merge under calm conditions to form thin sheets of ice on the surface (frazil ice), and consist of nearly pure fresh water. In fresh water, they form in supercooled water that is too turbulent to permit coagulation into sheet ice.  This is most common in swiftly flowing streams. They may accumulate as anchor ice on submerged objects obstructing the water flow.</rdfs:comment>
        <rdfs:label xml:lang="en">frazil</rdfs:label>
    </owl:Class>
    <owl:Axiom>
        <owl:annotatedSource rdf:resource="http://purl.obolibrary.org/obo/ENVO_01001523"/>
        <owl:annotatedProperty rdf:resource="http://purl.obolibrary.org/obo/IAO_0000115"/>
        <owl:annotatedTarget>Small, needle-like (spicules), plate-like, or discoid crystals derived from nearly pure fresh water, suspended in a water body.</owl:annotatedTarget>
        <oboInOwl:hasDbXref>https://nsidc.org/cryosphere/glossary/term/frazil</oboInOwl:hasDbXref>
    </owl:Axiom>
    <owl:Axiom>
        <owl:annotatedSource rdf:resource="http://purl.obolibrary.org/obo/ENVO_01001523"/>
        <owl:annotatedProperty rdf:resource="http://www.w3.org/2000/01/rdf-schema#comment"/>
        <owl:annotatedTarget>Typically 3 to 4 millimeters in diameter. These may form in both marine water and fresh water. They represent the first stages of sea ice growth; they merge under calm conditions to form thin sheets of ice on the surface (frazil ice), and consist of nearly pure fresh water. In fresh water, they form in supercooled water that is too turbulent to permit coagulation into sheet ice.  This is most common in swiftly flowing streams. They may accumulate as anchor ice on submerged objects obstructing the water flow.</owl:annotatedTarget>
        <oboInOwl:hasDbXref>https://orcid.org/0000-0003-4808-4736</oboInOwl:hasDbXref>
    </owl:Axiom>
    


    <!-- http://purl.obolibrary.org/obo/ENVO_01001614 -->

    <owl:Class rdf:about="http://purl.obolibrary.org/obo/ENVO_01001614">
        <rdfs:subClassOf rdf:resource="http://purl.obolibrary.org/obo/ENVO_00000134"/>
        <obo:IAO_0000111 xml:lang="en">ice permafrost</obo:IAO_0000111>
        <obo:IAO_0000115>Permafrost which contains inclusions of water-based ice.</obo:IAO_0000115>
        <dc:creator rdf:resource="http://orcid.org/0000-0002-4366-3088"/>
        <oboInOwl:creation_date rdf:datatype="http://www.w3.org/2001/XMLSchema#dateTime">2019-04-09T13:45:40Z</oboInOwl:creation_date>
        <oboInOwl:inSubset rdf:resource="http://bcodmo/sm#material"/>
        <oboInOwl:inSubset rdf:resource="http://bcodmo/sm#matrix"/>
        <rdfs:label xml:lang="en">ice permafrost</rdfs:label>
        <rdfs:label xml:lang="en">ice-bearing permafrost</rdfs:label>
    </owl:Class>
    


    <!-- http://purl.obolibrary.org/obo/ENVO_01001850 -->

    <owl:Class rdf:about="http://purl.obolibrary.org/obo/ENVO_01001850">
        <obo:IAO_0000111 xml:lang="en">frost</obo:IAO_0000111>
        <obo:IAO_0000115>An environmental material which is primarily composed of minute ice crystals covering a cold surface.</obo:IAO_0000115>
        <dc:creator rdf:resource="http://orcid.org/0000-0002-4366-3088"/>
        <dc:date rdf:datatype="http://www.w3.org/2001/XMLSchema#dateTime">2020-02-12T21:05:54Z</dc:date>
        <oboInOwl:inSubset rdf:resource="http://bcodmo/sm#material"/>
        <oboInOwl:inSubset rdf:resource="http://bcodmo/sm#matrix"/>
        <rdfs:label xml:lang="en">frost</rdfs:label>
    </owl:Class>
    <owl:Axiom>
        <owl:annotatedSource rdf:resource="http://purl.obolibrary.org/obo/ENVO_01001850"/>
        <owl:annotatedProperty rdf:resource="http://purl.obolibrary.org/obo/IAO_0000115"/>
        <owl:annotatedTarget>An environmental material which is primarily composed of minute ice crystals covering a cold surface.</owl:annotatedTarget>
        <oboInOwl:hasDbXref rdf:resource="https://www.merriam-webster.com/dictionary/frost"/>
    </owl:Axiom>
    


    <!-- http://purl.obolibrary.org/obo/ENVO_02000008 -->

    <owl:Class rdf:about="http://purl.obolibrary.org/obo/ENVO_02000008">
        <rdfs:subClassOf rdf:resource="http://purl.obolibrary.org/obo/BSM_0100004"/>
        <obo:IAO_0000111 xml:lang="en">cell culture</obo:IAO_0000111>
        <obo:IAO_0000115>A cell culture is a growth of cells in vitro in an artificial medium for experimental research.</obo:IAO_0000115>
        <oboInOwl:hasDbXref>https://en.wikipedia.org/wiki/Cell_culture</oboInOwl:hasDbXref>
        <oboInOwl:inSubset rdf:resource="http://bcodmo/sm#material"/>
        <oboInOwl:inSubset rdf:resource="http://bcodmo/sm#matrix"/>
        <rdfs:label>cell culture</rdfs:label>
        <rdfs:label xml:lang="en">cell culture</rdfs:label>
    </owl:Class>
    <owl:Axiom>
        <owl:annotatedSource rdf:resource="http://purl.obolibrary.org/obo/ENVO_02000008"/>
        <owl:annotatedProperty rdf:resource="http://purl.obolibrary.org/obo/IAO_0000115"/>
        <owl:annotatedTarget>A cell culture is a growth of cells in vitro in an artificial medium for experimental research.</owl:annotatedTarget>
        <oboInOwl:hasDbXref>URL:http://stemcells.nih.gov/StemCells/Templates/StemCellContentPage.aspx?NRMODE=Published&amp;NRNODEGUID=%7b3C35BAB6-0FE6-4C4E-95F2-2CB61B58D96D%7d&amp;NRORIGINALURL=%2finfo%2fglossary%2easp&amp;NRCACHEHINT=NoModifyGuest#cellculture</oboInOwl:hasDbXref>
    </owl:Axiom>
    


    <!-- http://purl.obolibrary.org/obo/ENVO_02000090 -->

    <owl:Class rdf:about="http://purl.obolibrary.org/obo/ENVO_02000090">
        <obo:IAO_0000111 xml:lang="en">ash</obo:IAO_0000111>
        <obo:IAO_0000115>An environmental material that is the non-aqueous, non-gaseous residues that remain after something is burned.</obo:IAO_0000115>
        <oboInOwl:inSubset rdf:resource="http://bcodmo/sm#material"/>
        <oboInOwl:inSubset rdf:resource="http://bcodmo/sm#matrix"/>
        <rdfs:label xml:lang="en">ash</rdfs:label>
    </owl:Class>
    <owl:Axiom>
        <owl:annotatedSource rdf:resource="http://purl.obolibrary.org/obo/ENVO_02000090"/>
        <owl:annotatedProperty rdf:resource="http://purl.obolibrary.org/obo/IAO_0000115"/>
        <owl:annotatedTarget>An environmental material that is the non-aqueous, non-gaseous residues that remain after something is burned.</owl:annotatedTarget>
        <oboInOwl:hasDbXref>https://en.wikipedia.org/wiki/Ash</oboInOwl:hasDbXref>
    </owl:Axiom>
    


    <!-- http://purl.obolibrary.org/obo/ENVO_03000000 -->

    <owl:Class rdf:about="http://purl.obolibrary.org/obo/ENVO_03000000">
        <rdfs:subClassOf rdf:resource="http://purl.obolibrary.org/obo/ENVO_01000406"/>
        <obo:IAO_0000111 xml:lang="en">neve</obo:IAO_0000111>
        <obo:IAO_0000115>Partially compacted granular snow, which has undergone several cycles of melting and refreezing while being compacted, usually found on the atmosphere-exposed surface of a glacier.</obo:IAO_0000115>
        <obo:IAO_0000117 rdf:resource="http://orcid.org/0000-0002-4366-3088"/>
        <obo:IAO_0000117>http://orcid.org/0000-0002-3410-4655</obo:IAO_0000117>
        <oboInOwl:hasExactSynonym>névé</oboInOwl:hasExactSynonym>
        <oboInOwl:inSubset rdf:resource="http://bcodmo/sm#material"/>
        <oboInOwl:inSubset rdf:resource="http://bcodmo/sm#matrix"/>
        <oboInOwl:inSubset>envoPolar</oboInOwl:inSubset>
        <rdfs:comment>Névé that survives a full season of ablation turns into firn.</rdfs:comment>
        <rdfs:label xml:lang="en">neve</rdfs:label>
    </owl:Class>
    <owl:Axiom>
        <owl:annotatedSource rdf:resource="http://purl.obolibrary.org/obo/ENVO_03000000"/>
        <owl:annotatedProperty rdf:resource="http://purl.obolibrary.org/obo/IAO_0000115"/>
        <owl:annotatedTarget>Partially compacted granular snow, which has undergone several cycles of melting and refreezing while being compacted, usually found on the atmosphere-exposed surface of a glacier.</owl:annotatedTarget>
        <oboInOwl:hasDbXref>https://en.wikipedia.org/wiki/N%C3%A9v%C3%A9</oboInOwl:hasDbXref>
    </owl:Axiom>
    


    <!-- http://purl.obolibrary.org/obo/ENVO_03000002 -->

    <owl:Class rdf:about="http://purl.obolibrary.org/obo/ENVO_03000002">
        <rdfs:subClassOf rdf:resource="http://purl.obolibrary.org/obo/ENVO_01000406"/>
        <obo:IAO_0000111 xml:lang="en">firn</obo:IAO_0000111>
        <obo:IAO_0000115>Granular snow which contains a proportion of fused granules formed through melting and re-thawing while being compacted by the weight of overlying material and which contains interconnected gaseous pores.</obo:IAO_0000115>
        <obo:IAO_0000117 rdf:resource="http://orcid.org/0000-0002-4366-3088"/>
        <obo:IAO_0000117>http://orcid.org/0000-0002-3410-4655</obo:IAO_0000117>
        <oboInOwl:inSubset rdf:resource="http://bcodmo/sm#material"/>
        <oboInOwl:inSubset rdf:resource="http://bcodmo/sm#matrix"/>
        <oboInOwl:inSubset>envoPolar</oboInOwl:inSubset>
        <rdfs:comment>Firn derives from névé which has survived a full season of ablation and has undergone a metamorphic transition.</rdfs:comment>
        <rdfs:label xml:lang="en">firn</rdfs:label>
    </owl:Class>
    <owl:Axiom>
        <owl:annotatedSource rdf:resource="http://purl.obolibrary.org/obo/ENVO_03000002"/>
        <owl:annotatedProperty rdf:resource="http://purl.obolibrary.org/obo/IAO_0000115"/>
        <owl:annotatedTarget>Granular snow which contains a proportion of fused granules formed through melting and re-thawing while being compacted by the weight of overlying material and which contains interconnected gaseous pores.</owl:annotatedTarget>
        <oboInOwl:hasDbXref>https://en.wikipedia.org/wiki/Firn</oboInOwl:hasDbXref>
    </owl:Axiom>
    


    <!-- http://purl.obolibrary.org/obo/ENVO_03000004 -->

    <owl:Class rdf:about="http://purl.obolibrary.org/obo/ENVO_03000004">
        <rdfs:subClassOf rdf:resource="http://purl.obolibrary.org/obo/ENVO_01000277"/>
        <obo:IAO_0000111 xml:lang="en">glacial ice</obo:IAO_0000111>
        <obo:IAO_0000115>Any water ice that is part of a glacier.</obo:IAO_0000115>
        <obo:IAO_0000116>It is suggested that users complement this term with ice terms that are more descriptive of the ice itself, rather than its location/parthood.</obo:IAO_0000116>
        <obo:IAO_0000117 rdf:resource="http://orcid.org/0000-0002-4366-3088"/>
        <obo:IAO_0000117>http://orcid.org/0000-0002-3410-4655</obo:IAO_0000117>
        <oboInOwl:inSubset rdf:resource="http://bcodmo/sm#material"/>
        <oboInOwl:inSubset rdf:resource="http://bcodmo/sm#matrix"/>
        <oboInOwl:inSubset>envoPolar</oboInOwl:inSubset>
        <rdfs:label xml:lang="en">glacial ice</rdfs:label>
    </owl:Class>
    <owl:Axiom>
        <owl:annotatedSource rdf:resource="http://purl.obolibrary.org/obo/ENVO_03000004"/>
        <owl:annotatedProperty rdf:resource="http://purl.obolibrary.org/obo/IAO_0000115"/>
        <owl:annotatedTarget>Any water ice that is part of a glacier.</owl:annotatedTarget>
        <oboInOwl:hasDbXref>https://en.wikipedia.org/wiki/Glacier</oboInOwl:hasDbXref>
    </owl:Axiom>
    


    <!-- http://purl.obolibrary.org/obo/ENVO_03000007 -->

    <owl:Class rdf:about="http://purl.obolibrary.org/obo/ENVO_03000007">
        <rdfs:subClassOf rdf:resource="http://purl.obolibrary.org/obo/ENVO_01000277"/>
        <obo:IAO_0000111 xml:lang="en">blue ice</obo:IAO_0000111>
        <obo:IAO_0000115>Water ice containing little to no air bubbles resulting in a reduction of internal light scattering and, given sufficient volume, a blue appearance.</obo:IAO_0000115>
        <obo:IAO_0000117 rdf:resource="http://orcid.org/0000-0002-4366-3088"/>
        <obo:IAO_0000117>http://orcid.org/0000-0002-3410-4655</obo:IAO_0000117>
        <oboInOwl:inSubset rdf:resource="http://bcodmo/sm#material"/>
        <oboInOwl:inSubset rdf:resource="http://bcodmo/sm#matrix"/>
        <oboInOwl:inSubset>envoPolar</oboInOwl:inSubset>
        <rdfs:comment>The blue &apos;appearance&apos; is to be understood as that within the visual range of humans.</rdfs:comment>
        <rdfs:label xml:lang="en">blue ice</rdfs:label>
    </owl:Class>
    <owl:Axiom>
        <owl:annotatedSource rdf:resource="http://purl.obolibrary.org/obo/ENVO_03000007"/>
        <owl:annotatedProperty rdf:resource="http://purl.obolibrary.org/obo/IAO_0000115"/>
        <owl:annotatedTarget>Water ice containing little to no air bubbles resulting in a reduction of internal light scattering and, given sufficient volume, a blue appearance.</owl:annotatedTarget>
        <oboInOwl:hasDbXref>https://en.wikipedia.org/wiki/Blue_ice_(glacial)</oboInOwl:hasDbXref>
        <oboInOwl:hasDbXref>https://en.wikipedia.org/wiki/Glacier</oboInOwl:hasDbXref>
    </owl:Axiom>
    


    <!-- http://purl.obolibrary.org/obo/ENVO_03000021 -->

    <owl:Class rdf:about="http://purl.obolibrary.org/obo/ENVO_03000021">
        <rdfs:subClassOf rdf:resource="http://purl.obolibrary.org/obo/ENVO_01000060"/>
        <obo:IAO_0000111 xml:lang="en">soot</obo:IAO_0000111>
        <obo:IAO_0000115>Particulate matter primarily composed of carbon particles formed through the incomplete combustion of hydrocarbons.</obo:IAO_0000115>
        <obo:IAO_0000117 rdf:resource="http://orcid.org/0000-0002-4366-3088"/>
        <obo:IAO_0000117>http://orcid.org/0000-0002-3410-4655</obo:IAO_0000117>
        <oboInOwl:inSubset rdf:resource="http://bcodmo/sm#material"/>
        <oboInOwl:inSubset rdf:resource="http://bcodmo/sm#matrix"/>
        <oboInOwl:inSubset>envoPolar</oboInOwl:inSubset>
        <rdfs:label xml:lang="en">soot</rdfs:label>
    </owl:Class>
    <owl:Axiom>
        <owl:annotatedSource rdf:resource="http://purl.obolibrary.org/obo/ENVO_03000021"/>
        <owl:annotatedProperty rdf:resource="http://purl.obolibrary.org/obo/IAO_0000115"/>
        <owl:annotatedTarget>Particulate matter primarily composed of carbon particles formed through the incomplete combustion of hydrocarbons.</owl:annotatedTarget>
        <oboInOwl:hasDbXref>https://en.wikipedia.org/wiki/Soot</oboInOwl:hasDbXref>
    </owl:Axiom>
    


    <!-- http://purl.obolibrary.org/obo/ENVO_03000027 -->

    <owl:Class rdf:about="http://purl.obolibrary.org/obo/ENVO_03000027">
        <rdfs:subClassOf rdf:resource="http://purl.obolibrary.org/obo/ENVO_01000406"/>
        <obo:IAO_0000111 xml:lang="en">powdery snow</obo:IAO_0000111>
        <obo:IAO_0000115>Uncompacted snow containing trapped atmospheric gases.</obo:IAO_0000115>
        <obo:IAO_0000117 rdf:resource="http://orcid.org/0000-0002-4366-3088"/>
        <obo:IAO_0000117>http://orcid.org/0000-0002-3410-4655</obo:IAO_0000117>
        <oboInOwl:inSubset rdf:resource="http://bcodmo/sm#material"/>
        <oboInOwl:inSubset rdf:resource="http://bcodmo/sm#matrix"/>
        <oboInOwl:inSubset>envoPolar</oboInOwl:inSubset>
        <rdfs:comment>Described as having a fluffy appearance.</rdfs:comment>
        <rdfs:label xml:lang="en">powdery snow</rdfs:label>
    </owl:Class>
    <owl:Axiom>
        <owl:annotatedSource rdf:resource="http://purl.obolibrary.org/obo/ENVO_03000027"/>
        <owl:annotatedProperty rdf:resource="http://purl.obolibrary.org/obo/IAO_0000115"/>
        <owl:annotatedTarget>Uncompacted snow containing trapped atmospheric gases.</owl:annotatedTarget>
        <oboInOwl:hasDbXref>https://en.wikipedia.org/wiki/Types_of_snow</oboInOwl:hasDbXref>
        <oboInOwl:hasDbXref>https://nsidc.org/cryosphere/snow/science/characteristics.html</oboInOwl:hasDbXref>
    </owl:Axiom>
    


    <!-- http://purl.obolibrary.org/obo/ENVO_03000033 -->

    <owl:Class rdf:about="http://purl.obolibrary.org/obo/ENVO_03000033">
        <rdfs:subClassOf rdf:resource="http://purl.obolibrary.org/obo/ENVO_00002007"/>
        <obo:IAO_0000111 xml:lang="en">marine sediment</obo:IAO_0000111>
        <obo:IAO_0000115>Sediment which has been transported through the marine water column, settling on the seafloor.</obo:IAO_0000115>
        <obo:IAO_0000117 rdf:resource="http://orcid.org/0000-0002-4366-3088"/>
        <obo:IAO_0000117>http://orcid.org/0000-0002-3410-4655</obo:IAO_0000117>
        <oboInOwl:hasExactSynonym>marine sediments</oboInOwl:hasExactSynonym>
        <oboInOwl:inSubset rdf:resource="http://bcodmo/sm#material"/>
        <oboInOwl:inSubset rdf:resource="http://bcodmo/sm#matrix"/>
        <oboInOwl:inSubset>envoPolar</oboInOwl:inSubset>
        <rdfs:comment>Particles of marine sediment are primarily generated by 1) processes in terrestrial systems and transported to the marine realm by the action of rivers or aeolian processes (amongst other routes) , 2) marine organisms, 3) chemical processes in seawater, or 4) cosmogeneous input.</rdfs:comment>
        <rdfs:label xml:lang="en">marine sediment</rdfs:label>
    </owl:Class>
    <owl:Axiom>
        <owl:annotatedSource rdf:resource="http://purl.obolibrary.org/obo/ENVO_03000033"/>
        <owl:annotatedProperty rdf:resource="http://purl.obolibrary.org/obo/IAO_0000115"/>
        <owl:annotatedTarget>Sediment which has been transported through the marine water column, settling on the seafloor.</owl:annotatedTarget>
        <oboInOwl:hasDbXref>https://en.wikipedia.org/wiki/Pelagic_sediment#_note-8</oboInOwl:hasDbXref>
    </owl:Axiom>
    


    <!-- http://purl.obolibrary.org/obo/ENVO_03000038 -->

    <owl:Class rdf:about="http://purl.obolibrary.org/obo/ENVO_03000038">
        <rdfs:subClassOf rdf:resource="http://purl.obolibrary.org/obo/ENVO_01000060"/>
        <obo:IAO_0000111 xml:lang="en">cryoconite</obo:IAO_0000111>
        <obo:IAO_0000115>Particulate matter which is composed primarily of dust, rock, and soot, as well as the microbial communities associated with these materials, deposited on an ice mass by an aeolian process.</obo:IAO_0000115>
        <obo:IAO_0000116>This actually is formed as a result of an accumulation process involving the constituents of cryoconite. When their semantics are more stable, we can axiomatise this fully.</obo:IAO_0000116>
        <obo:IAO_0000117 rdf:resource="http://orcid.org/0000-0002-4366-3088"/>
        <obo:IAO_0000117>http://orcid.org/0000-0001-5812-6405</obo:IAO_0000117>
        <obo:IAO_0000117>http://orcid.org/0000-0002-3410-4655</obo:IAO_0000117>
        <oboInOwl:inSubset rdf:resource="http://bcodmo/sm#material"/>
        <oboInOwl:inSubset rdf:resource="http://bcodmo/sm#matrix"/>
        <oboInOwl:inSubset>envoPolar</oboInOwl:inSubset>
        <rdfs:label xml:lang="en">cryoconite</rdfs:label>
        <rdfs:label xml:lang="en">cryoconite deposit</rdfs:label>
    </owl:Class>
    <owl:Axiom>
        <owl:annotatedSource rdf:resource="http://purl.obolibrary.org/obo/ENVO_03000038"/>
        <owl:annotatedProperty rdf:resource="http://purl.obolibrary.org/obo/IAO_0000115"/>
        <owl:annotatedTarget>Particulate matter which is composed primarily of dust, rock, and soot, as well as the microbial communities associated with these materials, deposited on an ice mass by an aeolian process.</owl:annotatedTarget>
        <oboInOwl:hasDbXref>http://www.nature.com/nrmicro/journal/v13/n11/full/nrmicro3522.html</oboInOwl:hasDbXref>
        <oboInOwl:hasDbXref>https://en.wikipedia.org/wiki/Cryoconite</oboInOwl:hasDbXref>
    </owl:Axiom>
    


    <!-- http://purl.obolibrary.org/obo/ENVO_03000063 -->

    <owl:Class rdf:about="http://purl.obolibrary.org/obo/ENVO_03000063">
        <rdfs:subClassOf rdf:resource="http://purl.obolibrary.org/obo/ENVO_01000277"/>
        <obo:IAO_0000111 xml:lang="en">new ice</obo:IAO_0000111>
        <obo:IAO_0000115>Water ice which is formed from freezing water and is suspended in a water body.</obo:IAO_0000115>
        <obo:IAO_0000116>Currently the new ice classes are not specific to sea water as they may form in non marine systems, but it would be good to confirm this especially for frazil ice.</obo:IAO_0000116>
        <obo:IAO_0000117 rdf:resource="http://orcid.org/0000-0002-4366-3088"/>
        <obo:IAO_0000117>http://orcid.org/0000-0002-3410-4655</obo:IAO_0000117>
        <oboInOwl:inSubset rdf:resource="http://bcodmo/sm#material"/>
        <oboInOwl:inSubset rdf:resource="http://bcodmo/sm#matrix"/>
        <oboInOwl:inSubset>envoPolar</oboInOwl:inSubset>
        <rdfs:comment>sea ice types include frazil, grease ice, slush, and shuga. These new ice classes refer to both marine water and fresh water ice. If using this term for annotation, use it in conjunction with another envo term to express whether the ice is in a marine, freshwater, or other system.</rdfs:comment>
        <rdfs:label xml:lang="en">new ice</rdfs:label>
    </owl:Class>
    <owl:Axiom>
        <owl:annotatedSource rdf:resource="http://purl.obolibrary.org/obo/ENVO_03000063"/>
        <owl:annotatedProperty rdf:resource="http://purl.obolibrary.org/obo/IAO_0000115"/>
        <owl:annotatedTarget>Water ice which is formed from freezing water and is suspended in a water body.</owl:annotatedTarget>
        <rdfs:comment>https://nsidc.org/cryosphere/glossary/term/new-ice</rdfs:comment>
    </owl:Axiom>
    


    <!-- http://purl.obolibrary.org/obo/ENVO_03000065 -->

    <owl:Class rdf:about="http://purl.obolibrary.org/obo/ENVO_03000065">
        <rdfs:subClassOf rdf:resource="http://purl.obolibrary.org/obo/ENVO_01000277"/>
        <obo:IAO_0000111 xml:lang="en">ice floe</obo:IAO_0000111>
        <obo:IAO_0000115>A cohesive and contiguous sheet of water ice which floats upon the surface of a water body.</obo:IAO_0000115>
        <obo:IAO_0000117 rdf:resource="http://orcid.org/0000-0002-4366-3088"/>
        <obo:IAO_0000117>http://orcid.org/0000-0002-3410-4655</obo:IAO_0000117>
        <oboInOwl:hasExactSynonym>ice floes</oboInOwl:hasExactSynonym>
        <oboInOwl:inSubset rdf:resource="http://bcodmo/sm#material"/>
        <oboInOwl:inSubset rdf:resource="http://bcodmo/sm#matrix"/>
        <oboInOwl:inSubset>envoPolar</oboInOwl:inSubset>
        <rdfs:comment>Ice floes can exist in sea ice, in rivers or lakes. The WMO offers the following extent-based classification. Floe giant: Over 10 km across.
Floe vast: 2-10 km across. Floe big: 500-2000 m across. Floe medium: 100-500 m across. Floe small: 20-100 m across. Ice cake: Less than 20 m across. Small ice cake: Less than 2 m across.</rdfs:comment>
        <rdfs:label xml:lang="en">ice floe</rdfs:label>
    </owl:Class>
    <owl:Axiom>
        <owl:annotatedSource rdf:resource="http://purl.obolibrary.org/obo/ENVO_03000065"/>
        <owl:annotatedProperty rdf:resource="http://purl.obolibrary.org/obo/IAO_0000115"/>
        <owl:annotatedTarget>A cohesive and contiguous sheet of water ice which floats upon the surface of a water body.</owl:annotatedTarget>
        <oboInOwl:hasDbXref>https://nsidc.org/cryosphere/glossary/term/ice-floe</oboInOwl:hasDbXref>
    </owl:Axiom>
    <owl:Axiom>
        <owl:annotatedSource rdf:resource="http://purl.obolibrary.org/obo/ENVO_03000065"/>
        <owl:annotatedProperty rdf:resource="http://www.w3.org/2000/01/rdf-schema#comment"/>
        <owl:annotatedTarget>Ice floes can exist in sea ice, in rivers or lakes. The WMO offers the following extent-based classification. Floe giant: Over 10 km across.
Floe vast: 2-10 km across. Floe big: 500-2000 m across. Floe medium: 100-500 m across. Floe small: 20-100 m across. Ice cake: Less than 20 m across. Small ice cake: Less than 2 m across.</owl:annotatedTarget>
        <oboInOwl:hasDbXref>http://hdl.handle.net/11329/394</oboInOwl:hasDbXref>
    </owl:Axiom>
    


    <!-- http://purl.obolibrary.org/obo/ENVO_03000066 -->

    <owl:Class rdf:about="http://purl.obolibrary.org/obo/ENVO_03000066">
        <rdfs:subClassOf rdf:resource="http://purl.obolibrary.org/obo/ENVO_03000065"/>
        <obo:IAO_0000111 xml:lang="en">sea ice floe</obo:IAO_0000111>
        <obo:IAO_0000115>An ice floe which is formed from frozen sea water, and floats upon the surface of a marine water body.</obo:IAO_0000115>
        <obo:IAO_0000117 rdf:resource="http://orcid.org/0000-0002-4366-3088"/>
        <obo:IAO_0000117>http://orcid.org/0000-0002-3410-4655</obo:IAO_0000117>
        <oboInOwl:hasDbXref>http://sweetontology.net/realmCryo/Floe</oboInOwl:hasDbXref>
        <oboInOwl:hasExactSynonym>sea ice floes</oboInOwl:hasExactSynonym>
        <oboInOwl:inSubset rdf:resource="http://bcodmo/sm#material"/>
        <oboInOwl:inSubset rdf:resource="http://bcodmo/sm#matrix"/>
        <oboInOwl:inSubset>envoPolar</oboInOwl:inSubset>
        <rdfs:label xml:lang="en">sea ice floe</rdfs:label>
    </owl:Class>
    <owl:Axiom>
        <owl:annotatedSource rdf:resource="http://purl.obolibrary.org/obo/ENVO_03000066"/>
        <owl:annotatedProperty rdf:resource="http://purl.obolibrary.org/obo/IAO_0000115"/>
        <owl:annotatedTarget>An ice floe which is formed from frozen sea water, and floats upon the surface of a marine water body.</owl:annotatedTarget>
        <oboInOwl:hasDbXref>https://nsidc.org/cryosphere/glossary/term/ice-floe</oboInOwl:hasDbXref>
    </owl:Axiom>
    


    <!-- http://purl.obolibrary.org/obo/ENVO_03000067 -->

    <owl:Class rdf:about="http://purl.obolibrary.org/obo/ENVO_03000067">
        <rdfs:subClassOf rdf:resource="http://purl.obolibrary.org/obo/ENVO_03000066"/>
        <obo:IAO_0000111 xml:lang="en">pancake ice</obo:IAO_0000111>
        <obo:IAO_0000115>A sea ice floe which has a rounded or circular shape and raised rims.</obo:IAO_0000115>
        <obo:IAO_0000117 rdf:resource="http://orcid.org/0000-0002-4366-3088"/>
        <obo:IAO_0000117>http://orcid.org/0000-0002-3410-4655</obo:IAO_0000117>
        <oboInOwl:inSubset rdf:resource="http://bcodmo/sm#material"/>
        <oboInOwl:inSubset rdf:resource="http://bcodmo/sm#matrix"/>
        <oboInOwl:inSubset>envoPolar</oboInOwl:inSubset>
        <rdfs:label xml:lang="en">pancake ice</rdfs:label>
    </owl:Class>
    <owl:Axiom>
        <owl:annotatedSource rdf:resource="http://purl.obolibrary.org/obo/ENVO_03000067"/>
        <owl:annotatedProperty rdf:resource="http://purl.obolibrary.org/obo/IAO_0000115"/>
        <owl:annotatedTarget>A sea ice floe which has a rounded or circular shape and raised rims.</owl:annotatedTarget>
        <oboInOwl:hasDbXref>https://en.wikipedia.org/wiki/Pancake_ice</oboInOwl:hasDbXref>
        <oboInOwl:hasDbXref>https://web.archive.org/web/20040712022508/http://ice-glaces.ec.gc.ca:80/App/WsvPageDsp.cfm?ID=10992&amp;Lang=eng</oboInOwl:hasDbXref>
    </owl:Axiom>
    


    <!-- http://purl.obolibrary.org/obo/ENVO_03000068 -->

    <owl:Class rdf:about="http://purl.obolibrary.org/obo/ENVO_03000068">
        <rdfs:subClassOf rdf:resource="http://purl.obolibrary.org/obo/ENVO_03000066"/>
        <obo:IAO_0000111 xml:lang="en">nilas</obo:IAO_0000111>
        <obo:IAO_0000115>A sea ice floe which is thin, elastic, continuous, and of a transparent gray color, which results from the freezing of new ice.</obo:IAO_0000115>
        <obo:IAO_0000117 rdf:resource="http://orcid.org/0000-0002-4366-3088"/>
        <obo:IAO_0000117>http://orcid.org/0000-0002-3410-4655</obo:IAO_0000117>
        <oboInOwl:inSubset rdf:resource="http://bcodmo/sm#material"/>
        <oboInOwl:inSubset rdf:resource="http://bcodmo/sm#matrix"/>
        <oboInOwl:inSubset>envoPolar</oboInOwl:inSubset>
        <rdfs:label xml:lang="en">nilas</rdfs:label>
    </owl:Class>
    <owl:Axiom>
        <owl:annotatedSource rdf:resource="http://purl.obolibrary.org/obo/ENVO_03000068"/>
        <owl:annotatedProperty rdf:resource="http://purl.obolibrary.org/obo/IAO_0000115"/>
        <owl:annotatedTarget>A sea ice floe which is thin, elastic, continuous, and of a transparent gray color, which results from the freezing of new ice.</owl:annotatedTarget>
        <oboInOwl:hasDbXref>http://encyclopedia2.thefreedictionary.com/nilas</oboInOwl:hasDbXref>
        <oboInOwl:hasDbXref>https://en.wikipedia.org/wiki/Sea_ice#New_ice.2C_nilas_and_young_ice</oboInOwl:hasDbXref>
        <oboInOwl:hasDbXref>https://nsidc.org/cryosphere/glossary/term/nilas</oboInOwl:hasDbXref>
    </owl:Axiom>
    


    <!-- http://purl.obolibrary.org/obo/ENVO_03000069 -->

    <owl:Class rdf:about="http://purl.obolibrary.org/obo/ENVO_03000069">
        <rdfs:subClassOf rdf:resource="http://purl.obolibrary.org/obo/ENVO_03000066"/>
        <obo:IAO_0000111 xml:lang="en">young ice</obo:IAO_0000111>
        <obo:IAO_0000115>A sea ice floe which is inflexible and thicker than nilas.</obo:IAO_0000115>
        <obo:IAO_0000117 rdf:resource="http://orcid.org/0000-0002-4366-3088"/>
        <obo:IAO_0000117>http://orcid.org/0000-0002-3410-4655</obo:IAO_0000117>
        <oboInOwl:inSubset rdf:resource="http://bcodmo/sm#material"/>
        <oboInOwl:inSubset rdf:resource="http://bcodmo/sm#matrix"/>
        <oboInOwl:inSubset>envoPolar</oboInOwl:inSubset>
        <rdfs:label xml:lang="en">young ice</rdfs:label>
    </owl:Class>
    <owl:Axiom>
        <owl:annotatedSource rdf:resource="http://purl.obolibrary.org/obo/ENVO_03000069"/>
        <owl:annotatedProperty rdf:resource="http://purl.obolibrary.org/obo/IAO_0000115"/>
        <owl:annotatedTarget>A sea ice floe which is inflexible and thicker than nilas.</owl:annotatedTarget>
        <oboInOwl:hasDbXref>https://en.wikipedia.org/wiki/Sea_ice#New_ice.2C_nilas_and_young_ice</oboInOwl:hasDbXref>
    </owl:Axiom>
    


    <!-- http://purl.obolibrary.org/obo/ENVO_03000071 -->

    <owl:Class rdf:about="http://purl.obolibrary.org/obo/ENVO_03000071">
        <rdfs:subClassOf rdf:resource="http://purl.obolibrary.org/obo/ENVO_00002200"/>
        <obo:IAO_0000111 xml:lang="en">first year ice</obo:IAO_0000111>
        <obo:IAO_0000115>Sea ice which has formed over a single freezing season.</obo:IAO_0000115>
        <obo:IAO_0000117 rdf:resource="http://orcid.org/0000-0002-4366-3088"/>
        <obo:IAO_0000117>http://orcid.org/0000-0002-3410-4655</obo:IAO_0000117>
        <oboInOwl:hasDbXref>http://sweetontology.net/realmCryo/SeasonalIce</oboInOwl:hasDbXref>
        <oboInOwl:hasRelatedSynonym>seasonal ice</oboInOwl:hasRelatedSynonym>
        <oboInOwl:inSubset rdf:resource="http://bcodmo/sm#material"/>
        <oboInOwl:inSubset rdf:resource="http://bcodmo/sm#matrix"/>
        <oboInOwl:inSubset>envoPolar</oboInOwl:inSubset>
        <rdfs:comment>Sea ice develops from young ice; thickness from 0.3 to 2 meters (1 to 6.6 feet).  Sea ice be subdivided into thin first-year ice (white ice), medium first-year ice, and thick first-year ice.  First-year ice is distinguished from older ice primarily by having a higher salinity. Undeformed first-year ice differs from older ice in that it is smoother and lacks refrozen melt ponds. Characteristically level where undisturbed by pressure, but where ridges occur, they  distinguished by being larger, more angular, and more porous than multiyear ridges.</rdfs:comment>
        <rdfs:label xml:lang="en">first year ice</rdfs:label>
    </owl:Class>
    <owl:Axiom>
        <owl:annotatedSource rdf:resource="http://purl.obolibrary.org/obo/ENVO_03000071"/>
        <owl:annotatedProperty rdf:resource="http://purl.obolibrary.org/obo/IAO_0000115"/>
        <owl:annotatedTarget>Sea ice which has formed over a single freezing season.</owl:annotatedTarget>
        <oboInOwl:hasDbXref>http://nsidc.org/arcticseaicenews/tag/first-year-ice/</oboInOwl:hasDbXref>
        <oboInOwl:hasDbXref>https://en.wikipedia.org/wiki/Sea_ice#New_ice.2C_nilas_and_young_ice</oboInOwl:hasDbXref>
        <oboInOwl:hasDbXref>https://orcid.org/0000-0003-4808-4736</oboInOwl:hasDbXref>
    </owl:Axiom>
    <owl:Axiom>
        <owl:annotatedSource rdf:resource="http://purl.obolibrary.org/obo/ENVO_03000071"/>
        <owl:annotatedProperty rdf:resource="http://www.geneontology.org/formats/oboInOwl#hasRelatedSynonym"/>
        <owl:annotatedTarget>seasonal ice</owl:annotatedTarget>
        <rdfs:comment>First year ice which melts before the next freezing season is often referred to as seasonal ice. By definition, seasonal ice cannot become second year ice.</rdfs:comment>
    </owl:Axiom>
    <owl:Axiom>
        <owl:annotatedSource rdf:resource="http://purl.obolibrary.org/obo/ENVO_03000071"/>
        <owl:annotatedProperty rdf:resource="http://www.w3.org/2000/01/rdf-schema#comment"/>
        <owl:annotatedTarget>Sea ice develops from young ice; thickness from 0.3 to 2 meters (1 to 6.6 feet).  Sea ice be subdivided into thin first-year ice (white ice), medium first-year ice, and thick first-year ice.  First-year ice is distinguished from older ice primarily by having a higher salinity. Undeformed first-year ice differs from older ice in that it is smoother and lacks refrozen melt ponds. Characteristically level where undisturbed by pressure, but where ridges occur, they  distinguished by being larger, more angular, and more porous than multiyear ridges.</owl:annotatedTarget>
        <oboInOwl:hasDbXref>https://orcid.org/0000-0003-4808-4736</oboInOwl:hasDbXref>
    </owl:Axiom>
    


    <!-- http://purl.obolibrary.org/obo/ENVO_03000072 -->

    <owl:Class rdf:about="http://purl.obolibrary.org/obo/ENVO_03000072">
        <rdfs:subClassOf rdf:resource="http://purl.obolibrary.org/obo/ENVO_00002200"/>
        <obo:IAO_0000111 xml:lang="en">second year ice</obo:IAO_0000111>
        <obo:IAO_0000115>Sea ice which is thicker than first year ice, and has survived a seasonal melting process.</obo:IAO_0000115>
        <obo:IAO_0000117 rdf:resource="http://orcid.org/0000-0002-4366-3088"/>
        <obo:IAO_0000117>http://orcid.org/0000-0002-3410-4655</obo:IAO_0000117>
        <oboInOwl:inSubset rdf:resource="http://bcodmo/sm#material"/>
        <oboInOwl:inSubset rdf:resource="http://bcodmo/sm#matrix"/>
        <oboInOwl:inSubset>envoPolar</oboInOwl:inSubset>
        <rdfs:label xml:lang="en">second year ice</rdfs:label>
    </owl:Class>
    <owl:Axiom>
        <owl:annotatedSource rdf:resource="http://purl.obolibrary.org/obo/ENVO_03000072"/>
        <owl:annotatedProperty rdf:resource="http://purl.obolibrary.org/obo/IAO_0000115"/>
        <owl:annotatedTarget>Sea ice which is thicker than first year ice, and has survived a seasonal melting process.</owl:annotatedTarget>
        <oboInOwl:hasDbXref>https://en.wikipedia.org/wiki/Sea_ice#New_ice.2C_nilas_and_young_ice</oboInOwl:hasDbXref>
    </owl:Axiom>
    


    <!-- http://purl.obolibrary.org/obo/ENVO_03000073 -->

    <owl:Class rdf:about="http://purl.obolibrary.org/obo/ENVO_03000073">
        <rdfs:subClassOf rdf:resource="http://purl.obolibrary.org/obo/ENVO_00002200"/>
        <obo:IAO_0000111 xml:lang="en">multiyear ice</obo:IAO_0000111>
        <obo:IAO_0000115>Sea ice which is thicker than second year ice, and has survived more than two seasonal melting process.</obo:IAO_0000115>
        <obo:IAO_0000117 rdf:resource="http://orcid.org/0000-0002-4366-3088"/>
        <obo:IAO_0000117>http://orcid.org/0000-0002-3410-4655</obo:IAO_0000117>
        <oboInOwl:inSubset rdf:resource="http://bcodmo/sm#material"/>
        <oboInOwl:inSubset rdf:resource="http://bcodmo/sm#matrix"/>
        <oboInOwl:inSubset>envoPolar</oboInOwl:inSubset>
        <rdfs:label xml:lang="en">multiyear ice</rdfs:label>
    </owl:Class>
    <owl:Axiom>
        <owl:annotatedSource rdf:resource="http://purl.obolibrary.org/obo/ENVO_03000073"/>
        <owl:annotatedProperty rdf:resource="http://purl.obolibrary.org/obo/IAO_0000115"/>
        <owl:annotatedTarget>Sea ice which is thicker than second year ice, and has survived more than two seasonal melting process.</owl:annotatedTarget>
        <oboInOwl:hasDbXref>https://en.wikipedia.org/wiki/Sea_ice#New_ice.2C_nilas_and_young_ice</oboInOwl:hasDbXref>
    </owl:Axiom>
    


    <!-- http://purl.obolibrary.org/obo/ENVO_03000075 -->

    <owl:Class rdf:about="http://purl.obolibrary.org/obo/ENVO_03000075">
        <rdfs:subClassOf rdf:resource="http://purl.obolibrary.org/obo/ENVO_03000063"/>
        <obo:IAO_0000111 xml:lang="en">shuga</obo:IAO_0000111>
        <obo:IAO_0000115>New ice, which is spongy, lumpy and opaque, and forms from water which freezes in an agitated water body.</obo:IAO_0000115>
        <obo:IAO_0000117 rdf:resource="http://orcid.org/0000-0002-4366-3088"/>
        <obo:IAO_0000117>http://orcid.org/0000-0002-3410-4655</obo:IAO_0000117>
        <oboInOwl:inSubset rdf:resource="http://bcodmo/sm#material"/>
        <oboInOwl:inSubset rdf:resource="http://bcodmo/sm#matrix"/>
        <oboInOwl:inSubset>envoPolar</oboInOwl:inSubset>
        <rdfs:comment>These new ice classes refer to both marine water and fresh water ice. If using this term for annotation, use it in conjunction with another envo term to express whether the ice is in a marine, freshwater, or other system.</rdfs:comment>
        <rdfs:label xml:lang="en">shuga</rdfs:label>
    </owl:Class>
    <owl:Axiom>
        <owl:annotatedSource rdf:resource="http://purl.obolibrary.org/obo/ENVO_03000075"/>
        <owl:annotatedProperty rdf:resource="http://purl.obolibrary.org/obo/IAO_0000115"/>
        <owl:annotatedTarget>New ice, which is spongy, lumpy and opaque, and forms from water which freezes in an agitated water body.</owl:annotatedTarget>
        <oboInOwl:hasDbXref>http://encyclopedia2.thefreedictionary.com/shuga</oboInOwl:hasDbXref>
        <oboInOwl:hasDbXref>https://nsidc.org/cryosphere/glossary/term/shuga</oboInOwl:hasDbXref>
    </owl:Axiom>
    


    <!-- http://purl.obolibrary.org/obo/ENVO_03000088 -->

    <owl:Class rdf:about="http://purl.obolibrary.org/obo/ENVO_03000088">
        <rdfs:subClassOf rdf:resource="http://purl.obolibrary.org/obo/ENVO_00000134"/>
        <obo:IAO_0000111 xml:lang="en">methane permafrost</obo:IAO_0000111>
        <obo:IAO_0000115>Permafrost which contains pockets of trapped methane gas.</obo:IAO_0000115>
        <obo:IAO_0000116>It would probably be better to assert parthood between the permafrost and cavities filled with gas rather than the gases themselves.</obo:IAO_0000116>
        <obo:IAO_0000117 rdf:resource="http://orcid.org/0000-0002-4366-3088"/>
        <obo:IAO_0000117>http://orcid.org/0000-0002-3410-4655</obo:IAO_0000117>
        <oboInOwl:hasExactSynonym>bulgunyakh</oboInOwl:hasExactSynonym>
        <oboInOwl:inSubset rdf:resource="http://bcodmo/sm#material"/>
        <oboInOwl:inSubset rdf:resource="http://bcodmo/sm#matrix"/>
        <oboInOwl:inSubset>envoPolar</oboInOwl:inSubset>
        <rdfs:comment>Other hydrocarbon gasses such as carbon dioxide may also be present. These pockets can be sufficently large that the permafrost surface will undulate when pressure is applied.</rdfs:comment>
        <rdfs:label xml:lang="en">methane permafrost</rdfs:label>
        <rdfs:label xml:lang="en">methane-laden permafrost</rdfs:label>
    </owl:Class>
    <owl:Axiom>
        <owl:annotatedSource rdf:resource="http://purl.obolibrary.org/obo/ENVO_03000088"/>
        <owl:annotatedProperty rdf:resource="http://purl.obolibrary.org/obo/IAO_0000115"/>
        <owl:annotatedTarget>Permafrost which contains pockets of trapped methane gas.</owl:annotatedTarget>
        <oboInOwl:hasDbXref>http://www.nature.com/news/mysterious-siberian-crater-attributed-to-methane-1.15649</oboInOwl:hasDbXref>
        <oboInOwl:hasDbXref>http://www.sciencealert.com/7-000-huge-gas-bubbles-have-formed-under-siberia-and-could-explode-at-any-moment</oboInOwl:hasDbXref>
    </owl:Axiom>
    


    <!-- http://purl.obolibrary.org/obo/ENVO_03000108 -->

    <owl:Class rdf:about="http://purl.obolibrary.org/obo/ENVO_03000108">
        <rdfs:subClassOf rdf:resource="http://purl.obolibrary.org/obo/ENVO_01000406"/>
        <obo:IAO_0000111 xml:lang="en">slab snow</obo:IAO_0000111>
        <obo:IAO_0000115>Snow which is cohesive, hard and overlies weaker snow.</obo:IAO_0000115>
        <obo:IAO_0000117 rdf:resource="http://orcid.org/0000-0002-4366-3088"/>
        <obo:IAO_0000117>http://orcid.org/0000-0002-3410-4655</obo:IAO_0000117>
        <oboInOwl:inSubset rdf:resource="http://bcodmo/sm#material"/>
        <oboInOwl:inSubset rdf:resource="http://bcodmo/sm#matrix"/>
        <oboInOwl:inSubset>envoPolar</oboInOwl:inSubset>
        <rdfs:label xml:lang="en">slab snow</rdfs:label>
    </owl:Class>
    <owl:Axiom>
        <owl:annotatedSource rdf:resource="http://purl.obolibrary.org/obo/ENVO_03000108"/>
        <owl:annotatedProperty rdf:resource="http://purl.obolibrary.org/obo/IAO_0000115"/>
        <owl:annotatedTarget>Snow which is cohesive, hard and overlies weaker snow.</owl:annotatedTarget>
        <oboInOwl:hasDbXref>http://www.fsavalanche.org/slab</oboInOwl:hasDbXref>
    </owl:Axiom>
    


    <!-- http://purl.obolibrary.org/obo/ENVO_04000007 -->

    <owl:Class rdf:about="http://purl.obolibrary.org/obo/ENVO_04000007">
        <rdfs:subClassOf rdf:resource="http://purl.obolibrary.org/obo/ENVO_00002006"/>
        <obo:IAO_0000111 xml:lang="en">lake water</obo:IAO_0000111>
        <obo:IAO_0000115>Water which is part of a lake.</obo:IAO_0000115>
        <dc:creator rdf:resource="http://orcid.org/0000-0003-1264-1166"/>
        <dc:date rdf:datatype="http://www.w3.org/2001/XMLSchema#dateTime">2019-03-20T20:15:54Z</dc:date>
        <oboInOwl:inSubset rdf:resource="http://bcodmo/sm#material"/>
        <oboInOwl:inSubset rdf:resource="http://bcodmo/sm#matrix"/>
        <oboInOwl:inSubset>envoNceas</oboInOwl:inSubset>
        <rdfs:label xml:lang="en">lake water</rdfs:label>
    </owl:Class>
    


    <!-- http://purl.obolibrary.org/obo/ENVO_1000746 -->

    <owl:Class rdf:about="http://purl.obolibrary.org/obo/ENVO_1000746">
        <rdfs:subClassOf rdf:resource="http://purl.obolibrary.org/obo/ENVO_01000155"/>
        <obo:IAO_0000111 xml:lang="en">marine mucilage</obo:IAO_0000111>
        <obo:IAO_0000115>A gelatinous material primarily composed of exopolymeric compounds with colloidal properties, formed through the aggregation of marine snow particles, often found in large sheets,  flocs, and clouds.</obo:IAO_0000115>
        <obo:IAO_0000116>See issue #276.
This class is complex as marine mucilage is quite complex. It will also requre new class creation in GO process for deeper semantics.</obo:IAO_0000116>
        <oboInOwl:hasBroadSynonym>sea snot</oboInOwl:hasBroadSynonym>
        <oboInOwl:inSubset rdf:resource="http://bcodmo/sm#material"/>
        <oboInOwl:inSubset rdf:resource="http://bcodmo/sm#matrix"/>
        <rdfs:comment>The formation of marine mucilage is often associated with conditions which stress marine microorganisms such as diatoms.</rdfs:comment>
        <rdfs:label xml:lang="en">marine mucilage</rdfs:label>
    </owl:Class>
    <owl:Axiom>
        <owl:annotatedSource rdf:resource="http://purl.obolibrary.org/obo/ENVO_1000746"/>
        <owl:annotatedProperty rdf:resource="http://purl.obolibrary.org/obo/IAO_0000115"/>
        <owl:annotatedTarget>A gelatinous material primarily composed of exopolymeric compounds with colloidal properties, formed through the aggregation of marine snow particles, often found in large sheets,  flocs, and clouds.</owl:annotatedTarget>
        <oboInOwl:hasDbXref>DOI:10.1371/journal.pone.0007006</oboInOwl:hasDbXref>
    </owl:Axiom>
    


    <!-- http://purl.obolibrary.org/obo/ENVO_2000007 -->

    <owl:Class rdf:about="http://purl.obolibrary.org/obo/ENVO_2000007">
        <rdfs:subClassOf rdf:resource="http://purl.obolibrary.org/obo/ENVO_01000560"/>
        <obo:IAO_0000111 xml:lang="en">biochar</obo:IAO_0000111>
        <obo:IAO_0000115>charcoal that is used as a soil amendment.</obo:IAO_0000115>
        <oboInOwl:created_by>cjm</oboInOwl:created_by>
        <oboInOwl:creation_date rdf:datatype="http://www.w3.org/2001/XMLSchema#dateTime">2018-11-03T19:28:29Z</oboInOwl:creation_date>
        <oboInOwl:inSubset rdf:resource="http://bcodmo/sm#material"/>
        <oboInOwl:inSubset rdf:resource="http://bcodmo/sm#matrix"/>
        <rdfs:label>biochar</rdfs:label>
        <rdfs:label xml:lang="en">biochar</rdfs:label>
    </owl:Class>
    <owl:Axiom>
        <owl:annotatedSource rdf:resource="http://purl.obolibrary.org/obo/ENVO_2000007"/>
        <owl:annotatedProperty rdf:resource="http://purl.obolibrary.org/obo/IAO_0000115"/>
        <owl:annotatedTarget>charcoal that is used as a soil amendment.</owl:annotatedTarget>
        <oboInOwl:hasDbXref>https://en.wikipedia.org/wiki/Biochar</oboInOwl:hasDbXref>
    </owl:Axiom>
    


    <!-- http://purl.obolibrary.org/obo/ENVO_2000045 -->

    <owl:Class rdf:about="http://purl.obolibrary.org/obo/ENVO_2000045">
        <obo:IAO_0000111 xml:lang="en">hydrocarbon material</obo:IAO_0000111>
        <oboInOwl:created_by>cjm</oboInOwl:created_by>
        <oboInOwl:creation_date rdf:datatype="http://www.w3.org/2001/XMLSchema#dateTime">2018-11-03T21:35:24Z</oboInOwl:creation_date>
        <oboInOwl:inSubset rdf:resource="http://bcodmo/sm#material"/>
        <oboInOwl:inSubset rdf:resource="http://bcodmo/sm#matrix"/>
        <rdfs:label xml:lang="en">hydrocarbon material</rdfs:label>
        <rdfs:label>hydrocarbon-based environmental material</rdfs:label>
    </owl:Class>
</rdf:RDF>



<!-- Generated by the OWL API (version 4.5.6) https://github.com/owlcs/owlapi -->

